@prefix rdf: <http://www.w3.org/1999/02/22-rdf-syntax-ns#>.
@prefix rdfs: <http://www.w3.org/2000/01/rdf-schema#>.
@prefix owl: <http://www.w3.org/2002/07/owl#>.
@prefix xsd: <http://www.w3.org/2001/XMLSchema#>.
@prefix skos: <http://www.w3.org/2004/02/skos/core#>.
@prefix dct: <http://purl.org/dc/terms/>.
@prefix cidoc: <http://www.cidoc-crm.org/cidoc-crm/>.
# @prefix frbroo: <http://iflastandards.info/ns/fr/frbr/frbroo/>.
@prefix text: <http://www.nie-ine.ch/ontology/text#>.
@prefix kb: <http://www.knora.org/ontology/knora-base#>.
@prefix sg: <http://www.knora.org/ontology/salsah-gui>.
@prefix image: <http://www.nie-ine.ch/ontology/image#>.

<http://www.nie-ine.ch/ontology/image>
	a owl:Ontology;
	dct:title "An ontology about image"@en;
	dct:description """Formal description of image in broadest sense, general subclasses, related classes e.g. carrier, and properties."""@en;
	rdfs:isDefinedBy <http://www.nie-ine.ch/ontology/image#>;
#	owl:versionInfo "Version x - yyyy-mm-dd"@en;	# OR other format, datatype
	dct:creator "Hans Cools, software developer, NIE, Basel University, Switzerland"@en;
	dct:conformsTo "OWL Full"@en.

# general:
	# DB: mapping to mysql elements
		# KR
		# PL

#
# CLASSES
#

# cidoc:E73_Information_Object # physical carrier, e.g. human memory, on one or more carriers simultaneously

image:Image
	a rdfs:Class;
	rdfs:label "image"@en,"Bild"@de;
	rdfs:comment """2-dimensional representation of a resource made with artificial light processing."""@en;
	rdfs:isDefinedBy <http://www.nie-ine.ch/ontology/image#>;
	rdfs:subClassOf cidoc:E38_Image, kb:StillImageFileValue, [
		a owl:Restriction; owl:onProperty text:hasNameObject; owl:minCardinality "1"^^xsd:nonNegativeInteger].

# https://raw.githubusercontent.com/dhlab-basel/Knora/develop/webapi/_test_data/ontologies/images-onto.ttl

image:StillImageRepresentationLinkValue
	a rdfs:Class;
	rdfs:label "still image representation link value"@en,"Bild-Repräsentationslinkwert"@de;
	rdfs:comment """Statement reification describing a link between a resource and a still image representation thereof."""@en;
	rdfs:isDefinedBy <http://www.nie-ine.ch/ontology/image#>;
	rdfs:subClassOf kb:LinkValue.

#
# PROPERTIES
#

image:hasImage
	a owl:ObjectProperty;
	rdfs:label "has image";
	rdfs:comment """Relating a resource to an image thereof."""@en;
	rdfs:isDefinedBy <http://www.nie-ine.ch/ontology/image#>;
	owl:propertyChainAxiom (image:hasStillImageRepresentation kb:hasStillImageFileValue);
	rdfs:domain rdfs:Resource;
	rdfs:range image:Image.

image:hasStillImageRepresentation
	a owl:ObjectProperty;
	rdfs:label "has still image representation"@en, "hat Bild-Repräsentation"@de;
	rdfs:comment """Relating a resource to an abstract 2-dimensional image representation thereof."""@en;
	rdfs:isDefinedBy <http://www.nie-ine.ch/ontology/image#>;
	rdfs:subPropertyOf kb:hasRepresentation;
	kb:subjectClassConstraint kb:Resource;
	kb:objectClassConstraint kb:StillImageRepresentation.

image:hasStillImageRepresentationLinkValue
	a owl:ObjectProperty;
	rdfs:label "has still image representation value"@en;
	rdfs:comment """Relating a resource to a statement reification describing a link between that resource and another one."""@en;
	rdfs:isDefinedBy <http://www.nie-ine.ch/ontology/image>;
	rdfs:subPropertyOf kb:hasRepresentationValue;
	kb:subjectClassConstraint kb:Resource;
	kb:objectClassConstraint kb:StillImageRepresentationLinkValue.
