@prefix rdfs: <http://www.w3.org/2000/01/rdf-schema#>.
@prefix owl: <http://www.w3.org/2002/07/owl#>.
@prefix xsd: <http://www.w3.org/2001/XMLSchema#>.
@prefix skos: <http://www.w3.org/2004/02/skos/core#>.
@prefix dct: <http://purl.org/dc/terms/>.
@prefix foaf: <http://xmlns.com/foaf/0.1/>.
@prefix unicore: <http://purl.uniprot.org/core/>.
@prefix frbroo: <http://iflastandards.info/ns/fr/frbr/frbroo/>.
@prefix event: <http://www.nie-ine.ch/event#>.
@prefix standard: <http://www.nie-ine.ch/standards#>.
@prefix kb: <http://www.knora.org/ontology/knora-base#>.
@prefix lang: <http://www.nie-ine.ch/ontology/language#>.

<http://www.nie-ine.ch/ontology/language>
	a owl:Ontology;
	dct:title "An ontology about language"@en;
	dct:description """Formal description of language, general subclasses, related classes and properties."""@en;
	rdfs:isDefinedBy <http://www.nie-ine.ch/ontology/language#>;
#	owl:versionInfo "Version x - yyyy-mm-dd"@en;	# OR other format, datatype
	dct:creator "Hans Cools, software developer, NIE, Basel University, Switzerland"@en;
	dct:conformsTo "OWL Full"@en.


# general:
	# DB: mysql elements
		# krd: Raeber
		# PL: Lombardus
	# TBS: to be specified


#
# CLASSES
#

lang:Language
	a rdfs:Class;
	rdfs:label "language"@en, "Sprache"@de;
	rdfs:comment """A dynamic set of sensory signs, including sounds and gestures, of communication and the semantic, pragmatic, and grammar elements or rules to manipulate them."""@en;
	rdfs:isDefinedBy <http://www.nie-ine.ch/ontology/language#>;
	rdfs:subClassOf dct:LinguisticSystem, kb:Resource, [
		a owl:Restriction; owl:onProperty lang:hasLanguageValue; owl:minCardinality "0"^^xsd:nonNegativeInteger].

lang:LanguageCodeObject
	a rdfs:Class;
	rdfs:label "language code object"@en, "Sprache-Kode-Objekt"@de;
	rdfs:comment """A abstract element representing an objectivation of a standard language code, e.g. ISO 639."""@en;
	rdfs:isDefinedBy <http://www.nie-ine.ch/ontology/language#>;
	rdfs:subClassOf kb:Value, [
		a owl:Restriction; owl:onProperty lang:hasCode; owl:minCardinality "1"^^xsd:nonNegativeInteger].

# lang:Expressing
# 	a rdfs:Class;
# 	rdfs:label """language expressing"""@en;
# 	skos:definition """Expressing a language."""@en;
# 	rdfs:isDefinedBy <http://www.nie-ine.ch/ontology/language#>;
# 	rdfs:subClassOf event:Action.

# lang:Expression
# 	a rdfs:Class;
# 	rdfs:label """language expression"""@en;
# 	skos:definition """Expression in a language."""@en;
# 	rdfs:isDefinedBy <http://www.nie-ine.ch/ontology/language#>;
# 	rdfs:subClassOf [a owl:Restriction; owl:onProperty event:outputOf; owl:someValuesFrom lang:Expressing].

#
# PROPERTIES
#

lang:hasLanguage # relating something to a language as a resource, not as a kb:Value
	a owl:ObjectProperty;
	rdfs:label "has language"@en, "hat Sprache"@de;
	rdfs:comment """Relating a resource to a language e.g. in which an information resource is expressed."""@en;
	rdfs:isDefinedBy <http://www.nie-ine.ch/ontology/language#>;
	rdfs:subPropertyOf dct:language, kb:hasLinkTo;
	rdfs:domain rdfs:Resource;
	rdfs:range lang:Language;
	kb:subjectClassConstraint kb:Resource; # Knora requirement
	kb:objectClassConstraint lang:Language. # Knora requirement

lang:hasLanguageStatement # Knora requirement
	a owl:ObjectProperty;
	rdfs:label "has language statement"@en, "hat Sprache-Aussage"@de;
	rdfs:comment """Relating a resource to a language statement as reification of the relation between the resource and the language as a resource."""@en;
	rdfs:isDefinedBy <http://www.nie-ine.ch/ontology/language#>;
	rdfs:subPropertyOf kb:hasLinkToValue;
	kb:subjectClassConstraint kb:Resource; # Knora requirement
	kb:objectClassConstraint kb:LinkValue. # Knora requirement

lang:hasLanguageCodeObject
	a owl:ObjectProperty;
	rdfs:label "has language code object"@en, "hat Sprache-Kode-Objekt"@de;
	rdfs:comment """Relating a resource to a language code object representing a language e.g. in which an information resource is expressed."""@en;
	rdfs:isDefinedBy <http://www.nie-ine.ch/ontology/language#>;
	rdfs:subPropertyOf kb:hasValue;
	rdfs:domain rdfs:Resource;
	rdfs:range lang:LanguageCodeObject;
	kb:subjectClassConstraint kb:Resource;
	kb:objectClassConstraint lang:LanguageCodeObject.

lang:hasCode
	a owl:DatatypeProperty;
	rdfs:label "has code"@en, "hat Kode"@de;
	rdfs:comment """Relating a language code object to a standard language code, e.g. of ISO 639."""@en;
	rdfs:isDefinedBy <http://www.nie-ine.ch/ontology/language#>;
	rdfs:subPropertyOf kb:valueHas;
	kb:subjectClassConstraint lang:LanguageCodeObject;
	kb:objectDatatypeConstraint [a rdfs:Datatype; owl:oneOf(standard:iso639-1Datatype standard:iso639-2Datatype standard:iso639-3Datatype)]. # instead of xsd:string

lang:hasLanguageCode # DB: jsmwh_k2_categories/language, jsmwh_k2_items/language
	a owl:DatatypeProperty;
	rdfs:label "has language code"@en;
	rdfs:comment """Relating a resource to a language code."""@en;
	rdfs:isDefinedBy <http://www.nie-ine.ch/ontology/language#>;
	owl:propertyChainAxiom (lang:hasLanguageCodeObject lang:hasCode);
	rdfs:domain rdfs:Resource;
	rdfs:range [a rdfs:Datatype; owl:oneOf(standard:iso639-1Datatype standard:iso639-2Datatype standard:iso639-3Datatype)]. # instead of xsd:string