@prefix rdfs: <http://www.w3.org/2000/01/rdf-schema#>.
@prefix owl: <http://www.w3.org/2002/07/owl#>.
@prefix skos: <http://www.w3.org/2004/02/skos/core#>.
@prefix dct: <http://purl.org/dc/terms/>.
@prefix standard: <http://www.nie-ine.ch/ontology/standards#>.

<http://www.nie-ine.ch/ontology/standards>
	a owl:Ontology;
	dct:title "An ontology about standards"@en;
	dct:description """Formal description of standards, subclasses, and properties."""@en;
	rdfs:isDefinedBy <http://www.nie-ine.ch/ontology/standards#>;
#	owl:versionInfo "Version x - yyyy-mm-dd"@en;	# OR other format, datatype
	dct:creator "Hans Cools, software developer, NIE, Basel University, Switzerland"@en;
	dct:conformsTo "OWL Full"@en.

#
# SKOS CONCEPT SCHEME AND DATATYPE INSTANCES
#

## LANGUAGE

standard:iso639
	a skos:ConceptScheme;
	rdfs:label "ISO 639"@en;
	rdfs:comment """International standard for codes for the representation of names of languages."""@en;
	rdfs:isDefinedBy <http://www.nie-ine.ch/ontology/standards#>;
	rdfs:seeAlso <https://www.iso.org/iso-639-language-codes.html>.

standard:iso639-1
	a skos:ConceptScheme;
	rdfs:label "ISO 639-1"@en;
	rdfs:comment """ISO 639 part 1: alpha-2 (two-letter) codes."""@en;
	rdfs:isDefinedBy <http://www.nie-ine.ch/ontology/standards#>;
	rdfs:subClassOf standard:iso639;
	dct:hasVersion "ISO 639-1:2002";
	standard:hasDataType standard:iso639-1Datatype;
	rdfs:seeAlso <http://www.infoterm.info/standardization/iso_639_1_2002.php>.

standard:iso639-1Datatype
	a rdfs:Datatype;
	rdfs:label "ISO 639-1 datatype"@en;
	rdfs:comment """Datatype to type an ISO 639-1 alpha-2 code."""@en;
	rdfs:isDefinedBy <http://www.nie-ine.ch/ontology/standards#>.

standard:iso639-2
	a skos:ConceptScheme;
	rdfs:label "ISO 639-2"@en;
	rdfs:comment """ISO 639 part 2: alpha-3 (three-letter) codes."""@en;
	rdfs:isDefinedBy <http://www.nie-ine.ch/ontology/standards#>;
	rdfs:subClassOf standard:iso639;
	dct:hasVersion "ISO 639-2:1998";
	standard:hasDataType standard:iso639-2Datatype;
	rdfs:seeAlso <http://www.loc.gov/standards/iso639-2/>.

standard:iso639-2Datatype
	a rdfs:Datatype;
	rdfs:label "ISO 639-2 datatype"@en;
	rdfs:comment """Datatype to type an ISO 639-2 alpha-3 code."""@en;
	rdfs:isDefinedBy <http://www.nie-ine.ch/ontology/standards#>.

standard:iso639-3
	a skos:ConceptScheme;
	rdfs:label "ISO 639-3"@en;
	rdfs:comment """ISO 639 part 3: alpha-3 (three-letter) codes for comprehensive coverage of languages."""@en;
	rdfs:isDefinedBy <http://www.nie-ine.ch/ontology/standards#>;
	rdfs:subClassOf standard:iso639;
	dct:hasVersion "ISO 639-3:2007";
	standard:hasDataType standard:iso639-3Datatype;
	rdfs:seeAlso <http://www-01.sil.org/iso639-3/>.

standard:iso639-3Datatype
	a rdfs:Datatype;
	rdfs:label "ISO 639-3 datatype"@en;
	rdfs:comment """Datatype to type an ISO 639-3 alpha-3 code."""@en;
	rdfs:isDefinedBy <http://www.nie-ine.ch/ontology/standards#>.

## COUNTRY

standard:iso3166
	a skos:ConceptScheme;
	rdfs:label "ISO 3166"@en;
	rdfs:comment """International standard for codes for the representation of names of countries and their subdivisions."""@en;
	rdfs:isDefinedBy <http://www.nie-ine.ch/ontology/standards#>;
	rdfs:seeAlso <https://www.iso.org/iso-3166-country-codes.html>.

standard:iso3166-1
	a skos:ConceptScheme;
	rdfs:label "ISO 3166 part 1"@en;
	rdfs:comment """ISO 3166 part 1: country codes including codes for the names of dependent territories and special areas of geographical interest."""@en;
	rdfs:isDefinedBy <http://www.nie-ine.ch/ontology/standards#>;
	rdfs:subClassOf standard:iso3166;
	dct:hasVersion "ISO 3166-1:2013";
	rdfs:seeAlso <https://www.iso.org/standard/63545.html>.

standard:iso3166-1-alpha-2
	a skos:ConceptScheme;
	rdfs:label "ISO 3166 part 1 alpha-2"@en;
	rdfs:comment """ISO 3166 part 1: alpha-2 (two-letter) country codes."""@en;
	rdfs:isDefinedBy <http://www.nie-ine.ch/ontology/standards#>;
	rdfs:subClassOf standard:iso3166-1;
	standard:hasDataType standard:iso3166-1-alpha-2Datatype.

standard:iso3166-1-alpha-2Datatype
	a rdfs:Datatype;
	rdfs:label "ISO 3166 part 1 alpha-2 datatype"@en;
	rdfs:comment """Datatype to type an ISO 3166-1 alpha-2 code."""@en;
	rdfs:isDefinedBy <http://www.nie-ine.ch/ontology/standards#>.

standard:iso3166-1-alpha-3
	a skos:ConceptScheme;
	rdfs:label "ISO 3166 part 1 alpha-3"@en;
	rdfs:comment """ISO 3166 part 1: alpha-3 (three-letter) country codes."""@en;
	rdfs:isDefinedBy <http://www.nie-ine.ch/ontology/standards#>;
	rdfs:subClassOf standard:iso3166-1;
	standard:hasDataType standard:iso3166-1-alpha-3Datatype.

standard:iso3166-1-alpha-3Datatype
	a rdfs:Datatype;
	rdfs:label "ISO 3166 part 1 alpha-3 datatype"@en;
	rdfs:comment """Datatype to type an ISO 3166-1 alpha-3 code."""@en;
	rdfs:isDefinedBy <http://www.nie-ine.ch/ontology/standards#>.

standard:iso3166-1-num
	a skos:ConceptScheme;
	rdfs:label "ISO 3166 part 1 numeric"@en;
	rdfs:comment """ISO 3166 part 1: numeric country codes."""@en;
	skos:note """Identical to codes of the United Nations Statistics Division."""@en;
	rdfs:isDefinedBy <http://www.nie-ine.ch/ontology/standards#>;
	rdfs:subClassOf standard:iso3166-1;
	standard:hasDataType standard:iso3166-1-numDatatype.

standard:iso3166-1-numDatatype
	a rdfs:Datatype;
	rdfs:label "ISO 3166 part 1 numeric datatype"@en;
	rdfs:comment """Datatype to type an ISO 3166-1 numeric code."""@en;
	rdfs:isDefinedBy <http://www.nie-ine.ch/ontology/standards#>.

standard:iso3166-2
	a skos:ConceptScheme;
	rdfs:label "ISO 3166 part 2"@en;
	rdfs:comment """ISO 3166 part 2: codes for the names of the principal subdivisions (e.g. provinces or states) of countries coded in ISO 3166 part 1."""@en;
	skos:note """The first part of a code is the ISO 3166-1 alpha-2 code; the second part is a string of up to three alphanumeric characters stemming from a national coding system of the country concerned, or developed by the ISO itself."""@en;
	rdfs:isDefinedBy <http://www.nie-ine.ch/ontology/standards#>;
	rdfs:subClassOf standard:iso3166;
	dct:hasVersion "ISO 3166-2:2013";
	standard:hasDataType standard:iso3166-2Datatype;
	rdfs:seeAlso <https://www.iso.org/standard/63546.html>.

standard:iso3166-2Datatype
	a rdfs:Datatype;
	rdfs:label "ISO 3166 part 2 datatype"@en;
	rdfs:comment """Datatype to type an ISO 3166-2 code."""@en;
	rdfs:isDefinedBy <http://www.nie-ine.ch/ontology/standards#>.

# to add standard:iso3166-3

#
# PROPERTIES
#

standard:hasDataType
	a owl:ObjectProperty;
	rdfs:label "has data type"@en;
	rdfs:comment """Relating a SKOS concept scheme to its data type."""@en;
	rdfs:isDefinedBy <http://www.nie-ine.ch/ontology/standards#>;
	rdfs:domain skos:ConceptScheme;
	rdfs:range rdfs:Datatype;
	kb:subjectClassConstraint skos:ConceptScheme;
	kb:objectClassConstraint rdfs:Datatype.