@prefix rdf: <http://www.w3.org/1999/02/22-rdf-syntax-ns#>.
@prefix rdfs: <http://www.w3.org/2000/01/rdf-schema#>.
@prefix owl: <http://www.w3.org/2002/07/owl#>.
@prefix xml: <http://www.w3.org/XML/1998/namespace>.
@prefix xsd: <http://www.w3.org/2001/XMLSchema#>.
@prefix skos: <http://www.w3.org/2004/02/skos/core#>.
@prefix dct: <http://purl.org/dc/terms/>.
@prefix foaf: <http://xmlns.com/foaf/0.1/>.
@prefix frbroo: <http://iflastandards.info/ns/fr/frbr/frbroo/>.
@prefix text: <http://www.nie-ine.ch/text#>.
@prefix kb: <http://www.knora.org/ontology/knora-base#>.
@prefix ka: <http://www.knora.org/ontology/knora-admin#>.
@prefix work: <http://www.nie-ine.ch/ontology/work#>.

# @prefix bibo: <http://purl.org/ontology/bibo/>. # dereferences via http://bibliographic-ontology.org/bibo/bibo.php to rdf-xml file
# proposed not to use it, cf. NIE_ontology_evaluation_bibo.txt
# @prefix biblio: <http://www.knora.org/ontology/biblio#> . # not yet in production; uses bibo

@prefix krd: <http://www.nie-ine.ch/kunoRaeber-data#>.	# mock-up

<http://www.nie-ine.ch/ontology/work>
	a owl:Ontology;
	dct:title "An ontology about work"@en;
	dct:description """Formal description of work as  in broadest sense, and general subclasses, related classes and properties."""@en;
	rdfs:isDefinedBy <http://www.nie-ine.ch/ontology/work#>;
	owl:versionInfo "Version x - yyyy-mm-dd"@en;	# OR other format, datatype
	dct:creator "Hans Cools, software developer, NIE, Basel University, Switzerland"@en;
	dct:conformsTo "OWL Full"@en.

# general:
	# DB: mysql elements
		# krd: Raeber
		# PL: Lombardus
	# TBS: to be specified

#
# CLASSES
#

# frbroo:F14_Individual_Work
# frbroo:R3_is_realised_in
# frbroo:F22_Self-Contained_Expression

work:Work # DB KR: Synopse where ?: cf. itemlist/tag
	a rdfs:Class;
	rdfs:label "work"@en, "Werk"@de;
	rdfs:comment """See http://iflastandards.info/ns/fr/frbr/frbroo/F14_Individual_Work."""@en;
	rdfs:isDefinedBy <http://www.nie-ine.ch/ontology/work#>;
	rdfs:subClassOf frbroo:F14_Individual_Work, kb:Resource, [
		a owl:Restriction; owl:onProperty text:hasName; owl:minCardinality "0"^^xsd:nonNegativeInteger].

# e.g. on page http://www.kunoraeber.ch/feetest/index.php/notizbuecher/notizbuch-1979-1982
# 'Synopse: Museggeromgang' = link:
# http://www.kunoraeber.ch/feetest/index.php/notizbuecher/notizbuch-1979-1982/itemlist/tag/Museggeromgang
# to page with in upper left corner 'Synopse: Museggeromgang (6)'



# published -> creation, made public in DB online

#	rdfs:subClassOf kb:TextRepresentation. # OR kb:DocumentRepresentation?
#	kb:hasTextFileValue krd:IntrotextFileValue: needed? ~ cardinality  


# krd:_	kb:hasTextFileValue kb:TextFileValue; :valueHasString


# krd:creatorOf foaf:Agent
# krd:createdBy


# frbroo:

work:hasManifestation
	a owl:ObjectProperty;
	rdfs:label "has manifestation"@en;
	rdfs:comment "A property linking a particular work to its manifestations. This property is additional to the relationships between FRBR endeavours present in the classical FRBR data model."@en;
	rdfs:domain work:Work;
	rdfs:range work:Manifestation;
	owl:propertyChainAxiom (work:hasRealization work:hasEmbodiment).


	
