@prefix rdfs: <http://www.w3.org/2000/01/rdf-schema#>.
@prefix owl: <http://www.w3.org/2002/07/owl#>.
@prefix xsd: <http://www.w3.org/2001/XMLSchema#>.
@prefix skos: <http://www.w3.org/2004/02/skos/core#>.
@prefix dct: <http://purl.org/dc/terms/>.
@prefix human: <http://www.nie.org/ontology/human#>.
@prefix language: <http://www.nie.org/ontology/language#>.
@prefix teach: <http://www.nie.org/ontology/teaching#>.
@prefix document: <http://www.nie.org/ontology/document#>.
@prefix text: <http://www.nie.org/ontology/text#>.
@prefix text-expression: <http://www.nie.org/ontology/text-expression#>.
@prefix text-structure: <http://www.nie.org/ontology/text-structure#>.
@prefix prosodic-structure: <http://www.nie.org/ontology/prosodic-structure#>.
@prefix textedit: <http://www.nie.org/ontology/text-editing#>.
@prefix scholarly-editing: <http://www.nie.org/ontology/scholarly-editing#>.
@prefix publish: <http://www.nie.org/ontology/publishing#>.
@prefix literature: <http://www.nie.org/ontology/literature#>.

# @base <http://www.nie.org/ontology/delille>.
@prefix delille: <http://www.nie.org/ontology/delille#>.

<http://www.nie.org/ontology/delille>
	a owl:Ontology;
	dct:license <http://creativecommons.org/licenses/by/3.0/>;
	dct:title "An ontology about Jacques Delille's poetry"@en; #*
	dct:description """Formal description of specific concepts in the scientific study of poetry of Jacques Delille, 22 June 1738 – 1 May 1813."""@en;
	dct:creator "Hans Cools, MD, knowledge engineer, ontologist, software developer, NIE-INE, Basel University, Switzerland"@en;
	dct:contributor "Roberta Padlina, tool coordinator and software developer, NIE-INE, University of Basel, Switzerland"@en;
	dct:publisher "University of Basel, Switzerland"@en.

#
# CLASSES
#

delille:VersePoem
	rdfs:isDefinedBy <http://www.nie.org/ontology/delille#>;
	a rdfs:Class;
	rdfs:label "Jacques Delille verse poem"@en, "Versgedicht Jacques Delilles"@de;
	rdfs:comment """Verse poem authored by Jacques Delille."""@en;
	rdfs:subClassOf literature:VersePoem, publish:Expression.

delille:TranslatedVersePoem
	rdfs:isDefinedBy <http://www.nie.org/ontology/delille#>;
	a rdfs:Class;
	rdfs:label "Translated Jacques Delille verse poem"@en, "übersetzter gereimter Versgedicht Jacques Delilles"@de;
	rdfs:comment """Translated Jacques Delille verse poem."""@en;
	rdfs:subClassOf delille:VersePoem, language:PersonTranslation, text:Translation.

delille:EditedVersePoem
	rdfs:isDefinedBy <http://www.nie.org/ontology/delille#>;
	a rdfs:Class;
	rdfs:label "edited Jacques Delille verse poem"@en, "ediertes Versgedicht Jacques Delilles"@de;
	rdfs:comment """Verse poem authored by Jacques Delille and edited."""@en;
	rdfs:subClassOf delille:VersePoem, textedit:Edition.

delille:Canto
	rdfs:isDefinedBy <http://www.nie.org/ontology/delille#>;
	a rdfs:Class;
	rdfs:label "Jacques Delille canto"@en, "Canto Jacques Delilles"@de, "chant de Jacques Delille"@fr, "canto di Jacques Delille"@it;
	rdfs:comment """Group of strophes in a verse poem authored by Jacques Delille."""@en;
	rdfs:subClassOf prosodic-structure:VerseSection, text-expression:ExpressionPart.

delille:Dictionary
	rdfs:isDefinedBy <http://www.nie.org/ontology/delille#>;
	a rdfs:Class;
	rdfs:label "citing dictionary"@en, "zitierendes Wörterbuch"@de; #, ""@fr, ""@it;
	rdfs:comment """Dictionary citing one or more verses of a poem authored by Jacques Delille."""@en;
	rdfs:subClassOf text-expression:Dictionary, publish:TextExpression.

delille:AnthologyOrManual
	rdfs:isDefinedBy <http://www.nie.org/ontology/delille#>;
	a rdfs:Class;
	rdfs:label "citing anthology or teaching manual"@en, "zitierende/s Anthologie oder Lehrbuch"@de; #, ""@fr, ""@it;
	rdfs:comment """Anthology or teaching manual citing one or more verses of a poem authored by Jacques Delille."""@en;
	rdfs:subClassOf publish:TextExpression.
#	owl:disjointUnionOf (literature:Anthology teach:Manual).

delille:LiteraryExpression
	rdfs:isDefinedBy <http://www.nie.org/ontology/delille#>;
	a rdfs:Class;
	rdfs:label "citing literary publication expression"@en, "zitierende literarische Publikationsexpression"@de; #, ""@fr, ""@it;
	rdfs:comment """Literary publication expression citing one or more verses of a poem authored by Jacques Delille."""@en;
	rdfs:subClassOf literature:Expression, publish:TextExpression.

delille:PoemOrVersePlay
	rdfs:isDefinedBy <http://www.nie.org/ontology/delille#>;
	a rdfs:Class;
	rdfs:label "citing poem or verse play"@en, "zitierendes Gedicht oder Vers-Theaterstück"@de, "poème ou pièce de théâtre en vers citante"@fr; #, ""@it;
	rdfs:comment """Poem or verse play citing one or more verses of a poem authored by Jacques Delille."""@en;
	rdfs:subClassOf delille:LiteraryExpression.

delille:Novel
	rdfs:isDefinedBy <http://www.nie.org/ontology/delille#>;
	a rdfs:Class;
	rdfs:label "citing novel"@en, "zitierender Roman"@de; #, "récit fictionnel"@fr, ""@it;
	rdfs:comment """Novel citing one or more verses of a poem authored by Jacques Delille."""@en;
	rdfs:subClassOf literature:Novel, delille:LiteraryExpression.

delille:EssayOrPanoramicLiteraryOrPhilisophicOrHumanitiesExpression # mix of literary and scientific expressions?
	rdfs:isDefinedBy <http://www.nie.org/ontology/delille#>;
	a rdfs:Class;
	rdfs:label "citing essay, or panoramic literary, philisophic or Humanities expression"@en, "zitierendes Essay, oder panoramisch literarisch, philosophisch oder geisteswissenschaftliche Expression"@de, "essai citant , ou expression littéraire panoramique et pittoresque, philosophique ou scientifique humaines"@fr; #, ""@it;
	rdfs:comment """Essay, or panoramic literary, philisophic or Humanities publication expression citing one or more verses of a poem authored by Jacques Delille."""@en;
	rdfs:subClassOf delille:LiteraryExpression.

delille:LiteraryNonfictionExpression
	rdfs:isDefinedBy <http://www.nie.org/ontology/delille#>;
	a rdfs:Class;
	rdfs:label "citing literary nonfiction expression"@en, "zitierende sachliche literarische Expression"@de, "expression littéraire non-fiction citante"@fr; #, ""@it;
	rdfs:comment """Literary nonfiction expression citing one or more verses of a poem authored by Jacques Delille, being a memoir, biography, history, anecdote, or correspondence."""@en;
	rdfs:subClassOf delille:LiteraryExpression, [
		a owl:Restriction; owl:onProperty literature:hasGenre; owl:someValuesFrom literature:Nonfiction].

delille:LiteraryScientificExpression
	rdfs:isDefinedBy <http://www.nie.org/ontology/delille#>;
	a rdfs:Class;
	rdfs:label "citing literary scientific expression"@en, "zitierende Literaturwissenschaftliche Expression"@de, "expression scientifique littéraire citante"@fr; #, ""@it;
	rdfs:comment """Literary scientific publication expression in esthetics, poetry and literary history, citing one or more verses of a poem authored by Jacques Delille."""@en;
	rdfs:subClassOf text-expression:ScientificExpression, publish:TextExpression.

delille:ScientificOrVulgarizedExpression
	rdfs:isDefinedBy <http://www.nie.org/ontology/delille#>;
	a rdfs:Class;
	rdfs:label "citing scientific or vulgarized publication expression"@en, "zitierende wissenschaftliche oder vulgarisierte Publikation-Expression"@de;
	rdfs:comment """Scientific or vulgarized publication expression citing one or more verses of a poem authored by Jacques Delille."""@en;
	rdfs:subClassOf text-expression:ScientificExpression, publish:TextExpression.

delille:Catalogue
	rdfs:isDefinedBy <http://www.nie.org/ontology/delille#>;
	a rdfs:Class;
	rdfs:label "citing catalogue"@en, "zitierende Katalog"@de;
	rdfs:comment """Catalogue citing one or more verses of a poem authored by Jacques Delille."""@en;
	rdfs:subClassOf document:Catalogue, publish:TextExpression.

delille:Commentary
	rdfs:isDefinedBy <http://www.nie.org/ontology/delille#>;
	a rdfs:Class;
	rdfs:label "commentary"@en, "Kommentar"@de;
	rdfs:comment """Commentary on a citation of a verse of a poem authored by Jacques Delille."""@en;
	rdfs:subClassOf text-expression:Commentary, text-expression:ScientificExpression, publish:TextExpression.

delille:Argument
	rdfs:isDefinedBy <http://www.nie.org/ontology/delille#>;
	a rdfs:Class;
	rdfs:label "argument"@en, "Argument"@de;
	rdfs:comment """Argument of a commentary on a citation of a verse of a poem authored by Jacques Delille."""@en;
	rdfs:subClassOf literature:Argument, publish:TextExpression.

delille:Non-Artist-ManOfLetters-Vulgarizer
	rdfs:isDefinedBy <http://www.nie.org/ontology/delille#>;
	a rdfs:Class;
	rdfs:label "non-artist-man of letters-vulgarizer"@en, "Non-KünstlerIn-Literat-VulgarisatorIn"@de;
	rdfs:comment """Role of a person which is not an artist, a man of letters, and/or a vulgarizer."""@en;
	rdfs:subClassOf human:PersonRole;
	owl:disjointWith human:Artist, text-expression:ManOfLetters, text-expression:Vulgarizer.

# image

#
# PROPERTIES
#
