@prefix rdfs: <http://www.w3.org/2000/01/rdf-schema#>.
@prefix owl: <http://www.w3.org/2002/07/owl#>.
@prefix xsd: <http://www.w3.org/2001/XMLSchema#>.
@prefix dct: <http://purl.org/dc/terms/>.
@prefix skos: <http://www.w3.org/2004/02/skos/core#>.
@prefix physical: <http://www.nie.org/ontology/shared/physical-entity#>.
@prefix event: <http://www.nie.org/ontology/shared/event#>.
@prefix human: <http://www.nie.org/ontology/shared/human#>.
@prefix creating: <http://www.nie.org/ontology/shared/creating#>.
@prefix concept: <http://www.nie.org/ontology/shared/concept#>.
@prefix language: <http://www.nie.org/ontology/shared/language#>.
@prefix document: <http://www.nie.org/ontology/shared/document#>.
@prefix text: <http://www.nie.org/ontology/shared/text#>.
@prefix text-expression: <http://www.nie.org/ontology/shared/text-expression#>.
@prefix text-structure: <http://www.nie.org/ontology/shared/text-structure#>.
@prefix prosodic-structure: <http://www.nie.org/ontology/shared/prosodic-structure#>.
@prefix textedit: <http://www.nie.org/ontology/shared/text-editing#>.
@prefix scholarly-editing: <http://www.nie.org/ontology/shared/scholarly-editing#>.
@prefix infocar: <http://www.nie.org/ontology/shared/information-carrier#>.
@prefix image: <http://www.nie.org/ontology/shared/image#>.
@prefix litera: <http://www.nie.org/ontology/shared/literature#>.
@prefix publish: <http://www.nie.org/ontology/shared/publishing#>.
@prefix letter-corresponding: <http://www.nie.org/ontology/shared/letter-corresponding#>.

# @base <http://www.nie.org/ontology/004D/kuno-raeber>.
@prefix kuno-raeber: <http://www.nie.org/ontology/004D/kuno-raeber#>.

<http://www.nie.org/ontology/004D/kuno-raeber>
	a owl:Ontology;
	dct:license <http://creativecommons.org/licenses/by/3.0/>;
	dct:title "An ontology about the lyric of Kuno Raeber"@en;
	dct:description """Formal description of elements in the online publication of the lyric work of the Swiss poet Kuno Raeber."""@en;
	dct:creator "Hans Cools, MD, knowledge engineer, ontologist, software developer, NIE-INE, Basel University, Switzerland"@en.

#
# CLASSES
#

kuno-raeber:Work
	a rdfs:Class;
	rdfs:label "Kuno Raeber work"@en, "Werk Kuno Raebers"@de;
	rdfs:comment """Work by Kuno Raeber."""@en;
	rdfs:subClassOf concept:IndividualWork.

kuno-raeber:Text
	a rdfs:Class;
	rdfs:label "Kuno Raeber text expression"@en, "Textexpression Kuno Raebers"@de;
	rdfs:comment """Text expression authored by Kuno Raeber."""@en;
	rdfs:subClassOf text-expression:IndividualExpression, [
		a owl:Restriction; owl:onProperty text:hasAlias; owl:minCardinality "0"^^xsd:nonNegativeInteger], [
		a owl:Restriction; owl:onProperty text:hasDetailDescription; owl:minCardinality "0"^^xsd:nonNegativeInteger], [
		a owl:Restriction; owl:onProperty text:hasSpecialDescription; owl:minCardinality "0"^^xsd:nonNegativeInteger], [
		a owl:Restriction; owl:onProperty kuno-raeber:isFinalVersion; owl:maxCardinality "1"^^xsd:nonNegativeInteger], [
		a owl:Restriction; owl:onProperty kuno-raeber:isInSwissGerman; owl:maxCardinality "1"^^xsd:nonNegativeInteger], [
		a owl:Restriction; owl:onProperty kuno-raeber:isPartOfCycle; owl:maxCardinality "1"^^xsd:nonNegativeInteger].
	# seqnum

kuno-raeber:PublicationTextPart
	a rdfs:Class;
	rdfs:label "Kuno Raeber publication text expression part"@en, "Publikation-Textexpressionsteil Kuno Raebers"@de;
	rdfs:comment """Part of a publication text expression authored by Kuno Raeber."""@en;
	rdfs:subClassOf text-expression:ExpressionPart, publish:Expression, [
		a owl:Restriction; owl:onProperty text:hasAlias; owl:minCardinality "0"^^xsd:nonNegativeInteger], [
		a owl:Restriction; owl:onProperty text:hasSpecialDescription; owl:minCardinality "0"^^xsd:nonNegativeInteger].

kuno-raeber:TypewrittenCommentary
	a rdfs:Class;
	rdfs:label "Kuno Raeber typewritten commentary"@en, "maschinengeschriebener Kommentar Kuno Raebers"@de;
	rdfs:comment """Typewritten commentary authored by Kuno Raeber."""@en;
	rdfs:subClassOf text-expression:Commentary, text:TypewrittenText, text:Nonfiction, kuno-raeber:Text.

kuno-raeber:Preface
	a rdfs:Class;
	rdfs:label "Kuno Raeber preface"@en, "Vorwort Kuno Raebers"@de;
	rdfs:comment """Preface authored by Kuno Raeber."""@en;
	rdfs:subClassOf litera:Preface, text:Nonfiction, kuno-raeber:Text.

kuno-raeber:DraftHandwrittenPreface
	a rdfs:Class;
	rdfs:label "Kuno Raeber handwritten preface draft"@en, "handgeschriebener Vorwort-Entwurf Kuno Raebers"@de;
	rdfs:comment """Draft handwritten preface authored by Kuno Raeber."""@en;
	rdfs:subClassOf kuno-raeber:Preface, text:HandwrittenText, text-expression:Draft.

kuno-raeber:TypewrittenPreface
	a rdfs:Class;
	rdfs:label "Kuno Raeber typewritten preface"@en, "maschinengeschriebener Vorwort Kuno Raebers"@de;
	rdfs:comment """Typewritten preface authored by Kuno Raeber."""@en;
	rdfs:subClassOf kuno-raeber:Preface, text:TypewrittenText.

kuno-raeber:PublicationPreface
	a rdfs:Class;
	rdfs:label "Kuno Raeber publication preface"@en, "Publikationsvorwort Kuno Raebers"@de;
	rdfs:comment """Publication preface authored by Kuno Raeber."""@en;
	rdfs:subClassOf kuno-raeber:Preface, publish:Expression.

kuno-raeber:Postface
	a rdfs:Class;
	rdfs:label "Kuno Raeber postface"@en, "Nachwort Kuno Raebers"@de;
	rdfs:comment """Postface authored by Kuno Raeber."""@en;
	rdfs:subClassOf litera:Postface, text:Nonfiction, kuno-raeber:Text.

kuno-raeber:TypewrittenPostface
	a rdfs:Class;
	rdfs:label "Kuno Raeber typewritten postface"@en, "maschinengeschriebener Nachwort Kuno Raebers"@de;
	rdfs:comment """Typewritten postface authored by Kuno Raeber."""@en;
	rdfs:subClassOf kuno-raeber:Postface, text:TypewrittenText.

kuno-raeber:PublicationMotto
	a rdfs:Class;
	rdfs:label "publication motto"@en, "Publikation-Motto"@de;
	rdfs:comment """Publication motto authored by Kuno Raeber."""@en;
	rdfs:subClassOf litera:Motto, publish:Expression, kuno-raeber:Text.

kuno-raeber:Poem
	a rdfs:Class;
	rdfs:label "Kuno Raeber poem"@en, "Gedicht Kuno Raebers"@de;
	rdfs:comment """Poem authored by Kuno Raeber."""@en;
	rdfs:subClassOf litera:Poem, kuno-raeber:Text, [
		a owl:Restriction; owl:onProperty kuno-raeber:poemHasTitle; owl:minCardinality "0"^^xsd:nonNegativeInteger], [
		a owl:Restriction; owl:onProperty kuno-raeber:hasSameEditionAsIn; owl:minCardinality "0"^^xsd:nonNegativeInteger], [
		a owl:Restriction; owl:onProperty kuno-raeber:hasReferencePoem; owl:minCardinality "0"^^xsd:nonNegativeInteger], [
		a owl:Restriction; owl:onProperty kuno-raeber:hasReferenceTitle; owl:minCardinality "0"^^xsd:nonNegativeInteger], [
		a owl:Restriction; owl:onProperty kuno-raeber:hasStrophe; owl:minCardinality "0"^^xsd:nonNegativeInteger].

kuno-raeber:ScholarlyEdition
	a rdfs:Class;
	rdfs:label "scholarly Kuno Raeber text edition"@en, "wissenschaftliche Edition eines Kuno Raeber Textes"@de;
	rdfs:comment """Scholarly edition of a text authored by Kuno Raeber."""@en, """Wissenschaftliche Edition eines von Kuno Raeber verfassten Texts."""@de;
	rdfs:subClassOf scholarly-editing:Edition, [
		a owl:Restriction; owl:onProperty language:hasContent; owl:minCardinality "0"^^xsd:nonNegativeInteger], [
		a owl:Restriction; owl:onProperty kuno-raeber:hasPageIndicator; owl:minCardinality "0"^^xsd:nonNegativeInteger], [
		a owl:Restriction; owl:onProperty kuno-raeber:hasPageNumberIndicator; owl:minCardinality "0"^^xsd:nonNegativeInteger], [
		a owl:Restriction; owl:onProperty kuno-raeber:hasColumnIndicator; owl:minCardinality "0"^^xsd:nonNegativeInteger].

kuno-raeber:DiplomaticTranscription
	a rdfs:Class;
	rdfs:label "Kuno Raeber text diplomatic transcription"@en, "diplomatische Umschrift eines Kuno Raeber Textes"@de;
	rdfs:comment """Diplomatic transcription of a text authored by Kuno Raeber."""@en, """Diplomatische Umschrift eines von Kuno Raeber verfassten Texts."""@de;
	rdfs:subClassOf scholarly-editing:DiplomaticTranscription, [
		a owl:Restriction; owl:onProperty language:hasContent; owl:minCardinality "0"^^xsd:nonNegativeInteger]. # needed due to restriction in dhl-knora
	# seqnum

kuno-raeber:HandwrittenPoem
	a rdfs:Class;
	rdfs:label "Kuno Raeber handwritten poem"@en, "handgeschriebenes Gedicht Kuno Raebers"@de;
	rdfs:comment """Handwritten poem authored by Kuno Raeber."""@en, """Handgeschriebenes Gedicht Kuno Raebers."""@de;
	rdfs:subClassOf kuno-raeber:Poem, text:HandwrittenText, [
		a owl:Restriction; owl:onProperty kuno-raeber:isOnPage; owl:minCardinality "0"^^xsd:nonNegativeInteger].

kuno-raeber:PoemNote
	a rdfs:Class;
	rdfs:label "Kuno Raeber poem note"@en, "Gedichtnotiz Kuno Raebers"@de;
	rdfs:comment """Poem note authored by Kuno Raeber."""@en, """Gedichtnotiz Kuno Raebers."""@de;
	rdfs:subClassOf kuno-raeber:HandwrittenPoem, creating:FirstVersion, [
		a owl:Restriction; owl:onProperty kuno-raeber:isInNotebook; owl:minCardinality "0"^^xsd:nonNegativeInteger], [.

kuno-raeber:PostcardPoem
	a rdfs:Class;
	rdfs:label "Kuno Raeber postcard poem"@en, "Postkarten-Gedicht Kuno Raebers"@de;
	rdfs:comment """Postcard poem authored by Kuno Raeber."""@en, """Postkarten-Gedicht Kuno Raebers."""@de;
	rdfs:subClassOf kuno-raeber:HandwrittenPoem, [
		a owl:Restriction; owl:onProperty kuno-raeber:isOnPostcard; owl:minCardinality "0"^^xsd:nonNegativeInteger], [
		a owl:Restriction; owl:onProperty publish:hasNachlassPublicationDescription; owl:minCardinality "0"^^xsd:nonNegativeInteger].

kuno-raeber:TypewrittenPoem
	a rdfs:Class;
	rdfs:label "Kuno Raeber typewritten poem"@en, "maschinengeschriebenes Gedicht Kuno Raebers"@de;
	rdfs:comment """Typewritten poem authored by Kuno Raeber."""@en, """Maschinengeschriebenes Gedicht Kuno Raebers."""@de;
	rdfs:subClassOf kuno-raeber:Poem, text:TypewrittenText.

kuno-raeber:PublicationPoem
	a rdfs:Class;
	rdfs:label "Kuno Raeber publication poem"@en, "Publikation-Gedicht Kuno Raebers"@de;
	rdfs:comment """Poem authored by Kuno Raeber, as published."""@en, """Gedicht Kuno Raebers wie publiziert."""@de;
	rdfs:subClassOf kuno-raeber:Poem, publish:Expression, [
		a owl:Restriction; owl:onProperty kuno-raeber:isInPolyAuthorPublicationConvolute; owl:minCardinality "0"^^xsd:nonNegativeInteger].

kuno-raeber:DiaryEntry
	a rdfs:Class;
	rdfs:label "Kuno Raeber diary entry"@en, "Tagebucheintrag Kuno Raebers"@de;
	rdfs:comment """Diary entry authored by Kuno Raeber."""@en;
	rdfs:subClassOf text-expression:DiaryEntry, kuno-raeber:Text, [
		a owl:Restriction; owl:onProperty kuno-raeber:isInDiary; owl:minCardinality "0"^^xsd:nonNegativeInteger], [
		a owl:Restriction; owl:onProperty kuno-raeber:isInDiaryConvolute; owl:minCardinality "0"^^xsd:nonNegativeInteger].

kuno-raeber:DraftLetterExpression
	a rdfs:Class;
	rdfs:label "Kuno Raeber draft letter expression"@en,"Briefentwurf-Expression Kuno Raebers"@de;
	rdfs:comment """Draft letter expression authored by Kuno Raeber."""@en;
	rdfs:subClassOf text:HandwrittenText, kuno-raeber:Text, text-expression:Draft. # infocar:ArchiveElement.

kuno-raeber:LetterExpression
	a rdfs:Class;
	rdfs:label "Kuno Raeber letter expression"@en, "Brief-Expression Kuno Raebers"@de;
	rdfs:comment """Letter expression written by Kuno Raeber."""@en;
	rdfs:subClassOf letter-corresponding:Expression, text:WrittenText, kuno-raeber:Text, [
		a owl:Restriction; owl:onProperty text:hasSpecialDescription; owl:minCardinality "0"^^xsd:nonNegativeInteger].

kuno-raeber:StillImageRepresentation
	a rdfs:Class;
	rdfs:label "still image representation"@en, "Foto-Repräsentation"@de;
	rdfs:comment """Directory containing still images."""@en;
	skos:note """DHL knora application-specific entity."""@en;
	rdfs:subClassOf knora-base:StillImageRepresentation.

kuno-raeber:Page
	a rdfs:Class;
	rdfs:label "Kuno Raeber page"@en, "Seite Kuno Raebers"@de;
	rdfs:comment """Page with a handwritten poem by Kuno Raeber."""@en, """Seite mit einem handgeschriebenen Gedicht Kuno Raebers."""@de;
	rdfs:subClassOf infocar:Page, [
		a owl:Restriction; owl:onProperty knora-base:hasRepresentation; owl:minCardinality "0"^^xsd:nonNegativeInteger].

kuno-raeber:Convolute
	a rdfs:Class;
	rdfs:label "Kuno Raeber convolute"@en, "Konvolut Kuno Raebers"@de;
	rdfs:comment """Convolute of which the elements are authored by Kuno Raeber."""@en;
	rdfs:subClassOf infocar:Convolute, [
		a owl:Restriction; owl:onProperty text:hasComment; owl:minCardinality "0"^^xsd:nonNegativeInteger].

kuno-raeber:ConvoluteElement
	a rdfs:Class;
	rdfs:label "Kuno Raeber convolute element"@en, "Element eines Kuno Raeber-Konvoluts"@de;
	rdfs:comment """Element of a Kuno Raeber convolute."""@en;
	rdfs:subClassOf infocar:ConvoluteElement, [
		a owl:Restriction; owl:onProperty kuno-raeber:isPartOfConvolute; owl:minCardinality "0"^^xsd:nonNegativeInteger].

kuno-raeber:PoemNotebook
	a rdfs:Class;
	rdfs:label "Kuno Raeber poem notebook"@en, "Gedichten-Notizbuch Kuno Raebers"@de;
	rdfs:comment """Notebook with poem notes authored by Kuno Raeber."""@en;
	rdfs:subClassOf infocar:Manuscript, infocar:Notebook, kuno-raeber:Convolute, infocar:ArchiveElement, [
		a owl:Restriction; owl:onProperty knora-base:hasRepresentation; owl:minCardinality "0"^^xsd:nonNegativeInteger], [
		a owl:Restriction; owl:onProperty knora-base:hasRepresentationValue; owl:minCardinality "0"^^xsd:nonNegativeInteger], [
		a owl:Restriction; owl:onProperty kuno-raeber:containsEarlierStagesOfManuscriptConvolute; owl:minCardinality "0"^^xsd:nonNegativeInteger], [
		a owl:Restriction; owl:onProperty kuno-raeber:containsEarlierStagesOfTypescriptConvolute; owl:minCardinality "0"^^xsd:nonNegativeInteger].

kuno-raeber:Manuscript
	a rdfs:Class;
	rdfs:label "Kuno Raeber manuscript"@en, "Manuskript Kuno Raebers"@de;
	rdfs:comment """Manuscript authored by Kuno Raeber."""@en;
	rdfs:subClassOf infocar:Leaf, infocar:Manuscript, kuno-raeber:ConvoluteElement, infocar:ArchiveElement, [
		a owl:Restriction; owl:onProperty kuno-raeber:isPartOfManuscriptConvolute; owl:minCardinality "0"^^xsd:nonNegativeInteger].

kuno-raeber:PoemManuscript
	a rdfs:Class;
	rdfs:label "Kuno Raeber poem manuscript"@en, "Gedichtmanuskript Kuno Raebers"@de;
	rdfs:comment """Manuscript with a poem authored by Kuno Raeber."""@en;
	rdfs:subClassOf kuno-raeber:Manuscript.

kuno-raeber:ManuscriptConvolute
	a rdfs:Class;
	rdfs:label "Kuno Raeber manuscript convolute"@en, "Manuskriptenkonvolut Kuno Raebers"@de;
	rdfs:comment """Convolute with manuscripts authored by Kuno Raeber."""@en;
	rdfs:subClassOf kuno-raeber:Convolute, infocar:ArchiveElement, [
		a owl:Restriction; owl:onProperty kuno-raeber:containsLaterStagesOfNotebook; owl:minCardinality "0"^^xsd:nonNegativeInteger], [
		a owl:Restriction; owl:onProperty kuno-raeber:containsEarlierStagesOfTypescriptConvolute; owl:minCardinality "0"^^xsd:nonNegativeInteger].

kuno-raeber:PoemPostcard
	a rdfs:Class;
	rdfs:label "Kuno Raeber poem postcard"@en, "Gedicht-Postkarte Kuno Raebers"@de;
	rdfs:comment """Postcard with a poem authored by Kuno Raeber."""@en;
	rdfs:subClassOf infocar:Manuscript, infocar:Postcard, infocar:ArchiveElement, infocar:ConvoluteElement, [
		a owl:Restriction; owl:onProperty kuno-raeber:isPartOfPostcardConvolute; owl:minCardinality "0"^^xsd:nonNegativeInteger], [
		a owl:Restriction; owl:onProperty knora-base:hasRepresentation; owl:minCardinality "0"^^xsd:nonNegativeInteger].

kuno-raeber:PoemPostcardConvolute
	a rdfs:Class;
	rdfs:label "Kuno Raeber poem postcard convolute"@en, "Gedicht-Postkartenkonvolut Kuno Raebers"@de;
	rdfs:comment """Poem postcard convolute with poems authored by Kuno Raeber."""@en;
	rdfs:subClassOf kuno-raeber:Convolute, [
		a owl:Restriction; owl:onProperty knora-base:hasRepresentation; owl:minCardinality "0"^^xsd:nonNegativeInteger], [
		a owl:Restriction; owl:onProperty kuno-raeber:containsLaterStagesOfNotebook; owl:minCardinality "0"^^xsd:nonNegativeInteger].

kuno-raeber:Typescript
	a rdfs:Class;
	rdfs:label "Kuno Raeber typescript"@en, "Typoskript Kuno Raebers"@de;
	rdfs:comment """Typescript by Kuno Raeber."""@en;
	rdfs:subClassOf infocar:Leaf, infocar:Typescript, kuno-raeber:ConvoluteElement, infocar:ArchiveElement, [
		a owl:Restriction; owl:onProperty kuno-raeber:isPartOfTypescriptConvolute; owl:minCardinality "0"^^xsd:nonNegativeInteger].

kuno-raeber:PoemTypescript
	a rdfs:Class;
	rdfs:label "Kuno Raeber poem typescript"@en, "Gedichttyposkript Kuno Raebers"@de;
	rdfs:comment """Poem typescript by Kuno Raeber."""@en;
	rdfs:subClassOf kuno-raeber:Typescript.

kuno-raeber:TypescriptConvolute
	a rdfs:Class;
	rdfs:label "Kuno Raeber typescript convolute"@en, "Typoskriptenconvolut Kuno Raebers"@de;
	rdfs:comment """Convolute with typescripts authored by Kuno Raeber."""@en;
	rdfs:subClassOf kuno-raeber:Convolute, infocar:ArchiveElement, [
		a owl:Restriction; owl:onProperty kuno-raeber:containsLaterStagesOfNotebook; owl:minCardinality "0"^^xsd:nonNegativeInteger], [
		a owl:Restriction; owl:onProperty kuno-raeber:containsLaterStagesOfManuscriptConvolute; owl:minCardinality "0"^^xsd:nonNegativeInteger].

kuno-raeber:TypescriptConvoluteWithImage
	a rdfs:Class;
	rdfs:label "Kuno Raeber typescript convolute with image"@en, "Typoskriptenconvolut Kuno Raebers mit Bild"@de;
	rdfs:comment """Typescript convolute with poems authored by Kuno Raeber, mit bild."""@en;
	rdfs:subClassOf kuno-raeber:TypescriptConvolute, [
		a owl:Restriction; owl:onProperty knora-base:hasRepresentation; owl:minCardinality "0"^^xsd:nonNegativeInteger].

kuno-raeber:PrintedPoemBookPublication
	a rdfs:Class;
	rdfs:label "Kuno Raeber printed poem book publication"@en, "gedruckte Gedichtenbuchausgabe Kuno Raebers"@de;
	rdfs:comment """Printed publication of a book  with poems authored by Kuno Raeber."""@en;
	rdfs:subClassOf infocar:Book, publish:PrintedPublication, kuno-raeber:Convolute, [
		a owl:Restriction; owl:onProperty knora-base:hasRepresentation; owl:minCardinality "0"^^xsd:nonNegativeInteger], [
		a owl:Restriction; owl:onProperty kuno-raeber:containsLaterStagesOfNotebook; owl:minCardinality "0"^^xsd:nonNegativeInteger], [
		a owl:Restriction; owl:onProperty kuno-raeber:containsLaterStagesOfManuscriptConvolute; owl:minCardinality "0"^^xsd:nonNegativeInteger], [
		a owl:Restriction; owl:onProperty kuno-raeber:containsLaterStagesOfTypescriptConvolute; owl:minCardinality "0"^^xsd:nonNegativeInteger].

kuno-raeber:PolyAuthorPublication
	a rdfs:Class;
	rdfs:label "Kuno Raeber poly-author publication"@en, "Mehrautorenpublikationen Kuno Raebers"@de;
	rdfs:comment """Publication with a poem authored by Kuno Raeber among expressions by other authors."""@en;
	rdfs:subClassOf publish:PolyAuthorPublication, infocar:ArchiveElement, [
		a owl:Restriction; owl:onProperty kuno-raeber:hasContentPartInPolyAuthorPublicationConvolute; owl:minCardinality "0"^^xsd:nonNegativeInteger].

kuno-raeber:PolyAuthorPublicationConvolute
	a rdfs:Class;
	rdfs:label "Kuno Raeber poly-author publication convolute"@en, "Mehrautorenpublikationen-Konvolut Kuno Raebers"@de;
	rdfs:comment """Convolute of poems authored by Kuno Raeber as published among expressions by other authors."""@en;
	rdfs:subClassOf kuno-raeber:Convolute.

kuno-raeber:Diary
	a rdfs:Class;
	rdfs:label "Kuno Raeber diary"@en,"Tagebuch Kuno Raebers"@de;
	rdfs:comment """Diary with entries authored by Kuno Raeber."""@en;
	skos:note """Different from kuno-raeber:DiaryConvolute - in contrast to kuno-raeber:PoemNotebook - because only selections from different diaries are published online."""@en;
	rdfs:subClassOf infocar:Diary, infocar:Manuscript, infocar:Book, infocar:ArchiveElement.

kuno-raeber:DiaryConvolute
	a rdfs:Class;
	rdfs:label "Kuno Raeber diary convolute"@en,"Tagebuch-Konvolut Kuno Raebers"@de;
	rdfs:comment """Convolute of diaries with entries authored by Kuno Raeber."""@en;
	rdfs:subClassOf kuno-raeber:Convolute, infocar:ArchiveElement.

kuno-raeber:Letter
	a rdfs:Class;
	rdfs:label "Kuno Raeber letter"@en,"Brief Kuno Raebers"@de;
	rdfs:comment """Letter written by or to Kuno Raeber."""@en;
	rdfs:subClassOf letter-corresponding:Letter, infocar:ArchiveElement, [
		a owl:Restriction; owl:onProperty kuno-raeber:isPartOfLetterConvolute; owl:minCardinality "0"^^xsd:nonNegativeInteger].

kuno-raeber:LetterConvolute
	a rdfs:Class;
	rdfs:label "Kuno Raeber letter convolute"@en,"Briefekonvolut Kuno Raebers"@de;
	rdfs:comment """Convolute of letters written by and to Kuno Raeber."""@en;
	rdfs:subClassOf kuno-raeber:Convolute, infocar:ArchiveElement.

kuno-raeber:NachlassPublication
	a rdfs:Class;
	rdfs:label "Kuno Raeber nachlass publication"@en, "Nachlass-Publication Kuno Raebers"@de;
	rdfs:comment """Publication of a Nachlass of Kuno Raeber."""@en;
	rdfs:subClassOf publish:NachlassPublication, infocar:Volume, publish:PrintedPublication.

#
# PROPERTIES
#

kuno-raeber:poemHasTitle
	a owl:ObjectProperty;
	rdfs:label "poem has title"@en, "Gedicht hat Titel"@de;
	rdfs:comment """Relating a poem by Kuno Raeber to a title it has."""@en;
	rdfs:domain kuno-raeber:Poem;
	rdfs:range knora-base:TextValue;
	rdfs:subPropertyOf text-expression:hasTitle;
	knora-base:subjectClassConstraint kuno-raeber:Poem;
	knora-base:objectClassConstraint knora-base:TextValue.

kuno-raeber:hasPageIndicator
	a owl:ObjectProperty;
	rdfs:label "has page indicator"@en, "hat Seite-Indikator"@de;
	rdfs:comment """Relating a scholarly edition of an expression by by Kuno Raeber to an editorial symbol indicating where a page starts."""@en;
	rdfs:domain kuno-raeber:ScholarlyEdition;
#	rdfs:range rdfs:Literal;
	rdfs:subPropertyOf knora-base:hasValue;
	knora-base:subjectClassConstraint kuno-raeber:ScholarlyEdition;
	knora-base:objectClassConstraint knora-base:TextValue.

kuno-raeber:hasPageNumberIndicator
	a owl:ObjectProperty;
	rdfs:label "has page number indicator"@en, "hat Seitennummer-Indikator"@de;
	rdfs:comment """Relating a scholarly edition of an expression by Kuno Raeber to an editorial symbol indicating the number of a page."""@en;
	rdfs:domain kuno-raeber:ScholarlyEdition;
#	rdfs:range rdfs:Literal;
	rdfs:subPropertyOf knora-base:hasValue;
	knora-base:subjectClassConstraint kuno-raeber:ScholarlyEdition;
	knora-base:objectClassConstraint knora-base:TextValue.

kuno-raeber:hasColumnIndicator
	a owl:ObjectProperty;
	rdfs:label "has column indicator"@en, "hat Spalte-Indikator"@de;
	rdfs:comment """Relating a scholarly edition of an expression by Kuno Raeber to an editorial symbol indicating where on a page a column starts."""@en;
	rdfs:domain kuno-raeber:ScholarlyEdition;
#	rdfs:range rdfs:Literal;
	rdfs:subPropertyOf knora-base:hasValue;
	knora-base:subjectClassConstraint kuno-raeber:ScholarlyEdition;
	knora-base:objectClassConstraint knora-base:TextValue.

kuno-raeber:isOnPage # to be removed when knora-base:hasRepresentation will be implemented in Knora
	a owl:ObjectProperty;
	rdfs:label "is on page"@en, "ist auf Seite"@de;
	rdfs:comment """Relating a handwritten poem by Kuno Raeber to a carrier page it is on."""@en;
	rdfs:domain kuno-raeber:HandwrittenPoem;
	rdfs:range kuno-raeber:Page;
	rdfs:subPropertyOf infocar:isTextOnPage;
	knora-base:subjectClassConstraint kuno-raeber:HandwrittenPoem;
	knora-base:objectClassConstraint kuno-raeber:Page.

kuno-raeber:isOnPageValue # to be removed when knora-base:hasRepresentation will be implemented in Knora
	a owl:ObjectProperty;
	rdfs:label "is on page - statement"@en, "ist auf Seite - Festlegung"@de;
	rdfs:comment """Relating a handwritten poem by Kuno Raeber to a reification statement of the relation between the poem and a carrier page it is on."""@en;
	rdfs:subPropertyOf infocar:isTextOnPageValue;
	knora-base:subjectClassConstraint kuno-raeber:HandwrittenPoem;
	knora-base:objectClassConstraint knora-base:LinkValue.

kuno-raeber:isInNotebook
	a owl:ObjectProperty;
	rdfs:label "is in notebook"@en, "ist in Notizbuch"@de;
	rdfs:comment """Relating a poem note by Kuno Raeber to a notebook it is in."""@en;
	rdfs:domain kuno-raeber:PoemNote;
	rdfs:range kuno-raeber:PoemNotebook;
	rdfs:subPropertyOf infocar:isInManuscript;
	knora-base:subjectClassConstraint kuno-raeber:PoemNote;
	knora-base:objectClassConstraint kuno-raeber:PoemNotebook.

kuno-raeber:isInNotebookValue
	a owl:ObjectProperty;
	rdfs:label "is in notebook - statement"@en, "ist in Notizbuch - Festlegung"@de;
	rdfs:comment """Relating a poem note by Kuno Raeber to a reification statement of the relation between the poem note and a notebook it is in."""@en;
	rdfs:subPropertyOf infocar:isInManuscriptValue;
	knora-base:subjectClassConstraint kuno-raeber:PoemNote;
	knora-base:objectClassConstraint knora-base:LinkValue.

kuno-raeber:isOnPostcard
	a owl:ObjectProperty;
	rdfs:label "is on postcard"@en, "ist auf Postkarte"@de;
	rdfs:comment """Relating a poem by Kuno Raeber to a postcard it is on."""@en;
	rdfs:domain kuno-raeber:PostcardPoem;
	rdfs:range kuno-raeber:PoemPostcard;
	rdfs:subPropertyOf infocar:isInManuscript;
	knora-base:subjectClassConstraint kuno-raeber:PostcardPoem;
	knora-base:objectClassConstraint kuno-raeber:PoemPostcard.

kuno-raeber:isOnPostcardValue
	a owl:ObjectProperty;
	rdfs:label "is on postcard - statement"@en, "ist auf Postkarte - Festlegung"@de;
	rdfs:comment """Relating a poem by Kuno Raeber to a reification statement of the relation between the poem and a postcard it is on."""@en;
	rdfs:subPropertyOf infocar:isInManuscriptValue;
	knora-base:subjectClassConstraint kuno-raeber:PostcardPoem;
	knora-base:objectClassConstraint knora-base:LinkValue.

kuno-raeber:isInPolyAuthorPublicationConvolute
	a owl:ObjectProperty;
	rdfs:label "is in poly-author publication convolute"@en, "ist in Mehrautorenpublikationen-Konvolut"@de;
	rdfs:comment """Relating a publication poem by Kuno Raeber to a poly-author publication it is in."""@en;
	rdfs:domain kuno-raeber:PublicationPoem;
	rdfs:range kuno-raeber:PolyAuthorPublicationConvolute;
	rdfs:subPropertyOf knora-base:hasLinkTo;
	knora-base:subjectClassConstraint kuno-raeber:PublicationPoem;
	knora-base:objectClassConstraint kuno-raeber:PolyAuthorPublicationConvolute.

kuno-raeber:isInPolyAuthorPublicationConvoluteValue
	a owl:ObjectProperty;
	rdfs:label "is in poly-author publication convolute - statement"@en, "ist in Mehrautorenpublikationen-Konvolut - Festlegung"@de;
	rdfs:comment """Relating a publication poem by Kuno Raeber to a reification statement of the relation between the poem and a poly-author publication it is in."""@en;
	rdfs:subPropertyOf knora-base:hasLinkToValue;
	knora-base:subjectClassConstraint kuno-raeber:PublicationPoem;
	knora-base:objectClassConstraint knora-base:LinkValue.

kuno-raeber:isPartOfManuscriptConvolute
	a owl:ObjectProperty;
	rdfs:label "is part of manuscript convolute"@en, "ist Teil eines Manuskriptenkonvoluts"@de;
	rdfs:comment """Relating a manuscript by Kuno Raeber to the convolute it is part of."""@en;
	rdfs:domain kuno-raeber:Manuscript;
	rdfs:range kuno-raeber:ManuscriptConvolute;
	rdfs:subPropertyOf infocar:isPartOfConvolute;
	knora-base:subjectClassConstraint kuno-raeber:Manuscript;
	knora-base:objectClassConstraint kuno-raeber:ManuscriptConvolute.

kuno-raeber:isPartOfManuscriptConvoluteValue
	a owl:ObjectProperty;
	rdfs:label "is part of manuscript convolute - statement"@en, "ist Teil eines Manuskriptenkonvoluts - Festlegung"@de;
	rdfs:comment """Relating a manuscript by Kuno Raeber to a reification statement of the relation between the manuscript and the convolute it is part of."""@en;
	rdfs:subPropertyOf infocar:isPartOfConvoluteValue;
	knora-base:subjectClassConstraint kuno-raeber:Manuscript;
	knora-base:objectClassConstraint knora-base:LinkValue.

kuno-raeber:isPartOfPostcardConvolute
	a owl:ObjectProperty;
	rdfs:label "is part of postcard convolute"@en, "ist Teil von Postkartekonvolut"@de;
	rdfs:comment """Relating a poem postcard by Kuno Raeber to the convolute it is part of."""@en;
	rdfs:domain kuno-raeber:PoemPostcard;
	rdfs:range kuno-raeber:PoemPostcardConvolute;
	rdfs:subPropertyOf infocar:isPartOfConvolute;
	knora-base:subjectClassConstraint kuno-raeber:PoemPostcard;
	knora-base:objectClassConstraint kuno-raeber:PoemPostcardConvolute.

kuno-raeber:isPartOfPostcardConvoluteValue
	a owl:ObjectProperty;
	rdfs:label "is part of postcard convolute - statement"@en, "ist Teil von Postkartekonvolut - Festlegung"@de;
	rdfs:comment """Relating a poem postcard by Kuno Raeber to a reification statement of the relation between the poem postcard and the convolute it is part of."""@en;
	rdfs:subPropertyOf infocar:isPartOfConvoluteValue;
	knora-base:subjectClassConstraint kuno-raeber:PoemPostcard;
	knora-base:objectClassConstraint knora-base:LinkValue.
		
kuno-raeber:isPartOfTypescriptConvolute
	a owl:ObjectProperty;
	rdfs:label "is part of typescript convolute"@en, "ist Teil eines Typoskriptenkonvoluts"@de;
	rdfs:comment """Relating a typescript by Kuno Raeber to the convolute it is part of."""@en;
	rdfs:domain kuno-raeber:Typescript;
	rdfs:range kuno-raeber:TypescriptConvolute;
	rdfs:subPropertyOf infocar:isPartOfConvolute;
	knora-base:subjectClassConstraint kuno-raeber:Typescript;
	knora-base:objectClassConstraint kuno-raeber:TypescriptConvolute.

kuno-raeber:isPartOfTypescriptConvoluteValue
	a owl:ObjectProperty;
	rdfs:label "is part of typescript convolute - statement"@en, "ist Teil eines Typoskriptenkonvoluts - Festlegung"@de;
	rdfs:comment """Relating a typescript by Kuno Raeber to a reification statement of the relation between the typescript and the convolute it is part of."""@en;
	rdfs:subPropertyOf infocar:isPartOfConvoluteValue;
	knora-base:subjectClassConstraint kuno-raeber:Typescript;
	knora-base:objectClassConstraint knora-base:LinkValue.

kuno-raeber:containsEarlierStagesOfManuscriptConvolute
	a owl:ObjectProperty;
	rdfs:label "contains earlier stages of manuscript convolute"@en, "enthält Vorstufen von Manuskriptenkonvolut"@de;
	rdfs:comment """Relating a convolute to another one containing manuscripts with later stages of poems by Kuno Raeber of the former convolute."""@en;
	rdfs:domain kuno-raeber:PoemNotebook;
	rdfs:range kuno-raeber:ManuscriptConvolute;
	rdfs:subPropertyOf infocar:containsEarlierStagesOf;
	knora-base:subjectClassConstraint kuno-raeber:PoemNotebook;
	knora-base:objectClassConstraint kuno-raeber:ManuscriptConvolute.

kuno-raeber:containsEarlierStagesOfManuscriptConvoluteValue
	a owl:ObjectProperty;
	rdfs:label "contains earlier stages of manuscript convolute - statement"@en, "enthält Vorstufen von Manuskriptenkonvolut - Festlegung"@de;
	rdfs:comment """Relating a convolute to a reification statement of the relation between the convolute and another one containing manuscripts with later stages of poems by Kuno Raeber of the former convolute."""@en;
	rdfs:subPropertyOf infocar:containsEarlierStagesOfValue;
	knora-base:subjectClassConstraint kuno-raeber:PoemNotebook;
	knora-base:objectClassConstraint knora-base:LinkValue.

kuno-raeber:containsEarlierStagesOfTypescriptConvolute
	a owl:ObjectProperty;
	rdfs:label "contains earlier stages of typescript convolute"@en, "enthält Vorstufen von Typoskriptenonvolut"@de;
	rdfs:comment """Relating a convolute to another one containing typescripts with later stages of poems by Kuno Raeber of the former convolute."""@en;
	rdfs:domain kuno-raeber:Convolute;
	rdfs:range kuno-raeber:TypescriptConvolute;
	rdfs:subPropertyOf infocar:containsEarlierStagesOf;
	knora-base:subjectClassConstraint kuno-raeber:Convolute;
	knora-base:objectClassConstraint kuno-raeber:TypescriptConvolute.

kuno-raeber:containsEarlierStagesOfTypescriptConvoluteValue
	a owl:ObjectProperty;
	rdfs:label "contains earlier stages of typescript convolute - statement"@en, "enthält Vorstufen von Typoskriptenonvolut - Festlegung"@de;
	rdfs:comment """Relating a convolute to a reification statement of the relation between the convolute and another one containing typescripts with later stages of poems by Kuno Raeber of the former convolute."""@en;
	rdfs:subPropertyOf infocar:containsEarlierStagesOfValue;
	knora-base:subjectClassConstraint kuno-raeber:Convolute;
	knora-base:objectClassConstraint knora-base:LinkValue.

kuno-raeber:containsLaterStagesOfNotebook
	a owl:ObjectProperty;
	rdfs:label "contains later stages of notebook"@en, "enthält spätere Stufen von Notizbuch"@de;
	rdfs:comment """Relating a convolute to a notebook containing earlier stages of poems by Kuno Raeber of the former convolute."""@en;
	rdfs:domain kuno-raeber:Convolute;
	rdfs:range kuno-raeber:PoemNotebook;
	rdfs:subPropertyOf infocar:containsLaterStagesOf;
	knora-base:subjectClassConstraint kuno-raeber:Convolute;
	knora-base:objectClassConstraint kuno-raeber:PoemNotebook.

kuno-raeber:containsLaterStagesOfNotebookValue
	a owl:ObjectProperty;
	rdfs:label "contains later stages of notebook - statement"@en, "enthält spätere Stufen von Notizbuch - Festlegung"@de;
	rdfs:comment """Relating a convolute to a reification statement of the relation between the convolute and a notebook containing earlier stages of poems by Kuno Raeber of the former convolute."""@en;
	rdfs:subPropertyOf infocar:containsLaterStagesOfValue;
	knora-base:subjectClassConstraint kuno-raeber:Convolute;
	knora-base:objectClassConstraint knora-base:LinkValue.

kuno-raeber:containsLaterStagesOfManuscriptConvolute
	a owl:ObjectProperty;
	rdfs:label "contains later stages of manuscript convolute"@en, "enthält spätere Stufen von Manuskriptenkonvolut"@de;
	rdfs:comment """Relating a convolute to another one containing manuscripts with earlier stages of poems by Kuno Raeber of the former convolute."""@en;
	rdfs:domain kuno-raeber:Convolute;
	rdfs:range kuno-raeber:ManuscriptConvolute;
	rdfs:subPropertyOf infocar:containsLaterStagesOf;
	knora-base:subjectClassConstraint kuno-raeber:Convolute;
	knora-base:objectClassConstraint kuno-raeber:ManuscriptConvolute.

kuno-raeber:containsLaterStagesOfManuscriptConvoluteValue
	a owl:ObjectProperty;
	rdfs:label "contains later stages of manuscript convolute - statement"@en, "enthält spätere Stufen von Manuskriptenkonvolut - Festlegung"@de;
	rdfs:comment """Relating a convolute to a reification statement of the relation between the convolute and another one containing manuscripts with earlier stages of poems by Kuno Raeber of the former convolute."""@en;
	rdfs:subPropertyOf infocar:containsLaterStagesOfValue;
	knora-base:subjectClassConstraint kuno-raeber:Convolute;
	knora-base:objectClassConstraint knora-base:LinkValue.

kuno-raeber:containsLaterStagesOfTypescriptConvolute
	a owl:ObjectProperty;
	rdfs:label "contains later stages of typescript convolute"@en, "enthält spätere Stufen von Typoskriptenonvolut"@de;
	rdfs:comment """Relating a convolute to another one containing typescripts with earlier stages of poems by Kuno Raeber of the former convolute."""@en;
	rdfs:domain kuno-raeber:PrintedPoemBookPublication;
	rdfs:range kuno-raeber:TypescriptConvolute;
	rdfs:subPropertyOf infocar:containsLaterStagesOf;
	knora-base:subjectClassConstraint kuno-raeber:PrintedPoemBookPublication;
	knora-base:objectClassConstraint kuno-raeber:TypescriptConvolute.

kuno-raeber:containsLaterStagesOfTypescriptConvoluteValue
	a owl:ObjectProperty;
	rdfs:label "contains later stages of typescript convolute - statement"@en, "enthält spätere Stufen von Typoskriptenonvolut - Festlegung"@de;
	rdfs:comment """Relating a convolute to a reification statement of the relation between the convolute and another one containing typescripts with earlier stages of poems by Kuno Raeber of the former convolute."""@en;
	rdfs:subPropertyOf infocar:containsLaterStagesOfValue;
	knora-base:subjectClassConstraint kuno-raeber:PrintedPoemBookPublication;
	knora-base:objectClassConstraint knora-base:LinkValue.

kuno-raeber:isInDiary
	a owl:ObjectProperty;
	rdfs:label "entry is in diary"@en, "Eintrag ist in Tagebuch"@de;
	rdfs:comment """Relating a diary entry by Kuno Raeber to the diary it is in."""@en;
	rdfs:domain kuno-raeber:DiaryEntry;
	rdfs:range kuno-raeber:Diary;
	rdfs:subPropertyOf infocar:isEntryInDiary;
	knora-base:subjectClassConstraint kuno-raeber:DiaryEntry;
	knora-base:objectClassConstraint kuno-raeber:Diary.

kuno-raeber:isInDiaryValue
	a owl:ObjectProperty;
	rdfs:label "entry is in diary - statement"@en, "Eintrag ist in Tagebuch - Festlegung"@de;
	rdfs:comment """Relating a diary entry by Kuno Raeber to a reification statement of the relation between the entry and the diary it is in."""@en;
	rdfs:subPropertyOf infocar:isEntryInDiaryValue;
	knora-base:subjectClassConstraint kuno-raeber:DiaryEntry;
	knora-base:objectClassConstraint knora-base:LinkValue.

kuno-raeber:isInDiaryConvolute
	a owl:ObjectProperty;
	rdfs:label "is in diary convolute"@en, "ist in Tagebuch-Konvolut"@de;
	rdfs:comment """Relating a diary entry by Kuno Raeber to a diary convolute it is in."""@en;
	rdfs:domain kuno-raeber:DiaryEntry;
	rdfs:range kuno-raeber:DiaryConvolute;
	rdfs:subPropertyOf knora-base:hasLinkTo;
	knora-base:subjectClassConstraint kuno-raeber:DiaryEntry;
	knora-base:objectClassConstraint kuno-raeber:DiaryConvolute.

kuno-raeber:isInDiaryConvoluteValue
	a owl:ObjectProperty;
	rdfs:label "is in diary convolute - statement"@en, "ist in Tagebuch-Konvolut - Festlegung"@de;
	rdfs:comment """Relating a diary entry by Kuno Raeber to a reification statement of the relation between the diary entry and a diary convolute it is in."""@en;
	rdfs:subPropertyOf knora-base:hasLinkToValue;
	knora-base:subjectClassConstraint kuno-raeber:DiaryEntry;
	knora-base:objectClassConstraint knora-base:LinkValue.

kuno-raeber:isPartOfConvolute
	a owl:ObjectProperty;
	rdfs:label "is part of convolute"@en, "ist Teil eines Konvoluts"@de;
	rdfs:comment """Relating an element of a Kuno Raeber convolute to the convolute."""@en;
	rdfs:domain kuno-raeber:ConvoluteElement;
	rdfs:range kuno-raeber:Convolute;
	rdfs:subPropertyOf infocar:isPartOfConvolute;
	knora-base:subjectClassConstraint kuno-raeber:ConvoluteElement;
	knora-base:objectClassConstraint kuno-raeber:Convolute.

kuno-raeber:isPartOfConvoluteValue
	a owl:ObjectProperty;
	rdfs:label "is part of convolute - statement"@en, "ist Teil eines Konvoluts - Festlegung"@de;
	rdfs:comment """Relating an element of a Kuno Raeber convolute to a reification statement of the relation between the element and the convolute."""@en;
	rdfs:subPropertyOf infocar:isPartOfConvoluteValue;
	knora-base:subjectClassConstraint kuno-raeber:ConvoluteElement;
	knora-base:objectClassConstraint knora-base:LinkValue.

kuno-raeber:isPartOfLetterConvolute
	a owl:ObjectProperty;
	rdfs:label "is part of letter convolute"@en, "ist Teil eines Briefe-Konvolut"@de;
	rdfs:comment """Relating a letter by Kuno Raeber to a convolute it is in."""@en;
	rdfs:domain kuno-raeber:Letter;
	rdfs:range kuno-raeber:LetterConvolute;
	rdfs:subPropertyOf physical:isPartOf;
	knora-base:subjectClassConstraint kuno-raeber:Letter;
	knora-base:objectClassConstraint kuno-raeber:LetterConvolute.

kuno-raeber:isPartOfLetterConvoluteValue
	a owl:ObjectProperty;
	rdfs:label "is part of letter convolute - statement"@en, "ist Teil eines Briefe-Konvolut - Festlegung"@de;
	rdfs:comment """Relating a letter by Kuno Raeber to a reification statement of the relation between the letter and a convolute it is in."""@en;
	rdfs:subPropertyOf physical:isPartOfValue;
	knora-base:subjectClassConstraint kuno-raeber:Letter;
	knora-base:objectClassConstraint knora-base:LinkValue.

kuno-raeber:hasSameEditionAsIn
	a owl:ObjectProperty;
	rdfs:label "has same edition as in"@en, "hat gleiche Edition als in "@de;
	rdfs:comment """Relating a poem by Kuno Raeber to a convolute containing a poem with the same edition."""@en;
	rdfs:domain kuno-raeber:Poem;
	rdfs:range kuno-raeber:Convolute;
	rdfs:subPropertyOf knora-base:hasLinkTo;
	knora-base:subjectClassConstraint kuno-raeber:Poem;
	knora-base:objectClassConstraint kuno-raeber:Convolute.

kuno-raeber:hasSameEditionAsInValue
	a owl:ObjectProperty;
	rdfs:label "has same edition as in - statement"@en, "hat gleiche Edition als in - Festlegung"@de;
	rdfs:comment """Relating a poem by Kuno Raeber to a reification statement of the relation between the poem and a convolute containing a poem with the same edition."""@en;
	rdfs:subPropertyOf knora-base:hasLinkToValue;
	knora-base:subjectClassConstraint kuno-raeber:Poem;
	knora-base:objectClassConstraint knora-base:LinkValue.

kuno-raeber:hasReferencePoem
	 a owl:ObjectProperty;
	rdfs:label "has reference poem"@en, "hat Bezugsgedicht"@de;
	rdfs:comment "Relating a poem to another one as its reference."@en;
	rdfs:domain kuno-raeber:Poem;
	rdfs:range kuno-raeber:Poem;
	rdfs:subPropertyOf text:hasReferenceText;
	knora-base:subjectClassConstraint kuno-raeber:Poem;
	knora-base:objectClassConstraint kuno-raeber:Poem.

kuno-raeber:hasReferencePoemValue
	a owl:ObjectProperty;
	rdfs:label "has reference poem - statement"@en, "hat Bezugsgedicht - Festlegung"@de;
	rdfs:comment "Relating a poem to a reification statement of the relation between the poem and another one as its reference."@en;
	rdfs:subPropertyOf text:hasReferenceTextValue;
	knora-base:subjectClassConstraint kuno-raeber:Poem;
	knora-base:objectClassConstraint knora-base:LinkValue.

kuno-raeber:hasReferenceTitle
	a owl:ObjectProperty;
	rdfs:label "has reference title"@en, "hat Bezugstitel"@de;
	rdfs:comment """Relating a poem to a title of a reference poem."""@en;
	rdfs:domain kuno-raeber:Poem;
	rdfs:range rdfs:Literal;
	rdfs:subPropertyOf text:hasTitle;
	knora-base:subjectClassConstraint kuno-raeber:Poem;
	knora-base:objectClassConstraint knora-base:TextValue.

kuno-raeber:hasContentPartInPolyAuthorPublicationConvolute
	a owl:ObjectProperty;
	rdfs:label "has part in poly-author publication convolute"@en, "ist Teilweise in einem Mehrautorenpublikationen-Konvolut"@de;
	rdfs:comment "Relating a poly-author publication to a convolute it has part of its content in."@en;
	rdfs:domain kuno-raeber:PolyAuthorPublication;
	rdfs:range kuno-raeber:PolyAuthorPublicationConvolute;
	rdfs:subPropertyOf knora-base:hasLinkTo;
	knora-base:subjectClassConstraint kuno-raeber:PolyAuthorPublication;
	knora-base:objectClassConstraint kuno-raeber:PolyAuthorPublicationConvolute.

kuno-raeber:hasContentPartInPolyAuthorPublicationConvoluteValue
	a owl:ObjectProperty;
	rdfs:label "has part in poly-author publication convolute - statement"@en, "ist Teilweise in einem Mehrautorenpublikationen-Konvolut - Festlegung"@de;
	rdfs:comment "Relating a poly-author publication to a reification statement of the relation between the publication and a convolute it has part of its content in."@en;
	rdfs:subPropertyOf knora-base:hasLinkToValue;
	knora-base:subjectClassConstraint kuno-raeber:PolyAuthorPublication;
	knora-base:objectClassConstraint knora-base:LinkValue.

kuno-raeber:isFinalVersion
	a owl:ObjectProperty;
	rdfs:label "is final version"@en, "ist Endfassung"@de;
	rdfs:comment """Relating a text by Kuno Raeber to being a last version or not."""@en;
	rdfs:domain kuno-raeber:Text;
	rdfs:range xsd:boolean;
	rdfs:subPropertyOf knora-base:hasValue;
	knora-base:subjectClassConstraint kuno-raeber:Text;
	knora-base:objectClassConstraint knora-base:BooleanValue.

kuno-raeber:isInSwissGerman
	a owl:ObjectProperty;
	rdfs:label "is in Swiss German"@en, "ist auf Schweizerdeutsch"@de;
	rdfs:comment """Relating a text by Kuno Raeber to being expressed in Swiss German or not."""@en;
	rdfs:domain kuno-raeber:Text;
	rdfs:range xsd:boolean;
	rdfs:subPropertyOf knora-base:hasValue;
	knora-base:subjectClassConstraint kuno-raeber:Text;
	knora-base:objectClassConstraint knora-base:BooleanValue.

kuno-raeber:isPartOfCycle
	a owl:ObjectProperty;
	rdfs:label "is part of cycle"@en, "ist Teil eines Zyklus"@de;
	rdfs:comment """Relating a text by Kuno Raeber to being part of a cycle or not."""@en;
	rdfs:domain kuno-raeber:Text;
	rdfs:range xsd:boolean;
	rdfs:subPropertyOf knora-base:hasValue;
	knora-base:subjectClassConstraint kuno-raeber:Text;
	knora-base:objectClassConstraint knora-base:BooleanValue.

kuno-raeber:hasStrophe
	a owl:ObjectProperty;
	rdfs:label "has strophe"@en, "hat Strophe"@de;
	rdfs:comment """Relating a poem by Kuno Raeber to having a strophe or not."""@en;
	rdfs:domain kuno-raeber:Poem;
	rdfs:range xsd:boolean;
	rdfs:subPropertyOf knora-base:hasValue;
	knora-base:subjectClassConstraint kuno-raeber:Poem;
	knora-base:objectClassConstraint knora-base:BooleanValue.