@prefix rdf: <http://www.w3.org/1999/02/22-rdf-syntax-ns#>.
@prefix rdfs: <http://www.w3.org/2000/01/rdf-schema#>.
@prefix owl: <http://www.w3.org/2002/07/owl#>.
@prefix xsd: <http://www.w3.org/2001/XMLSchema#>.
@prefix skos: <http://www.w3.org/2004/02/skos/core#>.
@prefix dct: <http://purl.org/dc/terms/>.
@prefix foaf: <http://xmlns.com/foaf/0.1/>.
@prefix cidoc: <http://www.cidoc-crm.org/cidoc-crm/>.
@prefix frbroo: <http://iflastandards.info/ns/fr/frbr/frbroo/>.
@prefix event: <http://www.knora.org/ontology/0047/event#>.
@prefix human: <http://www.knora.org/ontology/0048/human#>.
@prefix concept: <http://www.knora.org/ontology/0044/concept#>.
@prefix math: <http://www.knora.org/ontology/0061/mathematics#>.
@prefix ling: <http://www.knora.org/ontology/005D/linguistics#>.
@prefix text: <http://www.knora.org/ontology/0059/text#>.
@prefix text-structure: <http://www.knora.org/ontology/005B/text-structure#>.
@prefix infocar: <http://www.knora.org/ontology/004C/information-carrier#>.
@prefix publish: <http://www.knora.org/ontology/0056/publishing#>.
@prefix knora-base: <http://www.knora.org/ontology/knora-base#>.

@base <http://www.knora.org/ontology/005C/document>.
@prefix document: <http://www.knora.org/ontology/005C/document#>.

<http://www.knora.org/ontology/005C/document>
	a owl:Ontology;
	dct:title "An ontology about document"@en;
	dct:description """Formal description of document, general subclasses, related classes and properties."""@en;
	dct:creator "Hans Cools, MD, knowledge engineer, ontologist, software developer, NIE-INE, Basel University, Switzerland"@en;
	dct:publisher "Basel University, Switzerland"@en;

	knora-base:attachedToProject <http://rdfh.ch/projects/005C>.


# EMBRYONIC: declared 'middle-out', on the go as concepts are needed, not intended to contain upfront all elements


#
# CLASSES
#

# Transfer text independent elemenst from 'text' etc.

document:Document
	a owl:Class;
	rdfs:label "document"@en, "Dokument"@de;
	rdfs:comment """."""@en;
	rdfs:subClassOf concept:Information, cidoc:E31_Document.

document:Element #*
	a owl:Class;
	rdfs:label "document element"@en, "Dokumentelement"@de;
	rdfs:comment """."""@en; #*
	rdfs:subClassOf concept:Information, [
		a owl:Restriction; owl:onProperty document:isPartOfDocument; owl:minCardinality "0"^^xsd:nonNegativeInteger], [
		a owl:Restriction; owl:onProperty document:isPartOfDocumentValue; owl:minCardinality "0"^^xsd:nonNegativeInteger], [
		a owl:Restriction; owl:onProperty document:hasFootnoteReferenceNumber; owl:minCardinality "0"^^xsd:nonNegativeInteger], [
		a owl:Restriction; owl:onProperty document:hasFootnoteReferenceNumberValue; owl:minCardinality "0"^^xsd:nonNegativeInteger], [
		a owl:Restriction; owl:onProperty document:hasFootnoteReferenceIdentifier; owl:minCardinality "0"^^xsd:nonNegativeInteger], [
		a owl:Restriction; owl:onProperty document:hasFootnoteReferenceIdentifierValue; owl:minCardinality "0"^^xsd:nonNegativeInteger], [
		a owl:Restriction; owl:onProperty document:hasEndnoteReferenceNumber; owl:minCardinality "0"^^xsd:nonNegativeInteger], [
		a owl:Restriction; owl:onProperty document:hasEndnoteReferenceNumberValue; owl:minCardinality "0"^^xsd:nonNegativeInteger], [
		a owl:Restriction; owl:onProperty document:hasEndnoteReferenceIdentifier; owl:minCardinality "0"^^xsd:nonNegativeInteger], [
		a owl:Restriction; owl:onProperty document:hasEndnoteReferenceIdentifierValue; owl:minCardinality "0"^^xsd:nonNegativeInteger].

# infocar:ElectronicFootnoteReference electronic link on carrier, not abstractable from carrier
#	a owl:Class;
#	rdfs:label "footnote reference"@en, "Fussnotereferenz"@de;
#	rdfs:comment """Symbol of a footnoteReference."""@en;
#*	rdfs:subClassOf x:z, [
#		a owl:Restriction; owl:onProperty document:ReferenceHasSymbol; owl:minCardinality "0"^^xsd:nonNegativeInteger], [
#		a owl:Restriction; owl:onProperty document:referenceHasLink; owl:minCardinality "0"^^xsd:nonNegativeInteger].

# document:Structure

document:Layout
	a owl:Class;
	rdfs:label "layout"@en, "Aufmachung"@de;
	rdfs:comment """Way in which the content of a page is set out."""@en;
	rdfs:subClassOf knora-base:Resource. #* concept:Layout

document:Column
	a owl:Class;
	rdfs:label "column"@en, "Spalte"@de;
	rdfs:comment """Document element displaying information, e.g. text lines and graphs, as a column as part of a page."""@en;
	rdfs:subClassOf text-structure:ReadabilityStructure, [ # document:Element
#		a owl:Restriction; owl:onProperty document:isPartOfPage; owl:allValuesFrom document:Page], [
		a owl:Restriction; owl:onProperty document:columnIsPartOfPage; owl:minCardinality "0"^^xsd:nonNegativeInteger], [
		a owl:Restriction; owl:onProperty document:columnIsPartOfPageValue; owl:minCardinality "0"^^xsd:nonNegativeInteger].

document:Page # text, visuals, page # etc.
	a owl:Class;
	rdfs:label "page"@en, "Seite"@de;
	rdfs:comment """Document element displaying information e.g. text lines and graphs, as a page as part of a document."""@en;
	rdfs:subClassOf text-structure:ReadabilityStructure, [ # document:Element
#		a owl:Restriction; owl:onProperty text-structure:pageIsPartO; owl:allValuesFrom language:HumanNaturalLanguageExpression], [
		a owl:Restriction; owl:onProperty document:pageIsPartOfDocument; owl:minCardinality "0"^^xsd:nonNegativeInteger], [
		a owl:Restriction; owl:onProperty document:pageIsPartOfDocumentValue; owl:minCardinality "0"^^xsd:nonNegativeInteger].

document:Marginal
	a owl:Class;
	rdfs:label "marginal"@en, "Marginale"@de; # in GUI can be "marginalia"@en, "Marginalien"@de
	rdfs:comment """Information besides a text in the margin of a carrier, e.g. text, doodles, illuminations."""@en;
	rdfs:subClassOf document:Element.

# document:Table

# Format
# Size
# structure
# Shape
# color

document:ElectronicDocument
	a owl:Class;
	rdfs:label "electronic document"@en,"elektronisches Dokument"@de;
	rdfs:comment """Document stored as electronic information."""@en;
	rdfs:subClassOf document:Document, concept:ElectronicInformation.

document:ElectronicElement #*
	a owl:Class;
	rdfs:label "electronic document element"@en, "elektronisches Dokumentelement"@de;
	rdfs:comment """."""@en; #*
	rdfs:subClassOf document:Element, concept:ElectronicInformation, [
		a owl:Restriction; owl:onProperty document:isPartOfElectronicDocument; owl:minCardinality "0"^^xsd:nonNegativeInteger], [
		a owl:Restriction; owl:onProperty document:isPartOfElectronicDocumentValue; owl:minCardinality "0"^^xsd:nonNegativeInteger], [
		a owl:Restriction; owl:onProperty document:hasHyperlink; owl:minCardinality "0"^^xsd:nonNegativeInteger].

document:HypertextDocument
	a owl:Class;
	rdfs:label "hypertext document"@en,"Hypertext-Dokument"@de;
	rdfs:comment """Electronic document written in HTML."""@en;
	rdfs:subClassOf document:ElectronicDocument.

#
# PROPERTIES
#

# document:isLayoutOf
#	a owl:ObjectProperty;
#	rdfs:label "is layout of"@en, "ist Aufmachung von"@de;
#	rdfs:comment "Relating a layout to a document."@en;
#	rdfs:domain layout:Layout;
#	rdfs:range document:Document;
#	rdfs:subPropertyOf knora-base:hasLinkTo;
#	knora-base:subjectClassConstraint layout:Layout;
#	knora-base:objectClassConstraint document:Document.

document:isPartOfDocument
	a owl:ObjectProperty;
	rdfs:label "is part of document"@en, "ist teil eines Dokumentes"@de;
	rdfs:comment """Relating a document element to a document it is part of."""@en;
	rdfs:domain document:Element;
	rdfs:range document:Document;
	rdfs:subPropertyOf concept:isPartOf;
	knora-base:subjectClassConstraint document:Element;
	knora-base:objectClassConstraint document:Document.

document:isPartOfDocumentValue
	a owl:ObjectProperty;
	rdfs:label "is part of document - statement"@en, "ist teil eines Dokumentes - Festlegung"@de;
	rdfs:comment """Relating a document element to a reification statement of the relation between the element and a document it is part of."""@en;
	rdfs:subPropertyOf concept:isPartOfValue;
	knora-base:subjectClassConstraint document:Element;
	knora-base:objectClassConstraint knora-base:LinkValue.

document:columnIsPartOfPage
	a owl:ObjectProperty;
	rdfs:label "column is part of page"@en, "Spalte ist Teil einer Seite"@de;
	rdfs:comment """Relating a column to a page it is part of."""@en;
	rdfs:domain document:Column;
	rdfs:range document:Page;
	rdfs:subPropertyOf concept:isPartOf;
	knora-base:subjectClassConstraint document:Column;
	knora-base:objectClassConstraint document:Page.

document:columnIsPartOfPageValue
	a owl:ObjectProperty;
	rdfs:label "column is part of page - statement"@en, "Spalte ist Teil einer Seite - Festlegung"@de;
	rdfs:comment """Relating a column to a reification statement of the relation between the column and a page it is part of."""@en;
	rdfs:subPropertyOf concept:isPartOfValue;
	knora-base:subjectClassConstraint document:Column;
	knora-base:objectClassConstraint knora-base:LinkValue.

document:pageIsPartOfDocument
	a owl:ObjectProperty;
	rdfs:label "page is part of document"@en, "Seite ist Teil eines Dokumentes"@de;
	rdfs:comment """Relating a page to a document it is part of."""@en;
	rdfs:domain document:Page;
	rdfs:range document:Document;
	rdfs:subPropertyOf concept:isPartOf;
	knora-base:subjectClassConstraint document:Page;
	knora-base:objectClassConstraint document:Document.

document:pageIsPartOfDocumentValue
	a owl:ObjectProperty;
	rdfs:label "page is part of document - statement"@en, "Seite ist Teil eines Dokumentes - Festlegung"@de;
	rdfs:comment """Relating a page to a reification statement of the relation between the page and a document it is part of."""@en;
	rdfs:subPropertyOf concept:isPartOfValue;
	knora-base:subjectClassConstraint document:Page;
	knora-base:objectClassConstraint knora-base:LinkValue.

document:hasFootnoteReferenceNumber
	a owl:ObjectProperty;
	rdfs:label "has footnote reference number"@en, "hat Fussnotereferenznummer"@de;
	rdfs:comment """Relating a document element to a footnote reference number (as resource) it has."""@en;
	rdfs:domain document:Element;
	rdfs:range math:NaturalNumber;
	rdfs:subPropertyOf knora-base:hasLinkTo;
	knora-base:subjectClassConstraint document:Element;
	knora-base:objectClassConstraint math:NaturalNumber.

document:hasFootnoteReferenceNumberValue
	a owl:ObjectProperty;
	rdfs:label "has footnote reference number - statement"@en, "hat Fussnotereferenznummer - Festlegung"@de;
	rdfs:comment """Relating a document element to a reification statement of the relation between the element and a footnote reference number (as resource) it has."""@en;
	rdfs:subPropertyOf knora-base:hasLinkToValue;
	knora-base:subjectClassConstraint document:Element;
	knora-base:objectClassConstraint knora-base:LinkValue.

document:hasFootnoteReferenceIdentifier
	a owl:ObjectProperty;
	rdfs:label "has footnote reference identifier"@en, "hat Fussnotereferenzidentifikator"@de;
	rdfs:comment """Relating a document element to a footnote reference identifier (as resource) it has."""@en;
	rdfs:domain document:Element;
	rdfs:range concept:Identifier;
	rdfs:subPropertyOf knora-base:hasLinkTo;
	knora-base:subjectClassConstraint document:Element;
	knora-base:objectClassConstraint concept:Identifier.

document:hasFootnoteReferenceIdentifierValue
	a owl:ObjectProperty;
	rdfs:label "has footnote reference identifier - statement"@en, "hat Fussnotereferenzidentifikator - Festlegung"@de;
	rdfs:comment """Relating a document element to a reification statement of the relation between the element and a footnote reference identifier (as resource) it has."""@en;
	rdfs:subPropertyOf knora-base:hasLinkToValue;
	knora-base:subjectClassConstraint document:Element;
	knora-base:objectClassConstraint knora-base:LinkValue.

document:hasEndnoteReferenceNumber
	a owl:ObjectProperty;
	rdfs:label "has endnote reference number"@en, "hat Endnotereferenznummer"@de;
	rdfs:comment """Relating a document element to an endnote reference number (as resource) it has."""@en;
	rdfs:domain document:Element;
	rdfs:range math:NaturalNumber;
	rdfs:subPropertyOf knora-base:hasLinkTo;
	knora-base:subjectClassConstraint document:Element;
	knora-base:objectClassConstraint math:NaturalNumber.

document:hasEndnoteReferenceNumberValue
	a owl:ObjectProperty;
	rdfs:label "has endnote reference number - statement"@en, "hat Endnotereferenznummer - Festlegung"@de;
	rdfs:comment """Relating a document element to a reification statement of the relation between the element and an endnote reference number (as resource) it has."""@en;
	rdfs:subPropertyOf knora-base:hasLinkToValue;
	knora-base:subjectClassConstraint document:Element;
	knora-base:objectClassConstraint knora-base:LinkValue.

document:hasEndnoteReferenceIdentifier
	a owl:ObjectProperty;
	rdfs:label "has endnote reference identifier"@en, "hat Endnotereferenzidentifikator"@de;
	rdfs:comment """Relating a document element to an endnote reference identifier (as resource) it has."""@en;
	rdfs:domain document:Element;
	rdfs:range concept:Identifier;
	rdfs:subPropertyOf knora-base:hasLinkTo;
	knora-base:subjectClassConstraint document:Element;
	knora-base:objectClassConstraint concept:Identifier.

document:hasEndnoteReferenceIdentifierValue
	a owl:ObjectProperty;
	rdfs:label "has endnote reference identifier - statement"@en, "hat Endnotereferenzidentifikator - Festlegung"@de;
	rdfs:comment """Relating a document element to a reification statement of the relation between the element and an endnote reference identifier (as resource) it has."""@en;
	rdfs:subPropertyOf knora-base:hasLinkToValue;
	knora-base:subjectClassConstraint document:Element;
	knora-base:objectClassConstraint knora-base:LinkValue.

document:isPartOfElectronicDocument
	a owl:ObjectProperty;
	rdfs:label "is part of electronic document"@en, "ist teil eines elektronischen Dokumentes"@de;
	rdfs:comment """Relating an electronic document element to an electronic document it is part of."""@en;
	rdfs:domain document:ElectronicElement;
	rdfs:range document:ElectronicDocument;
	rdfs:subPropertyOf concept:isPartOf;
	knora-base:subjectClassConstraint document:ElectronicElement;
	knora-base:objectClassConstraint document:ElectronicDocument.

document:isPartOfElectronicDocumentValue
	a owl:ObjectProperty;
	rdfs:label "is part of electronic document - statement"@en, "ist teil eines elektronischen Dokumentes - Festlegung"@de;
	rdfs:comment """Relating an electronic document element to a reification statement of the relation between the element and an electronic document it is part of."""@en;
	rdfs:subPropertyOf concept:isPartOfValue;
	knora-base:subjectClassConstraint document:ElectronicElement;
	knora-base:objectClassConstraint knora-base:LinkValue.

document:hasHyperlink
	a owl:ObjectProperty;
	rdfs:label "has hyperlink"@en, "hat Hyperlink"@de;
	rdfs:comment """Relating an electronic document element to a hyperlink it has."""@en;
	rdfs:domain document:ElectronicElement;
#	rdfs:range infocar:Hyperlink;
	rdfs:subPropertyOf knora-base:hasValue;
	knora-base:subjectClassConstraint document:ElectronicElement;
	knora-base:objectClassConstraint knora-base:UriValue.