@prefix rdfs: <http://www.w3.org/2000/01/rdf-schema#>.
@prefix owl: <http://www.w3.org/2002/07/owl#>.
@prefix xsd: <http://www.w3.org/2001/XMLSchema#>.
@prefix skos: <http://www.w3.org/2004/02/skos/core#>.
@prefix dct: <http://purl.org/dc/terms/>.
@prefix text: <http://www.knora.org/ontology/0059/text#>.
@prefix textedit: <http://www.knora.org/ontology/005A/text-editing#>.
@prefix knora-base: <http://www.knora.org/ontology/knora-base#>.

@base <http://www.knora.org/ontology/0067/parzival>.
@prefix parzival: <http://www.knora.org/ontology/0067/parzival#>.

<http://www.knora.org/ontology/0067/parzival>
	a owl:Ontology;
	dct:title """An ontology about Wolfram von Eschenbach's "Parzival" """@en;
	dct:description """Formal description of specific concepts in the scientific study and digital edition of Wolfram von Eschenbach's "Parzival"."""@en;
	dct:creator "Hans Cools, MD, knowledge engineer, ontologist, software developer, NIE-INE, Basel University, Switzerland"@en;
	dct:contributor "Reinhard Priber, tool coordinator and software developer, NIE-INE, University of Zürich, Switzerland"@en;
	dct:publisher "Basel University, Switzerland"@en;

	knora-base:attachedToProject <http://rdfh.ch/projects/0067>.

#
# CLASSES
#

° parzival:EditedVerseNovel
	a owl:Class;
	rdfs:label """edited version of Wolfram Von Eschenbach's 'Parzival'"""@en, """Vers von Wolfram Von Eschenbachs 'Parzival'"""@de;
	rdfs:comment """Handwritten transcription of Wolfram Von Eschenbach's 'Parzival'."""@en;
	rdfs:subClassOf text:HandwrittenText, [
		a owl:Restriction; owl:onProperty infocar:isInManuscript; owl:minCardinality "0"^^xsd:nonNegativeInteger], [
		a owl:Restriction; owl:onProperty infocar:isInManuscriptValue; owl:minCardinality "0"^^xsd:nonNegativeInteger].

parzival:Verse
	a owl:Class;
	rdfs:label """verse of Wolfram Von Eschenbach's 'Parzival'"""@en, """Vers von Wolfram Von Eschenbachs 'Parzival'"""@de;
	rdfs:comment """Verse in Wolfram Von Eschenbach's 'Parzival'."""@en;
	rdfs:subClassOf text-structure:Verse, [
		a owl:Restriction; owl:onProperty parzival:isVerseOfDreissiger; owl:minCardinality "0"^^xsd:nonNegativeInteger], [
		a owl:Restriction; owl:onProperty parzival:isVerseOfDreissigerValue; owl:minCardinality "0"^^xsd:nonNegativeInteger].

parzival:Dreissiger
	a owl:Class;
	rdfs:label "dreissiger"@en, "Dreissiger"@de;
	rdfs:comment """Strophe of 30 verses in Wolfram Von Eschenbach's 'Parzival'."""@en;
	rdfs:seeAlso """Bumke Joachim, "Wolfram von Eschenbach", Springer-Verlag, Stuttgart, 2004."""@en;
	rdfs:subClassOf text-structure:Strophe, [
		a owl:Restriction; owl:onProperty parzival:isDreissigerOfNovel; owl:minCardinality "0"^^xsd:nonNegativeInteger], [
		a owl:Restriction; owl:onProperty parzival:isDreissigerOfNovelValue; owl:minCardinality "0"^^xsd:nonNegativeInteger].

parzival:CriticalApparatus
	a owl:Class;
	rdfs:label "critical apparatus"@en, "textkritischer Apparat"@de;
	rdfs:comment """Editing apparatus to a critical text edition providing information of a textual version."""@en;
	rdfs:subClassOf text-structure:CriticalApparatus.

#
# PROPERTIES
#

parzival:isVerseOfDreissiger
	a owl:ObjectProperty;
	rdfs:label "is verse of dreissiger"@en, "ist Vers eines Dreissigers"@de;
	rdfs:comment """Relating a verse to a dreissiger it is part of."""@en;
	rdfs:domain parzival:Verse;
	rdfs:range parzival:Dreissiger;
	rdfs:subPropertyOf text-structure:isVerseOfStrophe;
	knora-base:subjectClassConstraint parzival:Verse;
	knora-base:objectClassConstraint parzival:Dreissiger.

parzival:isVerseOfDreissigerValue
	a owl:ObjectProperty;
	rdfs:label "is verse of dreissiger - statement"@en, "ist Vers eines Dreissigers - Festlegung"@de;
	rdfs:comment """Relating a verse to a reification statement of the relation between the verse and a dreissiger it is part of."""@en;
	rdfs:subPropertyOf text-structure:isVerseOfStropheValue;
	knora-base:subjectClassConstraint parzival:Verse;
	knora-base:objectClassConstraint knora-base:LinkValue.

parzival:isDreissigerOfNovel
	a owl:ObjectProperty;
	rdfs:label "is dreissiger of verse novel"@en, "ist Dreissiger eines Versromans"@de;
	rdfs:comment """Relating a dreissiger to a verse novel it is part of."""@en;
	rdfs:domain parzival:Dreissiger;
	rdfs:range litera:VerseNovel;
	rdfs:subPropertyOf concept:isPartOf;
	knora-base:subjectClassConstraint parzival:Dreissiger;
	knora-base:objectClassConstraint litera:VerseNovel.

parzival:isDreissigerOfNovelValue
	a owl:ObjectProperty;
	rdfs:label "is dreissiger of verse novel - statement"@en, "ist Dreissiger eines Versromans - Festlegung"@de;
	rdfs:comment """Relating a dreissiger to a reification statement of the relation between the dreissiger and a verse novel it is part of."""@en;
	rdfs:subPropertyOf concept:isPartOfValue;
	knora-base:subjectClassConstraint parzival:Dreissiger;
	knora-base:objectClassConstraint knora-base:LinkValue.