@prefix rdfs: <http://www.w3.org/2000/01/rdf-schema#>.
@prefix owl: <http://www.w3.org/2002/07/owl#>.
@prefix xsd: <http://www.w3.org/2001/XMLSchema#>.
@prefix skos: <http://www.w3.org/2004/02/skos/core#>.
@prefix dct: <http://purl.org/dc/terms/>.
@prefix cidoc: <http://www.cidoc-crm.org/cidoc-crm/>.
@prefix human: <http://www.knora.org/ontology/0048/human#>.
@prefix concept: <http://www.knora.org/ontology/0044/concept#>.
@prefix language: <http://www.knora.org/ontology/004F/language#>.
@prefix text: <http://www.knora.org/ontology/0059/text#>.
@prefix text-structure: <http://www.knora.org/ontology/005B/text-structure#>.
@prefix textedit: <http://www.knora.org/ontology/005A/text-editing#>.
@prefix ling: <http://www.knora.org/ontology/005D/linguistics#>.
@prefix logic: <http://www.knora.org/ontology/005E/logic#>.
@prefix knora-base: <http://www.knora.org/ontology/knora-base#>.

@base <http://www.knora.org/ontology/0057/scholasticism>.
@prefix schola: <http://www.knora.org/ontology/0057/scholasticism#>.

<http://www.knora.org/ontology/0057/scholasticism>
	a owl:Ontology;
	dct:title "An ontology about Scholasticism"@en;
	dct:description """Formal description of elements in Scholasticism."""@en;
	dct:creator "Hans Cools, MD, knowledge engineer, ontologist, software developer, NIE, University of Basel, Switzerland"@en;
	dct:contributor "Prof. Dr. Ueli Zahnd, Faculty of Theology, University of Basel, Switzerland"@en, "Gabriel MÃ¼ller, Faculty of Theology, University of Basel, Switzerland"@en;
	dct:publisher "Basel University, Switzerland"@en;

	knora-base:attachedToProject <http://rdfh.ch/projects/0057>.

#
# CLASSES
#

schola:Scholasticism
	a owl:Class;
	rdfs:label "scholasticism"@en, "Scholastik"@de;
	rdfs:comment """Method of critical thought dominating theological and philosophical study in Western Christianity and teaching by academics or scholastics (schoolmen) of universities in Europe from about 1100 to 1700."""@en;
	rdfs:subClassOf concept:ThoughtMethod. #*

schola:Scholastic
	a owl:Class;
	rdfs:label "scholastic"@en, "ScholastikerIn"@de;
	rdfs:comment """An adherent of Scholasticism."""@en;
	skos:note """There are no female scholastics because women were not allowed to universities."""@en; # Can this be stated that absolute?
	rdfs:subClassOf human:Person, [
#		a owl:Restriction; owl:onProperty schola:hasRole; owl:someValuesFrom schola:Role], [
		a owl:Restriction; owl:onProperty schola:hasRole; owl:minCardinality "0"^^xsd:nonNegativeInteger], [
		a owl:Restriction; owl:onProperty schola:hasRoleValue; owl:minCardinality "0"^^xsd:nonNegativeInteger] #, [
#		a owl:Restriction; owl:onProperty schola:hasReportatorRole; owl:minCardinality "0"^^xsd:nonNegativeInteger], [
#		a owl:Restriction; owl:onProperty schola:hasReportatorRoleValue; owl:minCardinality "0"^^xsd:nonNegativeInteger]
		.

#* schola:Translator: SCO text:Translator: handwriting?

schola:Role
	a owl:Class;
	rdfs:label "scholastic role"@en;
	rdfs:comment """Role a scholastic has."""@en;
	rdfs:subClassOf human:Role.

schola:Reportator
	a owl:Class;
	rdfs:label "reportator"@la, "reportator"@en, "Reportator"@de;
	rdfs:comment """Role of a scholastic student registering the content of a lesson."""@en; #* also secretary of lecturer, RP
	rdfs:subClassOf schola:Role.

# schola:Expression
#	a owl:Class;
#	rdfs:label "scholastic expression"@en, "scholastischer Expression"@de;
#	rdfs:comment """Expression created by a scholastic."""@en;
#	rdfs:subClassOf document:Expression.

schola:Commentary
	a owl:Class;
	rdfs:label "scholastic commentary"@en, "scholastischer Kommentar"@de, "commentarius scholasticus"@la;
	rdfs:comment """Commentary made by a scholastic."""@en;
	rdfs:subClassOf text:Commentary. # , [
#		a owl:Restriction; owl:onProperty schola:commentaryHasProcedure; owl:minCardinality "0"^^xsd:nonNegativeInteger], [
#		a owl:Restriction; owl:onProperty schola:commentaryHasProcedureValue; owl:minCardinality "0"^^xsd:nonNegativeInteger].

schola:ProceduralCommentary
	a owl:Class;
	rdfs:label "procedural scholastic commentary"@en, "prozeduraler scholastischer Kommentar"@de;
	rdfs:comment """Scholastic commentary as result of a creation procedure."""@en;
	rdfs:subClassOf schola:Commentary.

# schola:CommentingProcedure #* RLP: stage?
#	a owl:Class;
#	rdfs:label "scholastic commenting procedure"@en, "scholastische Kommentierungvorgehensweise"@de;
#	rdfs:comment """Scholastic procedure to comment."""@en;
#	rdfs:subClassOf event:Procedure. # event:Stage

schola:Lectura
	a owl:Class;
	rdfs:label "lectura"@la, "lectura"@en, "Lectura"@de;
	rdfs:comment """Scholastic commentary on a text expression, as presented by its author in a lecture."""@en;
	rdfs:subClassOf schola:ProceduralCommentary.

schola:LecturaRevisa #* RLP: = Ordinatio? => for publication? ; after Lectura
	a owl:Class;
	rdfs:label "lectura revisa"@la, "lectura revisa"@en, "Lectura Revisa"@de;
	rdfs:comment """Scholastic commentary on a text expression, as revised by its author after its presentation in a lecture."""@en;
	rdfs:subClassOf schola:ProceduralCommentary, [
		a owl:Restriction; owl:onProperty schola:hasReportator; owl:minCardinality "0"^^xsd:nonNegativeInteger], [
		a owl:Restriction; owl:onProperty schola:hasReportatorValue; owl:minCardinality "0"^^xsd:nonNegativeInteger].

schola:Reportatio #* after LecturaRevisa
	a owl:Class;
	rdfs:label "reportatio"@la, "reportatio"@en, "Reportatio"@de;
	rdfs:comment """Scholastic commentary on a text expression, as recorded by a *student* in a lecture."""@en; #* RLP: "listener", "auditor" instead of "student"?
	rdfs:subClassOf schola:ProceduralCommentary.

schola:ReportatioApprobata #* after Reportatio
	a owl:Class;
	rdfs:label "reportatio approbata"@la, "reportatio approbata"@en, "Reportatio Approbata"@de;
	rdfs:comment """Scholastic commentary on a text expression as recorded by * and approved by the *lecturer OR author*."""@en;
	rdfs:subClassOf schola:ProceduralCommentary.

schola:Ordinatio #* after ReportatioApprobata
	a owl:Class;
	rdfs:label "ordinatio"@la, "ordinatio"@en, "Ordinatio"@de;
	rdfs:comment """Scholastic commentary on a text expression as composed for publication."""@en;
	rdfs:subClassOf schola:ProceduralCommentary.

schola:Structure
	a owl:Class;
	rdfs:label "scholastic text structure"@en, "scholastischer Textstruktur"@de;
	rdfs:comment """Text structure as existing in scholastics."""@en;
	rdfs:subClassOf text-structure:Structure, [
		a owl:Restriction; owl:onProperty schola:isPartOfCommentary; owl:minCardinality "0"^^xsd:nonNegativeInteger], [
		a owl:Restriction; owl:onProperty schola:isPartOfCommentaryValue; owl:minCardinality "0"^^xsd:nonNegativeInteger].

schola:Gloss
	a owl:Class;
	rdfs:label "scholastic gloss"@en, "scholastischer Glosse"@de;
	rdfs:comment """Gloss as existing in scholastics."""@en;
	rdfs:subClassOf schola:Structure, text-structure:Gloss, [
		a owl:Restriction; owl:onProperty schola:isGlossOfCommentary; owl:minCardinality "0"^^xsd:nonNegativeInteger], [
		a owl:Restriction; owl:onProperty schola:isGlossOfCommentaryValue; owl:minCardinality "0"^^xsd:nonNegativeInteger].

# Sentence:
#		a owl:Restriction; owl:onProperty schola:hasGlossator; owl:minCardinality "0"^^xsd:nonNegativeInteger], [
#		a owl:Restriction; owl:onProperty schola:hasGlossatorValue; owl:minCardinality "0"^^xsd:nonNegativeInteger].

schola:Verse
	a owl:Class;
	rdfs:label "scholastic verse"@en, "scholastischer Vers"@de;
	rdfs:comment """Verse as existing in scholastics."""@en;
	rdfs:subClassOf schola:Structure, text-structure:Verse, [
		a owl:Restriction; owl:onProperty schola:isVerseOfCommentary; owl:minCardinality "0"^^xsd:nonNegativeInteger], [
		a owl:Restriction; owl:onProperty schola:isVerseOfCommentaryValue; owl:minCardinality "0"^^xsd:nonNegativeInteger].

schola:Table #** only text?
	a owl:Class;
	rdfs:label "scholastic table"@en, "scholastische Tabelle"@de;
	rdfs:comment """Table as existing in scholastics."""@en;
	rdfs:subClassOf text-structure:Table, schola:Structure,  [
		a owl:Restriction; owl:onProperty schola:isTableOfCommentary; owl:minCardinality "0"^^xsd:nonNegativeInteger], [
		a owl:Restriction; owl:onProperty schola:isTableOfCommentaryValue; owl:minCardinality "0"^^xsd:nonNegativeInteger].

schola:SentenceCommentary
	a owl:Class;
	rdfs:label "scholastic sentence commentary"@en, "scholastischer Satz-Kommentar"@de;
	rdfs:comment """Commentary with sentence structure, made by a scholastic."""@en;
	rdfs:subClassOf schola:Commentary, text:SentenceExpression.

schola:Question
	a owl:Class;
	rdfs:label "scholastic question"@en, "scholastische Frage"@de;
	rdfs:comment """Question as existing in scholastics."""@en;
	rdfs:subClassOf schola:Structure, ling:Question, [
		a owl:Restriction; owl:onProperty schola:isQuestionOfCommentary; owl:minCardinality "0"^^xsd:nonNegativeInteger], [
		a owl:Restriction; owl:onProperty schola:isQuestionOfCommentaryValue; owl:minCardinality "0"^^xsd:nonNegativeInteger].

schola:Conclusion
	a owl:Class;
	rdfs:label "scholastic conclusion"@en, "scholastische Konklusion"@de;
	rdfs:comment """Conclusion as existing in scholastics."""@en;
	rdfs:subClassOf schola:Structure, logic:Conclusion, [
		a owl:Restriction; owl:onProperty schola:isConclusionOfCommentary; owl:minCardinality "0"^^xsd:nonNegativeInteger], [
		a owl:Restriction; owl:onProperty schola:isConclusionOfCommentaryValue; owl:minCardinality "0"^^xsd:nonNegativeInteger].

schola:Syllogism
	a owl:Class;
	rdfs:label "scholastic syllogism"@en, "scholastischer Syllogismus"@de;
	rdfs:comment """Syllogism as existing in scholastics."""@en;
	rdfs:subClassOf schola:Structure, logic:Syllogism, [
		a owl:Restriction; owl:onProperty schola:isSyllogismOfCommentary; owl:minCardinality "0"^^xsd:nonNegativeInteger], [
		a owl:Restriction; owl:onProperty schola:isSyllogismOfCommentaryValue; owl:minCardinality "0"^^xsd:nonNegativeInteger].

schola:Abbreviation
	a owl:Class;
	rdfs:label "abbreviation commentary"@en, "Kurzfassung-Kommentar"@de, "abbreviatio"@la;
	rdfs:comment """Scholastic commentary as abbreviation."""@en;
	rdfs:subClassOf schola:Commentary, textedit:Abbreviation.

schola:Paraphrase
	a owl:Class;
	rdfs:label "paraphrase commentary"@en, "Paraphrase-Kommentar"@de;
	rdfs:comment """Scholastic commentary as paraphrase."""@en;
	rdfs:subClassOf schola:Commentary, textedit:Paraphrase.

schola:LiteralExposition
	a owl:Class;
	rdfs:label "literal exposition commentary"@en, "wÃ¶rtliche Auslegung-Kommentar"@de;
	rdfs:comment """Scholastic commentary as literal exposition."""@en;
	rdfs:subClassOf schola:Commentary, textedit:LiteralExposition.

#
# PROPERTIES
#

schola:hasRole
	a owl:ObjectProperty;
	rdfs:label "has role"@en, "hat Rolle"@de;
	rdfs:comment """Relating a scholastic to a role he has."""@en;
	rdfs:domain schola:Scholastic;
	rdfs:range schola:Role;
	rdfs:subPropertyOf human:hasRole;
	knora-base:subjectClassConstraint schola:Scholastic;
	knora-base:objectClassConstraint schola:Role.

schola:hasRoleValue
	a owl:ObjectProperty;
	rdfs:label "has role - statement"@en, "hat Rolle - Festlegung"@de;
	rdfs:comment """Relating a scholastic to a statement as reification of the relation between the scholastic and a role he has."""@en;
	rdfs:subPropertyOf human:hasRoleValue;
	knora-base:subjectClassConstraint schola:Scholastic;
	knora-base:objectClassConstraint knora-base:LinkValue.

# schola:hasReportatorRole
#	a owl:ObjectProperty;
#	rdfs:label "has reportator role"@en, "hat Reportator Rolle"@de;
#	rdfs:comment """Relating a scholastic to a reportator role he has."""@en;
#	rdfs:domain schola:Scholastic;
#	rdfs:range schola:Reportator;  
#	rdfs:subPropertyOf schola:hasRole;
#	knora-base:subjectClassConstraint schola:Scholastic;
#	knora-base:objectClassConstraint schola:Reportator.

# schola:hasReportatorRoleValue
#	a owl:ObjectProperty;
#	rdfs:label "has reportator role - statement"@en, "hat Reportator Rolle - Festlegung"@de;
#	rdfs:comment """Relating a scholastic to a statement as reification of the relation between the scholastic and a reportator role he has."""@en;
#	rdfs:subPropertyOf schola:hasRoleValue;
#	knora-base:subjectClassConstraint schola:Scholastic;
#	knora-base:objectClassConstraint knora-base:LinkValue.

 schola:hasReportator
	a owl:ObjectProperty;
	rdfs:label "has reportator"@en, "hat Reportator"@de;
	rdfs:comment """Relating a scholastic comment of a lecture to a scholastic who reported it."""@en;
	rdfs:domain schola:LecturaRevisa;
#	rdfs:range [rdfs:subClassOf schola:Scholastic, [a owl:Restriction; owl:onProperty schola:hasRole; owl:someValuesFrom schola:Reportator];
	rdfs:subPropertyOf knora-base:hasLinkTo;
	knora-base:subjectClassConstraint schola:LecturaRevisa;
	knora-base:objectClassConstraint schola:Scholastic.

schola:hasReportatorValue
	a owl:ObjectProperty;
	rdfs:label "has reportator - statement"@en, "hat Reportator - Festlegung"@de;
	rdfs:comment """Relating a scholastic lecture to a statement as reification of the relation between the lecture and a scholastic who reported it."""@en;
	rdfs:subPropertyOf knora-base:hasLinkToValue;
	knora-base:subjectClassConstraint schola:LecturaRevisa;
	knora-base:objectClassConstraint knora-base:LinkValue.

schola:isPartOfCommentary
	a owl:ObjectProperty;
	rdfs:label "is part of commentary "@en, "ist Teil eines Kommentars"@de;
	rdfs:comment """Relating a scholastic text structure to a scholastic commentary it is part of."""@en;
	rdfs:domain schola:Structure;
	rdfs:range schola:Commentary;
	rdfs:subPropertyOf text-structure:isPartOfTextExpression;
	knora-base:subjectClassConstraint schola:Structure;
	knora-base:objectClassConstraint schola:Commentary.

schola:isPartOfCommentaryValue
	a owl:ObjectProperty;
	rdfs:label "is part of commentary - statement"@en, "ist Teil eines Kommentars - Festlegung"@de;
	rdfs:comment """Relating a scholastic text structure to a statement as reification of the relation between the text and a commentary it is part of."""@en;
	rdfs:subPropertyOf text-structure:isPartOfTextExpressionValue;
	knora-base:subjectClassConstraint schola:Structure;
	knora-base:objectClassConstraint knora-base:LinkValue.

schola:isGlossOfCommentary
	a owl:ObjectProperty;
	rdfs:label "is gloss of commentary "@en, "ist Glosse eines Kommentars"@de;
	rdfs:comment """Relating a gloss to a scholastic commentary it is part of."""@en;
	rdfs:domain schola:Gloss;
	rdfs:range schola:Commentary;
	rdfs:subPropertyOf schola:isPartOfCommentary;
	knora-base:subjectClassConstraint schola:Gloss;
	knora-base:objectClassConstraint schola:Commentary.

schola:isGlossOfCommentaryValue
	a owl:ObjectProperty;
	rdfs:label "is gloss of commentary - statement"@en, "ist Glosse eines Kommentars - Festlegung"@de;
	rdfs:comment """Relating a gloss to a statement as reification of the relation between the gloss and a scholastic commentary it is part of."""@en;
	rdfs:subPropertyOf schola:isPartOfCommentaryValue;
	knora-base:subjectClassConstraint schola:Gloss;
	knora-base:objectClassConstraint knora-base:LinkValue.

schola:isVerseOfCommentary
	a owl:ObjectProperty;
	rdfs:label "is verse of commentary "@en, "ist Vers eines Kommentars"@de;
	rdfs:comment """Relating a verse to a scholastic commentary it is part of."""@en;
	rdfs:domain schola:Verse;
	rdfs:range schola:Commentary;
	rdfs:subPropertyOf schola:isPartOfCommentary;
	knora-base:subjectClassConstraint schola:Verse;
	knora-base:objectClassConstraint schola:Commentary.

schola:isVerseOfCommentaryValue
	a owl:ObjectProperty;
	rdfs:label "is verse of commentary - statement"@en, "ist Vers eines Kommentars - Festlegung"@de;
	rdfs:comment """Relating a verse to a statement as reification of the relation between the verse and a scholastic commentary it is part of."""@en;
	rdfs:subPropertyOf schola:isPartOfCommentaryValue;
	knora-base:subjectClassConstraint schola:Verse;
	knora-base:objectClassConstraint knora-base:LinkValue.

schola:isTableOfCommentary
	a owl:ObjectProperty;
	rdfs:label "is table of commentary "@en, "ist Tabelle eines Kommentars"@de;
	rdfs:comment """Relating a table to a scholastic commentary it is part of."""@en;
	rdfs:domain schola:Table;
	rdfs:range schola:Commentary;
	rdfs:subPropertyOf schola:isPartOfCommentary;
	knora-base:subjectClassConstraint schola:Table;
	knora-base:objectClassConstraint schola:Commentary.

schola:isTableOfCommentaryValue
	a owl:ObjectProperty;
	rdfs:label "is table of commentary - statement"@en, "ist Tabelle eines Kommentars - Festlegung"@de;
	rdfs:comment """Relating a table to a statement as reification of the relation between the table and a scholastic commentary it is part of."""@en;
	rdfs:subPropertyOf schola:isPartOfCommentaryValue;
	knora-base:subjectClassConstraint schola:Table;
	knora-base:objectClassConstraint knora-base:LinkValue.

schola:isQuestionOfCommentary
	a owl:ObjectProperty;
	rdfs:label "is question of commentary "@en, "ist Frage eines Kommentars"@de;
	rdfs:comment """Relating a question to a scholastic commentary it is part of."""@en;
	rdfs:domain schola:Question;
	rdfs:range schola:SentenceCommentary;
	rdfs:subPropertyOf schola:isPartOfCommentary;
	knora-base:subjectClassConstraint schola:Question;
	knora-base:objectClassConstraint schola:SentenceCommentary.

schola:isQuestionOfCommentaryValue #**
	a owl:ObjectProperty;
	rdfs:label "is question of commentary - statement"@en, "ist Frage eines Kommentars - Festlegung"@de;
	rdfs:comment """Relating a question to a statement as reification of the relation between the question and a commentary it is part of."""@en;
	rdfs:subPropertyOf schola:isPartOfCommentaryValue;
	knora-base:subjectClassConstraint schola:Question;
	knora-base:objectClassConstraint knora-base:LinkValue.

schola:isConclusionOfCommentary
	a owl:ObjectProperty;
	rdfs:label "is conclusion of commentary "@en, "ist Konklusion eines Kommentars"@de;
	rdfs:comment """Relating a conclusion to a scholastic commentary it is part of."""@en;
	rdfs:domain schola:Conclusion;
	rdfs:range schola:SentenceCommentary;
	rdfs:subPropertyOf schola:isPartOfCommentary;
	knora-base:subjectClassConstraint schola:Conclusion;
	knora-base:objectClassConstraint schola:SentenceCommentary.

schola:isConclusionOfCommentaryValue
	a owl:ObjectProperty;
	rdfs:label "is conclusion of commentary - statement"@en, "ist Konklusion eines Kommentars - Festlegung"@de;
	rdfs:comment """Relating a conclusion to a statement as reification of the relation between the conclusion and a commentary it is part of."""@en;
	rdfs:subPropertyOf schola:isPartOfCommentaryValue;
	knora-base:subjectClassConstraint schola:Conclusion;
	knora-base:objectClassConstraint knora-base:LinkValue.

schola:isSyllogismOfCommentary
	a owl:ObjectProperty;
	rdfs:label "is syllogism of commentary "@en, "ist Syllogismus eines Kommentars"@de;
	rdfs:comment """Relating a syllogism to a scholastic commentary it is part of."""@en;
	rdfs:domain schola:Syllogism;
	rdfs:range schola:SentenceCommentary;
	rdfs:subPropertyOf schola:isPartOfCommentary;
	knora-base:subjectClassConstraint schola:Syllogism;
	knora-base:objectClassConstraint schola:SentenceCommentary.

schola:isSyllogismOfCommentaryValue #**
	a owl:ObjectProperty;
	rdfs:label "is syllogism of commentary - statement"@en, "ist Syllogismus eines Kommentars - Festlegung"@de;
	rdfs:comment """Relating a syllogism to a statement as reification of the relation between the syllogism and a scholastic commentary it is part of."""@en;
	rdfs:subPropertyOf schola:isPartOfCommentaryValue;
	knora-base:subjectClassConstraint schola:Syllogism;
	knora-base:objectClassConstraint knora-base:LinkValue.