@prefix rdfs: <http://www.w3.org/2000/01/rdf-schema#>.
@prefix owl: <http://www.w3.org/2002/07/owl#>.
@prefix xsd: <http://www.w3.org/2001/XMLSchema#>.
@prefix skos: <http://www.w3.org/2004/02/skos/core#>.
@prefix dct: <http://purl.org/dc/terms/>.
@prefix foaf: <http://xmlns.com/foaf/0.1/>.
@prefix cidoc: <http://www.cidoc-crm.org/cidoc-crm/>.
@prefix frbroo: <http://iflastandards.info/ns/fr/frbr/frbroo/>.
@prefix event: <http://www.knora.org/ontology/event#>.
@prefix human: <http://www.knora.org/ontology/human#>.
@prefix language: <http://www.knora.org/ontology/language#>.
@prefix concept: <http://www.knora.org/ontology/concept#>.
@prefix text: <http://www.knora.org/ontology/text#>.
@prefix textedit: <http://www.knora.org/ontology/text-editing#>.
@prefix infocar: <http://www.knora.org/ontology/information-carrier#>.
@prefix publish: <http://www.knora.org/ontology/publishing#>.
@prefix litera: <http://www.knora.org/ontology/literature#>.
@prefix knora-base: <http://www.knora.org/ontology/knora-base#>.
@prefix salsah-gui: <http://www.knora.org/ontology/salsah-gui#>.
@prefix text-structure: <http://www.knora.org/ontology/text-structure#>.

<http://www.knora.org/ontology/text-structure>
	a owl:Ontology;
	dct:title "An ontology about text structure"@en;
	dct:description """Formal description of text structure, subclasses, related classes, and properties."""@en;
	skos:note """Text and editing are described in seperate ontologies"""@en;
	dct:creator "Hans Cools, software developer, NIE-INE, Basel University, Switzerland"@en;
	dct:contributor "Roberta Padlina, tool coordinator, NIE-INE, Basel University, Switzerland"@en;
	dct:publisher "Basel University, Switzerland"@en.

#
# CLASSES
#

text-structure:Structure
	a owl:Class;
	rdfs:label "text structure"@en, "Textstruktur"@de;
	rdfs:comment """Human natural language expression as structure, e.g. a sentence, text line, paragraph, verse, strophe."""@en;
	skos:note """Making up a text expression, without necessarily being one itself."""@en;
	rdfs:subClassOf language:HumanNaturalLanguageExpression, [
		a owl:Restriction; owl:onProperty text-structure:structureHasUnit; owl:minCardinality "0"^^xsd:nonNegativeInteger], [
		a owl:Restriction; owl:onProperty text-structure:structureHasUnitValue; owl:minCardinality "0"^^xsd:nonNegativeInteger].

text-structure:SyntacticStructure
	a owl:Class;
	rdfs:label "syntactic text structure"@en, "syntaktische Textstruktur"@de;
	rdfs:comment """Text structure depending on natural language-specific grammar, e.g. a sentence."""@en;
	rdfs:subClassOf text-structure:Structure.

text-structure:CompositionalStructure
	a owl:Class;
	rdfs:label "compositional text structure"@en, "kompositionelle Textstruktur"@de;
	rdfs:comment """Text structure depending on text composition in a two-dimensional plane, e.g. a header, line, paragraph, page, chapter."""@en;
	rdfs:subClassOf text-structure:Structure.

text-structure:ProsodicStructure
	a owl:Class;
	rdfs:label "prosodic text structure"@en, "prosodische Textstruktur"@de;
	rdfs:comment """Text structure depending on prosody, i.e. metre as basic rhythmic structure, rhyme and syllable."""@en;
	rdfs:subClassOf text-structure:Structure.

text-structure:Sentence
	a owl:Class;
	rdfs:label "sentence"@en, "Satz"@de;
	rdfs:comment """Syntactic structure unit as one or more linked words, typically a subject and predicate."""@en; #* more generic?
	rdfs:subClassOf text-structure:SyntacticStructure.

text-structure:Prose
	a owl:Class;
	rdfs:label "prose"@en, "Prosa"@de;
	rdfs:comment """Syntactic structure with a sentence as unit, in a natural flow of speech."""@en; #*
	rdfs:subClassOf text-structure:SyntacticStructure, [
		a owl:Restriction; owl:onProperty text-structure:structureHasUnit; owl:allValuesFrom text-structure:Sentence].

# text-structure:WrittenSentence: orthographic element: one or more words starting with a capital letter and ending in a full stop or period, question mark, or exclamation mark

text-structure:Line
	a owl:Class;
	rdfs:label "text line"@en, "Textzeile"@de;
	rdfs:comment """Text structure composed as a line."""@en;
	rdfs:subClassOf text-structure:CompositionalStructure, [
		a owl:Restriction; owl:onProperty text-structure:isLineOf; owl:allValuesFrom text:Expression], [
		a owl:Restriction; owl:onProperty text-structure:isLineOf; owl:minCardinality "0"^^xsd:nonNegativeInteger], [
		a owl:Restriction; owl:onProperty text-structure:isLineOfValue; owl:minCardinality "0"^^xsd:nonNegativeInteger].

text-structure:Paragraph
	a owl:Class;
	rdfs:label "paragraph"@en, "Paragraf"@de;
	rdfs:comment """Group of text lines."""@en;
	rdfs:subClassOf text-structure:CompositionalStructure, [
		a owl:Restriction; owl:onProperty text-structure:isParagraphOf; owl:allValuesFrom text:Expression], [
		a owl:Restriction; owl:onProperty text-structure:isParagraphOf; owl:minCardinality "0"^^xsd:nonNegativeInteger], [
		a owl:Restriction; owl:onProperty text-structure:isParagraphOfValue; owl:minCardinality "0"^^xsd:nonNegativeInteger], [
		a owl:Restriction; owl:onProperty text-structure:structureHasUnit; owl:allValuesFrom text-structure:Line].

#* text-structure:Chapter - Kapitel

#* section - Abschnitt: useful?

#* Absatz: useful?

#* running text - Fliesstext, as distinguished from headline, illustration, table

# text-structure:Cycle
#	a owl:Class;
#	rdfs:label "text cycle"@en, "Text-Zyklus"@de;
#	rdfs:comment """Set of text expressions belonging together, e.g. created around a certain theme, and intended to be experienced in a certain sequence."""@en;
#	rdfs:subClassOf concept:Cycle, text-structure:Structure. #*

#* scenic text - Szenischer Text # drama

#* Sachtext-structure: e.g. Essay, Einleitung

text-structure:Verse
	a owl:Class;
	rdfs:label "verse"@en, "Vers"@de;
	rdfs:comment """Text line with prosody."""@en;
	rdfs:subClassOf text-structure:ProsodicStructure, text-structure:Line, [
		a owl:Restriction; owl:onProperty text-structure:isVerseOf; owl:minCardinality "0"^^xsd:nonNegativeInteger], [
		a owl:Restriction; owl:onProperty text-structure:isVerseOfValue; owl:minCardinality "0"^^xsd:nonNegativeInteger].

#* Place an ancient verse without line structure in a place-time

text-structure:Strophe #* OR stanza OR verse - Vers
	a owl:Class;
	rdfs:label "strophe"@en, "Strophe"@de;
	rdfs:comment """Paragraph of verses as part of a poem."""@en;
	skos:note """The lyriks of a song can be structured as a poem with strophes."""@en;
	rdfs:subClassOf text-structure:Paragraph, [
		a owl:Restriction; owl:onProperty text-structure:isStropheOf; owl:allValuesFrom litera:VersePoem], [ #*
		a owl:Restriction; owl:onProperty text-structure:isStropheOf; owl:minCardinality "0"^^xsd:nonNegativeInteger], [
		a owl:Restriction; owl:onProperty text-structure:isStropheOfValue; owl:minCardinality "0"^^xsd:nonNegativeInteger], [
		a owl:Restriction; owl:onProperty text-structure:structureHasUnit; owl:allValuesFrom text-structure:Verse].

text-structure:FreeVerse
	a owl:Class;
	rdfs:label "free verse"@en, "freie Vers"@de;
	rdfs:comment """Verse without a fixed prosody."""@en; #*
	rdfs:subClassOf text-structure:Verse.

#* text-structure:FixedVerse

text-structure:RhymingVerse
	a owl:Class;
	rdfs:label "rhyming verse"@en, "gereimter Vers"@de;
	rdfs:comment """Verse with a rhyme."""@en;
	rdfs:subClassOf text-structure:Verse.

text-structure:RhythmicProse #*
	a owl:Class;
	rdfs:label "rhythmic prose"@en, "rhythmische Prosa"@de;
	rdfs:comment """Prose structure with a meter."""@en; #*
	skos:note """Structure of a prose poem."""@en; #*
	rdfs:subClassOf text-structure:Prose.

text-structure:NoteStructure #* pers√∂nlich-situative Notate (Mischkategorie): Motivnotizen (listen), Tagebucheintragungen (notizen), Titellisten, Vorbemerkungen, Nachworte
	a owl:Class;
	rdfs:label "note structure"@en, "Notiz-Struktur"@de;
	rdfs:comment """Text with note structure, not having a unit such as a sentence."""@en; #* , or being grammatically correct ?
	rdfs:subClassOf text-structure:Structure.

text-structure:LetterStructure #*
	a owl:Class;
	rdfs:label "letter structure"@en, "Brief-Struktur"@de;
	rdfs:comment """Text with letter structure."""@en;
	rdfs:subClassOf text-structure:Structure. #* format

#
# PROPERTIES
#

text-structure:structureHasUnit
	a owl:ObjectProperty;
	rdfs:label "text structure has unit"@en, "Textstruktur hat Einheit"@de;
	rdfs:comment """Relating a text structure to its unit."""@en;
	rdfs:subPropertyOf knora-base:hasLinkTo;
	knora-base:subjectClassConstraint text-structure:Structure;
	knora-base:objectClassConstraint text-structure:StructureUnit.

text-structure:structureHasUnitValue
	a owl:ObjectProperty;
	rdfs:label "text structure has unit - statement"@en, "Textstruktur hat Einheit - Festlegung"@de;
	rdfs:comment """Relating a text structure to a reification statement of the relation between the text structure and its unit."""@en;
	rdfs:subPropertyOf knora-base:hasLinkToValue;
	knora-base:subjectClassConstraint text-structure:Structure;
	knora-base:objectClassConstraint knora-base:LinkValue.

text-structure:isLineOf
	a owl:ObjectProperty;
	rdfs:label "is text line of"@en, "ist Textzeile von"@de;
	rdfs:comment """Relating a text line to a text it is part of."""@en;
	rdfs:domain text-structure:Line;
	rdfs:range text:Expression;
	rdfs:subPropertyOf concept:isPartOf;
	knora-base:subjectClassConstraint text-structure:Line;
	knora-base:objectClassConstraint text:Expression.

text-structure:isLineOfValue
	a owl:ObjectProperty;
	rdfs:label "is text line of - statement"@en, "ist Textzeile von - Festlegung"@de;
	rdfs:comment """Relating a text line to a reification statement of the relation between the line and a text it is part of."""@en;
	rdfs:subPropertyOf concept:isPartOfValue;
	knora-base:subjectClassConstraint text-structure:Line;
	knora-base:objectClassConstraint knora-base:LinkValue.

text-structure:hasLineNumber
	a owl:ObjectProperty;
	rdfs:label "has line number"@en, "hat Liniennummer"@de;
	rdfs:comment """Relating a text expression to the number (as object) of a line thereof."""@en;
	rdfs:subPropertyOf text:hasContent;
	knora-base:subjectClassConstraint text:Expression;
	knora-base:objectClassConstraint knora-base:TextValue;
	salsah-gui:guiElement salsah-gui:Richtext.

text-structure:isVerseOf
	a owl:ObjectProperty;
	rdfs:label "is verse of"@en, "ist Vers von"@de;
#*	rdfs:comment """Relating a verse to a poem it is part of."""@en;
	rdfs:domain text-structure:Verse;
#*	rdfs:range [owl:disjointUnionOf (litera:VersePoem litera:VerseNovel)];
	rdfs:subPropertyOf text-structure:isLineOf;
	knora-base:subjectClassConstraint text-structure:Verse;
	knora-base:objectClassConstraint litera:Poem. #*

text-structure:isVerseOfValue
	a owl:ObjectProperty;
	rdfs:label "is verse of - statement"@en, "ist Vers von - Festlegung"@de;
#*	rdfs:comment """Relating a verse to a reification statement of the relation between the verse and a poem it is part of."""@en;
	rdfs:subPropertyOf text-structure:isLineOfValue;
	knora-base:subjectClassConstraint text-structure:Verse;
	knora-base:objectClassConstraint knora-base:LinkValue.

text-structure:isParagraphOf
	a owl:ObjectProperty;
	rdfs:label "is paragraph of"@en, "ist Paragraf von"@de;
	rdfs:comment """Relating a paragraph to a text it is part of."""@en;
	rdfs:domain text-structure:Paragraph;
	rdfs:range text:Expression;
	rdfs:subPropertyOf concept:isPartOf;
	knora-base:subjectClassConstraint text-structure:Paragraph;
	knora-base:objectClassConstraint text:Expression.

text-structure:isParagraphOfValue
	a owl:ObjectProperty;
	rdfs:label "is paragraph of - statement"@en, "ist Paragraf von - Festlegung"@de;
	rdfs:comment """Relating a paragraph to a reification statement of the relation between the paragraph and a text it is part of."""@en;
	rdfs:subPropertyOf concept:isPartOfValue;
	knora-base:subjectClassConstraint text-structure:Paragraph;
	knora-base:objectClassConstraint knora-base:LinkValue.

text-structure:isStropheOf
	a owl:ObjectProperty;
	rdfs:label "is strophe of"@en, "ist Strophe von"@de;
	rdfs:comment """Relating a strophe to a verse poem it is part of."""@en;
	rdfs:domain text-structure:Strophe;
	rdfs:range litera:VersePoem;
	rdfs:subPropertyOf text-structure:isParagraphOf;
	knora-base:subjectClassConstraint text-structure:Strophe;
	knora-base:objectClassConstraint litera:VersePoem.

text-structure:isStropheOfValue
	a owl:ObjectProperty;
	rdfs:label "is strophe of - statement"@en, "ist Strophe von - Festlegung"@de;
	rdfs:comment """Relating a strophe to a reification statement of the relation between the strophe and a verse poem it is part of."""@en;
	rdfs:subPropertyOf text-structure:isParagraphOfValue;
	knora-base:subjectClassConstraint text-structure:Strophe;
	knora-base:objectClassConstraint knora-base:LinkValue.

text-structure:hasStrophe # check usefulness of this inverse property, NOT of inverse property in general
	a owl:ObjectProperty;
	rdfs:label "has strophe"@en, "hat Strophe"@de;
	rdfs:comment """Relating a verse poem to a strophe it contains."""@en;
	rdfs:domain litera:VersePoem;
	rdfs:range text-structure:Strophe;
	rdfs:subPropertyOf knora-base:hasLinkTo; #* text-structure:hasParagraph
	owl:inverseOf text-structure:isStropheOf;
	knora-base:subjectClassConstraint litera:VersePoem;
	knora-base:objectClassConstraint text-structure:Strophe.

text-structure:hasStropheValue
	a owl:ObjectProperty;
	rdfs:label "has strophe - statement"@en, "hat Strophe - Festlegung"@de;
	rdfs:comment """Relating a verse poem to a reification statement of the relation between the verse poem and a strophe it contains."""@en;
	rdfs:subPropertyOf knora-base:hasLinkTo; #* text-structure:hasParagraphValue
	knora-base:subjectClassConstraint litera:VersePoem;
	knora-base:objectClassConstraint knora-base:LinkValue.