@prefix rdfs: <http://www.w3.org/2000/01/rdf-schema#>.
@prefix owl: <http://www.w3.org/2002/07/owl#>.
@prefix xsd: <http://www.w3.org/2001/XMLSchema#>.
@prefix skos: <http://www.w3.org/2004/02/skos/core#>.
@prefix dct: <http://purl.org/dc/terms/>.
@prefix foaf: <http://xmlns.com/foaf/0.1/>.
@prefix cidoc: <http://www.cidoc-crm.org/cidoc-crm/>.
@prefix frbroo: <http://iflastandards.info/ns/fr/frbr/frbroo/>.
@prefix event: <http://www.knora.org/ontology/event#>.
@prefix human: <http://www.knora.org/ontology/human#>.
@prefix lang: <http://www.knora.org/ontology/language#>.
@prefix concept: <http://www.knora.org/ontology/concept#>.
@prefix textedit: <http://www.knora.org/ontology/text-editing#>.
@prefix infocar: <http://www.knora.org/ontology/information-carrier#>.
@prefix publish: <http://www.knora.org/ontology/publishing#>.
@prefix litera: <http://www.knora.org/ontology/literature#>.
@prefix knora-base: <http://www.knora.org/ontology/knora-base#>.
@prefix salsah-gui: <http://www.knora.org/ontology/salsah-gui#>.
@prefix text: <http://www.knora.org/ontology/text#>.

<http://www.knora.org/ontology/text>
	a owl:Ontology;
	dct:title "An ontology about text"@en;
	dct:description """Formal description of text in broadest sense, general subclasses, related classes, and properties."""@en;
	skos:note """Text editing is described in a seperate ontology"""@en;
	dct:creator "Hans Cools, software developer, NIE-INE, Basel University, Switzerland"@en;
	dct:contributor "Roberta Padlina, tool coordinator, NIE-INE, Basel University, Switzerland"@en;
	dct:publisher "Basel University, Switzerland"@en.
#	skos:note """Representation of an otherwise literal data element as object ('objectivation') enabling relating it to metadata"""@en.

#
# CLASSES
#

text:Expression
	a owl:Class;
	rdfs:label "text expression"@en, "Text-Expression"@de;
	rdfs:comment """Text as a human luinguistic expression."""@en;
	rdfs:subClassOf concept:Expression, lang:HumanNaturalLanguageExpression, [
		a owl:Restriction; owl:onProperty text:hasAuthor; owl:minCardinality "0"^^xsd:nonNegativeInteger], [
		a owl:Restriction; owl:onProperty text:hasAuthorValue; owl:minCardinality "0"^^xsd:nonNegativeInteger], [
		a owl:Restriction; owl:onProperty text:hasRevisor; owl:minCardinality "0"^^xsd:nonNegativeInteger], [
		a owl:Restriction; owl:onProperty text:hasRevisorValue; owl:minCardinality "0"^^xsd:nonNegativeInteger], [
		a owl:Restriction; owl:onProperty text:hasGlossator; owl:minCardinality "0"^^xsd:nonNegativeInteger], [
		a owl:Restriction; owl:onProperty text:hasGlossatorValue; owl:minCardinality "0"^^xsd:nonNegativeInteger], [
		a owl:Restriction; owl:onProperty text:hasAbbreviator; owl:minCardinality "0"^^xsd:nonNegativeInteger], [
		a owl:Restriction; owl:onProperty text:hasAbbreviatorValue; owl:minCardinality "0"^^xsd:nonNegativeInteger], [
		a owl:Restriction; owl:onProperty text:hasCopyist; owl:minCardinality "0"^^xsd:nonNegativeInteger], [
		a owl:Restriction; owl:onProperty text:hasCopyistValue; owl:minCardinality "0"^^xsd:nonNegativeInteger], [
		a owl:Restriction; owl:onProperty text:hasContent; owl:minCardinality "0"^^xsd:nonNegativeInteger], [
		a owl:Restriction; owl:onProperty text:hasStructure; owl:minCardinality "0"^^xsd:nonNegativeInteger], [
		a owl:Restriction; owl:onProperty text:hasStructureValue; owl:minCardinality "0"^^xsd:nonNegativeInteger], [
		a owl:Restriction; owl:onProperty text:hasIncipit; owl:minCardinality "0"^^xsd:nonNegativeInteger], [
		a owl:Restriction; owl:onProperty text:hasExplicit; owl:minCardinality "0"^^xsd:nonNegativeInteger], [
		a owl:Restriction; owl:onProperty text:hasPageIndicator; owl:minCardinality "0"^^xsd:nonNegativeInteger], [
		a owl:Restriction; owl:onProperty text:hasPageNumberIndicator; owl:minCardinality "0"^^xsd:nonNegativeInteger], [
		a owl:Restriction; owl:onProperty text:hasColumnIndicator; owl:minCardinality "0"^^xsd:nonNegativeInteger], [
		a owl:Restriction; owl:onProperty text:hasLineNumber; owl:minCardinality "0"^^xsd:nonNegativeInteger], [
		a owl:Restriction; owl:onProperty text:hasVersionIndicator; owl:minCardinality "0"^^xsd:nonNegativeInteger], [
		a owl:Restriction; owl:onProperty text:hasReferenceText; owl:minCardinality "0"^^xsd:nonNegativeInteger], [
		a owl:Restriction; owl:onProperty text:hasReferenceTextValue; owl:minCardinality "0"^^xsd:nonNegativeInteger], [
		a owl:Restriction; owl:onProperty textedit:hasEditor; owl:minCardinality "0"^^xsd:nonNegativeInteger], [
		a owl:Restriction; owl:onProperty textedit:hasEditorValue; owl:minCardinality "0"^^xsd:nonNegativeInteger], [
		a owl:Restriction; owl:onProperty textedit:hasRedactor; owl:minCardinality "0"^^xsd:nonNegativeInteger], [
		a owl:Restriction; owl:onProperty textedit:hasRedactorValue; owl:minCardinality "0"^^xsd:nonNegativeInteger], [
		a owl:Restriction; owl:onProperty textedit:hasEdition; owl:minCardinality "0"^^xsd:nonNegativeInteger], [
		a owl:Restriction; owl:onProperty textedit:hasEditionValue; owl:minCardinality "0"^^xsd:nonNegativeInteger], [
		a owl:Restriction; owl:onProperty textedit:hasSameEditionAs; owl:minCardinality "0"^^xsd:nonNegativeInteger], [
		a owl:Restriction; owl:onProperty textedit:hasSameEditionAsValue; owl:minCardinality "0"^^xsd:nonNegativeInteger], [
		a owl:Restriction; owl:onProperty textedit:hasDiplomaticTranscription; owl:minCardinality "0"^^xsd:nonNegativeInteger], [
		a owl:Restriction; owl:onProperty textedit:hasDiplomaticTranscriptionValue; owl:minCardinality "0"^^xsd:nonNegativeInteger], [
		a owl:Restriction; owl:onProperty textedit:hasCriticalEdition; owl:minCardinality "0"^^xsd:nonNegativeInteger], [
		a owl:Restriction; owl:onProperty textedit:hasCriticalEditionValue; owl:minCardinality "0"^^xsd:nonNegativeInteger].

text:Author
	a owl:Class;
	rdfs:label "author"@en, "Autor"@de;
	rdfs:comment """Role of a person being responsible for a text."""@en;
	skos:note """Often an author is also the creator of a text."""@en;
	rdfs:subClassOf human:Role.

text:Revisor #* SCO editor
	a owl:Class;
	rdfs:label "revisor"@en, "Revisor"@de;
	rdfs:comment """Role of a person checking on certain aspects of a text."""@en;
	rdfs:subClassOf human:Role.

text:Glossator #* -> scholastic? Unlikely to be used in modern times?
	a owl:Class;
	rdfs:label "glossator"@la, "glossator"@en, "Glossator"@de;
	rdfs:comment """Role of a person adding texts or glosses to a text."""@en;
# 	substantial OR marginal texts e.g. in the margin or between lines
	rdfs:subClassOf human:Creator.

text:Abbreviator #* -> scholastic?
	a owl:Class;
	rdfs:label "abbreviator"@la, "abbreviator"@en, "Abkürzer"@de;
	rdfs:comment """Role of a person being responsible for a shortened version of a text."""@en; #*
	rdfs:subClassOf human:Creator.

text:Copyist #* -> scholastic? ~ handwriting
	a owl:Class;
	rdfs:label "scribes"@la, "copyist"@en, "Kopist"@de; # "scribe"@en, "Schreiber"@de;
	rdfs:comment """Role of a person copying text by writing."""@en;
	rdfs:subClassOf human:Creator.

text:Translator #* -> scholastic? ~ handwriting
	a owl:Class;
	rdfs:label "translator"@en, "Übersetzer"@de;
	rdfs:comment """Role of a person translating text by writing."""@en;
	rdfs:subClassOf lang:Translator, human:Creator.

text:WrittenText
	a owl:Class;
	rdfs:label "written text"@en, "geschriebener Text"@de;
	rdfs:comment """Text written by any method, e.g. manually, with an analogue or digital typewriter, or on a computer, abstracted from its carrier."""@en;
	rdfs:subClassOf lang:HumanNaturalLanguageExpression, [
		a owl:Restriction; owl:onProperty infocar:isWrittenWith; owl:minCardinality "0"^^xsd:nonNegativeInteger], [
		a owl:Restriction; owl:onProperty infocar:isWrittenWithValue; owl:minCardinality "0"^^xsd:nonNegativeInteger].

text:HandwrittenText
	a owl:Class;
	rdfs:label "handwritten text"@en, "handgeschriebener Text"@de;
	rdfs:comment """Text written by hand."""@en;
	rdfs:subClassOf text:WrittenText, [
		a owl:Restriction; owl:onProperty infocar:isInManuscript; owl:cardinality "1"^^xsd:nonNegativeInteger], [
		a owl:Restriction; owl:onProperty infocar:isInManuscriptValue; owl:cardinality "1"^^xsd:nonNegativeInteger].

text:TypewrittenText
	a owl:Class;
	rdfs:label "typewritten text"@en, "maschinengeschriebener Text"@de;
	rdfs:comment """Text written with a typewriter."""@en;
	rdfs:subClassOf text:WrittenText, [
		a owl:Restriction; owl:onProperty infocar:isInTypescript; owl:cardinality "1"^^xsd:nonNegativeInteger], [
		a owl:Restriction; owl:onProperty infocar:isInTypescriptValue; owl:cardinality "1"^^xsd:nonNegativeInteger], [
		a owl:Restriction; owl:onProperty infocar:isWrittenWith; owl:allValuesFrom text:Typewriter].

text:Structure
	a owl:Class;
	rdfs:label "text structure"@en, "Textstruktur"@de;
	rdfs:comment """Human natural language expression as structure, e.g. a sentence, text line, paragraph, verse, strophe."""@en;
	skos:note """Making up a text expression, without necessarily being one itself."""@en;
	rdfs:subClassOf lang:HumanNaturalLanguageExpression, [
		a owl:Restriction; owl:onProperty text:structureHasUnit; owl:minCardinality "0"^^xsd:nonNegativeInteger], [
		a owl:Restriction; owl:onProperty text:structureHasUnitValue; owl:minCardinality "0"^^xsd:nonNegativeInteger].

text:SyntacticStructure
	a owl:Class;
	rdfs:label "syntactic text structure"@en, "syntaktische Textstruktur"@de;
	rdfs:comment """Text structure depending on natural language-specific grammar, e.g. a sentence."""@en;
	rdfs:subClassOf text:Structure.

text:CompositionalStructure
	a owl:Class;
	rdfs:label "compositional text structure"@en, "kompositionelle Textstruktur"@de;
	rdfs:comment """Text structure depending on text composition in a two-dimensional plane, e.g. a header, line, paragraph, page, chapter."""@en;
	rdfs:subClassOf text:Structure.

text:ProsodicStructure
	a owl:Class;
	rdfs:label "prosodic text structure"@en, "prosodische Textstruktur"@de;
	rdfs:comment """Text structure depending on prosody, i.e. metre as basic rhythmic structure, rhyme and syllable."""@en;
	rdfs:subClassOf text:Structure.

text:Sentence
	a owl:Class;
	rdfs:label "sentence"@en, "Satz"@de;
	rdfs:comment """Syntactic structure unit as one or more linked words, typically a subject and predicate."""@en; #* more generic?
	rdfs:subClassOf text:SyntacticStructure.

text:Prose
	a owl:Class;
	rdfs:label "prose"@en, "Prosa"@de;
	rdfs:comment """Syntactic structure with a sentence as unit, in a natural flow of speech."""@en; #*
	rdfs:subClassOf text:SyntacticStructure, [
		a owl:Restriction; owl:onProperty text:structureHasUnit; owl:allValuesFrom text:Sentence].

# text:WrittenSentence: orthographic element: one or more words starting with a capital letter and ending in a full stop or period, question mark, or exclamation mark

text:Line
	a owl:Class;
	rdfs:label "text line"@en, "Textzeile"@de;
	rdfs:comment """Text structure composed as a line."""@en;
	rdfs:subClassOf text:CompositionalStructure, [
		a owl:Restriction; owl:onProperty text:isLineOf; owl:allValuesFrom text:Expression], [
		a owl:Restriction; owl:onProperty text:isLineOf; owl:minCardinality "0"^^xsd:nonNegativeInteger], [
		a owl:Restriction; owl:onProperty text:isLineOfValue; owl:minCardinality "0"^^xsd:nonNegativeInteger].

text:Paragraph
	a owl:Class;
	rdfs:label "paragraph"@en, "Paragraf"@de;
	rdfs:comment """Group of text lines."""@en;
	rdfs:subClassOf text:CompositionalStructure, [
		a owl:Restriction; owl:onProperty text:isParagraphOf; owl:allValuesFrom text:Expression], [
		a owl:Restriction; owl:onProperty text:isParagraphOf; owl:minCardinality "0"^^xsd:nonNegativeInteger], [
		a owl:Restriction; owl:onProperty text:isParagraphOfValue; owl:minCardinality "0"^^xsd:nonNegativeInteger], [
		a owl:Restriction; owl:onProperty text:structureHasUnit; owl:allValuesFrom text:Line].

#* text:Chapter - Kapitel

#* section - Abschnitt: useful?

#* Absatz: useful?

#* running text - Fliesstext, as distinguished from headline, illustration, table

# text:Cycle
#	a owl:Class;
#	rdfs:label "text cycle"@en, "Text-Zyklus"@de;
#	rdfs:comment """Set of text expressions belonging together, e.g. created around a certain theme, and intended to be experienced in a certain sequence."""@en;
#	rdfs:subClassOf concept:Cycle, text:Structure. #*

#* scenic text - Szenischer Text # drama

#* Sachtext: e.g. Essay, Einleitung

text:Verse
	a owl:Class;
	rdfs:label "verse"@en, "Vers"@de;
	rdfs:comment """Text line with prosody."""@en;
	rdfs:subClassOf text:ProsodicStructure, text:Line, [
		a owl:Restriction; owl:onProperty text:isVerseOf; owl:minCardinality "0"^^xsd:nonNegativeInteger], [
		a owl:Restriction; owl:onProperty text:isVerseOfValue; owl:minCardinality "0"^^xsd:nonNegativeInteger].

#* text:Verse: place an ancient verse without line structure in a place-time

text:Strophe #* OR stanza OR verse - Vers
	a owl:Class;
	rdfs:label "strophe"@en, "Strophe"@de;
	rdfs:comment """Paragraph of verses as part of a poem."""@en;
#	skos:note """The lyriks of a song can be structured as a poem with strophes."""@en;
	rdfs:subClassOf text:Paragraph, [
		a owl:Restriction; owl:onProperty text:isStropheOf; owl:allValuesFrom litera:VersePoem], [ #*
		a owl:Restriction; owl:onProperty text:isStropheOf; owl:minCardinality "0"^^xsd:nonNegativeInteger], [
		a owl:Restriction; owl:onProperty text:isStropheOfValue; owl:minCardinality "0"^^xsd:nonNegativeInteger], [
		a owl:Restriction; owl:onProperty text:structureHasUnit; owl:allValuesFrom text:Verse].

text:FreeVerse
	a owl:Class;
	rdfs:label "free verse"@en, "freie Vers"@de;
	rdfs:comment """Verse without a fixed prosody."""@en; #*
	rdfs:subClassOf text:Verse.

#* text:FixedVerse

text:RhymingVerse
	a owl:Class;
	rdfs:label "rhyming verse"@en, "gereimter Vers"@de;
	rdfs:comment """Verse with a rhyme."""@en;
	rdfs:subClassOf text:Verse.

text:RhythmicProse #*
	a owl:Class;
	rdfs:label "rhythmic prose"@en, "rhythmische Prosa"@de;
	rdfs:comment """Prose structure with a meter."""@en; #*
	skos:note """Structure of a prose poem."""@en;
	rdfs:subClassOf text:Structure.

text:NoteStructure #* persönlich-situative Notate (Mischkategorie): Motivnotizen (listen), Tagebucheintragungen (notizen), Titellisten, Vorbemerkungen, Nachworte
	a owl:Class;
	rdfs:label "note structure"@en, "Notiz-Struktur"@de;
	rdfs:comment """Text with note structure, not having a unit such as a sentence."""@en; #* , or being grammatically correct ?
	rdfs:subClassOf text:Structure.

text:DiaryEntry
	a owl:Class;
	rdfs:label "diary entry"@en, "Tagebucheintrag"@de;
	rdfs:comment """Periodical, usually daily description of a personal experience or observation written in a diary."""@en;
	rdfs:subClassOf text:Expression, [
		a owl:Restriction; owl:onProperty infocar:isInDiary; owl:minCardinality "0"^^xsd:nonNegativeInteger], [
		a owl:Restriction; owl:onProperty infocar:isInDiaryValue; owl:minCardinality "0"^^xsd:nonNegativeInteger], [
		a owl:Restriction; owl:onProperty infocar:hasDiaryEnteringDate; owl:minCardinality "0"^^xsd:nonNegativeInteger].

text:LetterExpression #*
	a owl:Class;
	rdfs:label "letter expression"@en, "Brief-Expression"@de;
	rdfs:comment """Text expression with a letter structure."""@en;
	rdfs:subClassOf text:Expression, [
		a owl:Restriction; owl:onProperty text:hasStructure; owl:someValuesFrom text:LetterStructure], [
		a owl:Restriction; owl:onProperty text:hasStructure; owl:minCardinality "0"^^xsd:nonNegativeInteger], [
		a owl:Restriction; owl:onProperty text:hasStructureValue; owl:minCardinality "0"^^xsd:nonNegativeInteger], [
		a owl:Restriction; owl:onProperty infocar:isInLetter; owl:cardinality "1"^^xsd:nonNegativeInteger], [
		a owl:Restriction; owl:onProperty infocar:isInLetterValue; owl:cardinality "1"^^xsd:nonNegativeInteger].

text:LetterStructure #*
	a owl:Class;
	rdfs:label "letter structure"@en, "Brief-Struktur"@de;
	rdfs:comment """Text with letter structure."""@en;
	rdfs:subClassOf text:Structure. #* format

text:Commentary
	a owl:Class;
	rdfs:label "commentary"@en, "Kommentar"@de;
	rdfs:comment """Text expression in the form of a series of comments as analysis, interpretation or explanation of something, especially another textual expression."""@en;
	rdfs:subClassOf text:Expression.

text:Draft
	a owl:Class;
	rdfs:label "draft"@en, "Entwurf"@de;
	rdfs:comment """Developmental text expression."""@en;
	rdfs:subClassOf human:CreationVersion.

# genetic eiditon: description of ed of another

# Transcription: 1-1 copy of written text, OCR
# info: reader able to judge choices

text:Development
	a owl:Class;
	rdfs:label "text development"@en, "Text-Entwicklung"@de;
	rdfs:comment """Action wherein a person(s) creates text resulting in different manifestation, e.g. from notebook to manuscript to typescript to published print."""@en;
	rdfs:subClassOf human:Creating, [
		a owl:Restriction; owl:onProperty event:hasStage; owl:minCardinality "0"^^xsd:nonNegativeInteger], [
		a owl:Restriction; owl:onProperty event:hasStageValue; owl:minCardinality "0"^^xsd:nonNegativeInteger].

# extrinsic feature: carrier, typescript, system of signs diacritical eg. &
# intrinsic: formal content

#
# PROPERTIES
#

text:hasText
	a owl:ObjectProperty;
	rdfs:label "has text"@en, "hat Text"@de;
	rdfs:comment """Relating a resource to a text (as object) as a writable coherent set of signs representing semantics in a language."""@en;
	rdfs:subPropertyOf knora-base:hasValue;
	knora-base:subjectClassConstraint knora-base:Resource;
	knora-base:objectClassConstraint knora-base:TextValue;
	salsah-gui:guiElement salsah-gui:Richtext.

text:hasName
	a owl:ObjectProperty;
	rdfs:label "has name"@en, "hat Name"@de;
	rdfs:comment """Relating a resource to a name (as object) as a textual identifier of the resource."""@en;
	rdfs:domain rdfs:Resource;
	rdfs:range rdfs:Literal;
	rdfs:subPropertyOf text:hasText; # rdfs:label
	knora-base:subjectClassConstraint knora-base:Resource;
	knora-base:objectClassConstraint knora-base:TextValue;
	salsah-gui:guiElement salsah-gui:Richtext.

text:hasPreferredName
	a owl:ObjectProperty;
	rdfs:label "has preferred name"@en, "hat bevorzugter Name"@de;
	rdfs:comment """Relating a resource to a preferred name (as object)."""@en;
	rdfs:subPropertyOf text:hasName;
	knora-base:subjectClassConstraint knora-base:Resource;
	knora-base:objectClassConstraint knora-base:TextValue;
	salsah-gui:guiElement salsah-gui:Richtext.

text:hasAlias
	a owl:ObjectProperty;
	rdfs:label "has alias"@en, "hat Alias"@de;
	rdfs:comment """Relating a resource to an alias (as object) as an alternative name of the resource."""@en;
	rdfs:subPropertyOf text:hasName;
	knora-base:subjectClassConstraint knora-base:Resource;
	knora-base:objectClassConstraint knora-base:TextValue;
	salsah-gui:guiElement salsah-gui:Richtext.

text:hasIdentifier
	a owl:ObjectProperty;
	rdfs:label "has identifier"@en, "hat Kennzeichen"@de;
	rdfs:comment """Relating a resource to an identifier (as object) as a unique textual reference to the resource within a given context, and conforming to a formal identification system."""@en;
	rdfs:subPropertyOf text:hasText; # cidoc:E42_Identifier, cf. dcterms:identifier
	knora-base:subjectClassConstraint knora-base:Resource;
	knora-base:objectClassConstraint knora-base:TextValue;
	salsah-gui:guiElement salsah-gui:Richtext.

text:hasTitle
	a owl:ObjectProperty;
	rdfs:label "has title"@en, "hat Titel"@de;
	rdfs:comment """Relating a resource to a title (as object) as a textual identifier of the resource."""@en;
	rdfs:subPropertyOf text:hasText;
	knora-base:subjectClassConstraint knora-base:Resource;
	knora-base:objectClassConstraint knora-base:TextValue;
	salsah-gui:guiElement salsah-gui:Richtext.

text:hasComment
	a owl:ObjectProperty;
	rdfs:label "has comment"@en, "hat Kommentar"@de;
	rdfs:comment """Relating a resource to a comment (as object) as a textual statement about the resource."""@en;
	rdfs:subPropertyOf text:hasText;
	knora-base:subjectClassConstraint knora-base:Resource;
	knora-base:objectClassConstraint knora-base:TextValue;
	salsah-gui:guiElement salsah-gui:Richtext.

text:hasDescription
	a owl:ObjectProperty;
	rdfs:label "has description"@en, "hat Beschreibung"@de;
	rdfs:comment """Relating a resource to a description (as object) as a textual statement about features of the resource."""@en;
	rdfs:subPropertyOf text:hasText;
	knora-base:subjectClassConstraint knora-base:Resource;
	knora-base:objectClassConstraint knora-base:TextValue;
	salsah-gui:guiElement salsah-gui:Richtext.

text:hasDefinition
	a owl:ObjectProperty;
	rdfs:label "has definition"@en, "hat Definition"@de;
	rdfs:comment """Relating a resource to a definition (as object) as a textual statement about the essential features of the resource."""@en;
	rdfs:subPropertyOf text:hasDescription;
	knora-base:subjectClassConstraint knora-base:Resource;
	knora-base:objectClassConstraint knora-base:TextValue;
	salsah-gui:guiElement salsah-gui:Richtext.

text:hasDetailDescription
	a owl:ObjectProperty;
	rdfs:label "has detail description"@en, "hat Detail-Beschreibung"@de;
	rdfs:comment """Relating a resource to a description (as object) of its detail(s). E.g. in the case of a text a detail can be a passage variant or an emendation"""@en;
	rdfs:subPropertyOf text:hasDescription;
	knora-base:subjectClassConstraint knora-base:Resource;
	knora-base:objectClassConstraint knora-base:TextValue;
	salsah-gui:guiElement salsah-gui:Richtext.

text:hasSpecialDescription
	a owl:ObjectProperty;
	rdfs:label "has special description"@en, "hat Besonderes-Beschreibung"@de;
	rdfs:comment """Relating a resource to a description (as object) of (a) certain feature(s)."""@en;
	rdfs:subPropertyOf text:hasDescription;
	knora-base:subjectClassConstraint knora-base:Resource;
	knora-base:objectClassConstraint knora-base:TextValue;
	salsah-gui:guiElement salsah-gui:Richtext.

text:hasStructure
	a owl:ObjectProperty;
	rdfs:label "has structure"@en, "hat Struktur"@de;
	rdfs:comment """Relating a text expression to its structure."""@en;
	rdfs:subPropertyOf knora-base:hasLinkTo;
	knora-base:subjectClassConstraint text:Expression;
	knora-base:objectClassConstraint text:Structure.

text:hasStructureValue
	a owl:ObjectProperty;
	rdfs:label "has structure - statement"@en, "hat Struktur - Festlegung"@de;
	rdfs:comment """Relating a text expression to a reification statement of the relation between the text expression and its structure."""@en;
	rdfs:subPropertyOf knora-base:hasLinkToValue;
	knora-base:subjectClassConstraint text:Expression;
	knora-base:objectClassConstraint knora-base:LinkValue.

text:structureHasUnit
	a owl:ObjectProperty;
	rdfs:label "text structure has unit"@en, "Textstruktur hat Einheit"@de;
	rdfs:comment """Relating a text structure to its unit."""@en;
	rdfs:subPropertyOf knora-base:hasLinkTo;
	knora-base:subjectClassConstraint text:Structure;
	knora-base:objectClassConstraint text:StructureUnit.

text:structureHasUnitValue
	a owl:ObjectProperty;
	rdfs:label "text structure has unit - statement"@en, "Textstruktur hat Einheit - Festlegung"@de;
	rdfs:comment """Relating a text structure to a reification statement of the relation between the text structure and its unit."""@en;
	rdfs:subPropertyOf knora-base:hasLinkToValue;
	knora-base:subjectClassConstraint text:Structure;
	knora-base:objectClassConstraint knora-base:LinkValue.

text:hasIncipit
	a owl:ObjectProperty;
	rdfs:label "has incipit"@en, "hat Incipit"@de;
	rdfs:comment """Relating an untitled text expression to a beginning part thereof (as object) to identify the text."""@en;
	rdfs:subPropertyOf text:hasText;
	knora-base:subjectClassConstraint text:Expression;
	knora-base:objectClassConstraint knora-base:TextValue;
	salsah-gui:guiElement salsah-gui:Richtext.

text:hasExplicit
	a owl:ObjectProperty;
	rdfs:label "has explicit"@en, "hat Explicit"@de;
	rdfs:comment """Relating an untitled text expression to an end part thereof (as object) to identify the text."""@en;
	rdfs:subPropertyOf text:hasText;
	knora-base:subjectClassConstraint text:Expression;
	knora-base:objectClassConstraint knora-base:TextValue;
	salsah-gui:guiElement salsah-gui:Richtext.

text:hasContent
	a owl:ObjectProperty;
	rdfs:label "has content"@en, "hat Inhalt"@de;
	rdfs:comment """Relating a text expression to its content (as object)."""@en;
	rdfs:subPropertyOf text:hasText;
	knora-base:subjectClassConstraint text:Expression;
	knora-base:objectClassConstraint knora-base:TextValue;
	salsah-gui:guiElement salsah-gui:Richtext.

text:hasPageIndicator
	a owl:ObjectProperty;
	rdfs:label "has page indicator"@en, "hat Seite-Indikator"@de;
	rdfs:comment """Relating a text expression to a diacritical sign (as object) that indicates where a new page starts."""@en;
	rdfs:subPropertyOf text:hasDiacriticalSign;
	knora-base:subjectClassConstraint text:Derivative;
	knora-base:objectClassConstraint knora-base:TextValue;
	salsah-gui:guiElement salsah-gui:Richtext.

text:hasPageNumberIndicator
	a owl:ObjectProperty;
	rdfs:label "has page number indicator"@en, "hat Seitennummer-Indikator"@de;
	rdfs:comment """Relating a text expression to a diacritical sign (as object) that indicates the number of a new page."""@en;
	rdfs:subPropertyOf text:hasDiacriticalSign;
	knora-base:subjectClassConstraint text:Derivative;
	knora-base:objectClassConstraint knora-base:TextValue;
	salsah-gui:guiElement salsah-gui:Richtext.

text:hasColumnIndicator
	a owl:ObjectProperty;
	rdfs:label "has column indicator"@en, "hat Spalte-Indikator"@de;
	rdfs:comment """Relating a text expression to a diacritical sign (as object) that indicates where on a page a new column starts."""@en;
	rdfs:subPropertyOf text:hasDiacriticalSign;
	knora-base:subjectClassConstraint text:Derivative;
	knora-base:objectClassConstraint knora-base:TextValue;
	salsah-gui:guiElement salsah-gui:Richtext.

text:hasLineNumber
	a owl:ObjectProperty;
	rdfs:label "has line number"@en, "hat Liniennummer"@de;
	rdfs:comment """Relating a text expression to the number (as object) of a line thereof."""@en;
	rdfs:subPropertyOf text:hasContent;
	knora-base:subjectClassConstraint text:Expression;
	knora-base:objectClassConstraint knora-base:TextValue;
	salsah-gui:guiElement salsah-gui:Richtext.

text:hasVersionIndicator
	a owl:ObjectProperty;
	rdfs:label "has version indicator"@en, "hat Version-Indikator"@de;
	rdfs:comment """Relating a text expression to a textual element (as object) that indicates its version."""@en;
	rdfs:subPropertyOf text:hasContent;
	knora-base:subjectClassConstraint text:Expression;
	knora-base:objectClassConstraint knora-base:TextValue;
	salsah-gui:guiElement salsah-gui:Richtext.

text:hasAuthor #*
	a owl:ObjectProperty;
	rdfs:label "has author"@en, "hat Autor"@de;
	rdfs:comment """Relating a text to a person who authored it."""@en; # OR an Organisation that authored it -> foaf:Agent
#	skos:note """A text can have more than one author."""@en;
#	rdfs:domain text:Expression;
#	rdfs:range [rdfs:subClassOf human:Person, [a owl:Restriction; owl:onProperty event:hasRole; owl:someValuesFrom text:Author]];
	rdfs:subPropertyOf knora-base:hasLinkTo;
	knora-base:subjectClassConstraint text:Expression;
	knora-base:objectClassConstraint human:Person.

text:hasAuthorValue
	a owl:ObjectProperty;
	rdfs:label "has author - statement"@en, "hat Autor - Festlegung"@de;
	rdfs:comment """Relating a text to a reification statement of the relation between the text and a person who authored it."""@en;
	rdfs:subPropertyOf knora-base:hasLinkToValue;
	knora-base:subjectClassConstraint text:Expression;
	knora-base:objectClassConstraint knora-base:LinkValue.

#text:isAuthorOf
#	a owl:ObjectProperty;
#	rdfs:label "author of"@en;
#	rdfs:comment """Relating a person with author role to a text the person authored."""@en;
#	knora-base:subjectClassConstraint human:Person; # [rdfs:subClassOf human:Person, [a owl:Restriction; owl:onProperty event:hasRole; owl:someValuesFrom text:Author]];
#	knora-base:objectClassConstraint text:Expression.

text:hasRevisor
	a owl:ObjectProperty;
	rdfs:label "has revisor"@en, "hat Revisor"@de;
	rdfs:comment """Relating a text to a person who revised it."""@en;
#	rdfs:domain text:Expression;
#	rdfs:range [rdfs:subClassOf human:Person, [a owl:Restriction; owl:onProperty event:hasRole; owl:someValuesFrom text:Revisor]];
	rdfs:subPropertyOf knora-base:hasLinkTo;
	knora-base:subjectClassConstraint text:Expression;
	knora-base:objectClassConstraint human:Person.

text:hasRevisorValue
	a owl:ObjectProperty;
	rdfs:label "has revisor - statement"@en, "hat Revisor - Festlegung"@de;
	rdfs:comment """Relating a text to a reification statement of the relation between the text and a person who revised it."""@en;
	rdfs:subPropertyOf knora-base:hasLinkToValue;
	knora-base:subjectClassConstraint text:Expression;
	knora-base:objectClassConstraint knora-base:LinkValue.

text:hasGlossator
	a owl:ObjectProperty;
	rdfs:label "has glossator"@en, "hat Glossator"@de;
	rdfs:comment """Relating a text to a person who glossed it."""@en;
#	rdfs:domain text:Expression;
#	rdfs:range [rdfs:subClassOf human:Person, [a owl:Restriction; owl:onProperty event:hasRole; owl:someValuesFrom text:Glossator]];
	rdfs:subPropertyOf knora-base:hasLinkTo;
	knora-base:subjectClassConstraint text:Expression;
	knora-base:objectClassConstraint human:Person.

text:hasGlossatorValue
	a owl:ObjectProperty;
	rdfs:label "has glossator - statement"@en, "hat Glossator - Festlegung"@de;
	rdfs:comment """Relating a text to a reification statement of the relation between the text and a person who glossed it."""@en;
	rdfs:subPropertyOf knora-base:hasLinkToValue;
	knora-base:subjectClassConstraint text:Expression;
	knora-base:objectClassConstraint knora-base:LinkValue.

text:hasAbbreviator
	a owl:ObjectProperty;
	rdfs:label "has abbreviator"@en, "hat Abkurzer"@de;
	rdfs:comment """Relating a text to a person who abbreviated it."""@en;
#	rdfs:domain text:Expression;
#	rdfs:range [rdfs:subClassOf human:Person, [a owl:Restriction; owl:onProperty event:hasRole; owl:someValuesFrom text:Abbreviator]];
	rdfs:subPropertyOf knora-base:hasLinkTo;
	knora-base:subjectClassConstraint text:Expression;
	knora-base:objectClassConstraint human:Person.

text:hasAbbreviatorValue
	a owl:ObjectProperty;
	rdfs:label "has abbreviator - statement"@en, "hat Abkurzer - Festlegung"@de;
	rdfs:comment """Relating a text to a reification statement of the relation between the text and a person who abbreviated it."""@en;
	rdfs:subPropertyOf knora-base:hasLinkToValue;
	knora-base:subjectClassConstraint text:Expression;
	knora-base:objectClassConstraint knora-base:LinkValue.

text:hasCopyist
	a owl:ObjectProperty;
	rdfs:label "has copyist"@en, "hat Kopist"@de;
	rdfs:comment """Relating a text to a person who copied it by handwriting."""@en;
#	rdfs:domain text:Expression;
#	rdfs:range [rdfs:subClassOf human:Person, [a owl:Restriction; owl:onProperty event:hasRole; owl:someValuesFrom text:Copyist]];
	rdfs:subPropertyOf knora-base:hasLinkTo;
	knora-base:subjectClassConstraint text:Expression;
	knora-base:objectClassConstraint human:Person.

text:hasCopyistValue
	a owl:ObjectProperty;
	rdfs:label "has copyist - statement"@en, "hat Kopist - Festlegung"@de;
	rdfs:comment """Relating a text to a reification statement of the relation between the text and a person who copied it by handwriting."""@en;
	rdfs:subPropertyOf knora-base:hasLinkToValue;
	knora-base:subjectClassConstraint text:Expression;
	knora-base:objectClassConstraint knora-base:LinkValue.

text:isLineOf
	a owl:ObjectProperty;
	rdfs:label "is text line of"@en, "ist Textzeile von"@de;
	rdfs:comment """Relating a text line to a text it is part of."""@en;
	rdfs:domain text:Line;
	rdfs:range text:Expression;
	rdfs:subPropertyOf concept:isPartOf;
	knora-base:subjectClassConstraint text:Line;
	knora-base:objectClassConstraint text:Expression.

text:isLineOfValue
	a owl:ObjectProperty;
	rdfs:label "is text line of - statement"@en, "ist Textzeile von - Festlegung"@de;
	rdfs:comment """Relating a text line to a reification statement of the relation between the line and a text it is part of."""@en;
	rdfs:subPropertyOf concept:isPartOfValue;
	knora-base:subjectClassConstraint text:Line;
	knora-base:objectClassConstraint knora-base:LinkValue.

text:isVerseOf
	a owl:ObjectProperty;
	rdfs:label "is verse of"@en, "ist Vers von"@de;
#*	rdfs:comment """Relating a verse to a poem it is part of."""@en;
	rdfs:domain text:Verse;
#*	rdfs:range [owl:disjointUnionOf (litera:VersePoem litera:VerseNovel)];
	rdfs:subPropertyOf text:isLineOf;
	knora-base:subjectClassConstraint text:Verse;
	knora-base:objectClassConstraint litera:Poem. #*

text:isVerseOfValue
	a owl:ObjectProperty;
	rdfs:label "is verse of - statement"@en, "ist Vers von - Festlegung"@de;
#*	rdfs:comment """Relating a verse to a reification statement of the relation between the verse and a poem it is part of."""@en;
	rdfs:subPropertyOf text:isLineOfValue;
	knora-base:subjectClassConstraint text:Verse;
	knora-base:objectClassConstraint knora-base:LinkValue.

text:isParagraphOf
	a owl:ObjectProperty;
	rdfs:label "is paragraph of"@en, "ist Paragraf von"@de;
	rdfs:comment """Relating a paragraph to a text it is part of."""@en;
	rdfs:domain text:Paragraph;
	rdfs:range text:Expression;
	rdfs:subPropertyOf concept:isPartOf;
	knora-base:subjectClassConstraint text:Paragraph;
	knora-base:objectClassConstraint text:Expression.

text:isParagraphOfValue
	a owl:ObjectProperty;
	rdfs:label "is paragraph of - statement"@en, "ist Paragraf von - Festlegung"@de;
	rdfs:comment """Relating a paragraph to a reification statement of the relation between the paragraph and a text it is part of."""@en;
	rdfs:subPropertyOf concept:isPartOfValue;
	knora-base:subjectClassConstraint text:Paragraph;
	knora-base:objectClassConstraint knora-base:LinkValue.

text:isStropheOf
	a owl:ObjectProperty;
	rdfs:label "is strophe of"@en, "ist Strophe von"@de;
	rdfs:comment """Relating a strophe to a verse poem it is part of."""@en;
	rdfs:domain text:Strophe;
	rdfs:range litera:VersePoem;
	rdfs:subPropertyOf text:isParagraphOf;
	knora-base:subjectClassConstraint text:Strophe;
	knora-base:objectClassConstraint litera:VersePoem.

text:isStropheOfValue
	a owl:ObjectProperty;
	rdfs:label "is strophe of - statement"@en, "ist Strophe von - Festlegung"@de;
	rdfs:comment """Relating a strophe to a reification statement of the relation between the strophe and a verse poem it is part of."""@en;
	rdfs:subPropertyOf text:isParagraphOfValue;
	knora-base:subjectClassConstraint text:Strophe;
	knora-base:objectClassConstraint knora-base:LinkValue.

text:hasStrophe # check usefulness of inverse property
	a owl:ObjectProperty;
	rdfs:label "has strophe"@en, "hat Strophe"@de;
	rdfs:comment """Relating a verse poem to a strophe it contains."""@en;
	rdfs:domain litera:VersePoem;
	rdfs:range text:Strophe;
	rdfs:subPropertyOf knora-base:hasLinkTo; #* text:hasParagraph
	owl:inverseOf text:isStropheOf;
	knora-base:subjectClassConstraint text:VersePoem;
	knora-base:objectClassConstraint text:Strophe.

text:hasStropheValue
	a owl:ObjectProperty;
	rdfs:label "has strophe - statement"@en, "hat Strophe - Festlegung"@de;
	rdfs:comment """Relating a verse poem to a reification statement of the relation between the verse poem and a strophe it contains."""@en;
	rdfs:subPropertyOf knora-base:hasLinkTo; #* text:hasParagraphValue
	knora-base:subjectClassConstraint text:VersePoem;
	knora-base:objectClassConstraint knora-base:LinkValue.

text:hasReferenceText
	a owl:ObjectProperty;
	rdfs:label "has reference text"@en, "hat Bezugstext"@de;
	rdfs:comment "Relating a text to another one as its reference."@en;
	rdfs:subPropertyOf knora-base:hasLinkTo;
	knora-base:subjectClassConstraint text:Expression;
	knora-base:objectClassConstraint text:Expression.

text:hasReferenceTextValue
	a owl:ObjectProperty;
	rdfs:label "has reference text - statement"@en, "hat Bezugstext - Festlegung"@de;
	rdfs:comment "Relating a text to a reification statement of the relation between the text and another one as its reference."@en;
	rdfs:subPropertyOf knora-base:hasLinkToValue;
	knora-base:subjectClassConstraint text:Expression;
	knora-base:objectClassConstraint knora-base:LinkValue.