@prefix rdf: <http://www.w3.org/1999/02/22-rdf-syntax-ns#>.
@prefix rdfs: <http://www.w3.org/2000/01/rdf-schema#>.
@prefix owl: <http://www.w3.org/2002/07/owl#>.
@prefix xsd: <http://www.w3.org/2001/XMLSchema#>.
@prefix skos: <http://www.w3.org/2004/02/skos/core#>.
@prefix dct: <http://purl.org/dc/terms/>.
@prefix foaf: <http://xmlns.com/foaf/0.1/>.
@prefix cidoc: <http://www.cidoc-crm.org/cidoc-crm/>.
@prefix time: <http://www.nie.org/ontology/time#>.
@prefix event: <http://www.nie.org/ontology/event#>.
@prefix concept: <http://www.nie.org/ontology/concept#>.

@prefix calendar: <http://www.nie.org/ontology/calendar#>.

<http://www.nie.org/ontology/calendar>
	dct:issued "2019-12-28T13:45:00+01:00"^^xsd:dateTime;
	dct:license <http://creativecommons.org/licenses/by/3.0/>;
	dct:title "calendar-ontology"@en;
	dct:description """Formal description of calendar, subclasses, related classes, and properties."""@en;
	dct:creator "Hans Cools, MD, knowledge engineer, ontologist, software developer, NIE-INE, Basel University, Switzerland"@en;
	dct:publisher "Basel University, Switzerland"@en.

#
# CLASSES
#

calendar:Calendar
	rdfs:isDefinedBy <http://www.nie.org/ontology/calendar#>;
	a rdfs:Class;
	rdfs:label "calendar"@en, "Kalender"@de, "calendrier"@fr, "calendario"@it;
	rdfs:comment """System of reckoning time in which the beginning, length, and divisions of a year are defined, sometimes along with multiyear cycles."""@en;
	rdfs:subClassOf concept:Information.

calendar:JulianCalendar
	rdfs:isDefinedBy <http://www.nie.org/ontology/calendar#>;
	a rdfs:Class, calendar:Calendar; # OWL Full: class as instance
	rdfs:label "Julian calendar"@en, "julianischer Kalender"@de, "calendrier julien"@fr, "calendario juliano"@it;
	rdfs:comment """Calendar introduced in 46 BC in Rome by Julius Caesar. It is based on a solar year of 365 days. There are 12 months of 30 or 31 days, except for February, which has 28 days with the exception of every leap year when it has 29 days. Every fourth year and centenary year is a leap year of 366 days. The beginning of a year is not fixed on January 1. It was replaced by the Gregorian calendar in 1582 AD."""@en;
	skos:note """Has 365.25 days/year."""@en;
	skos:note """A year that is exactly divisible by four is a leap year, except for years that are exactly divisible by 100, but these centurial years are leap years if they are exactly divisible by 400. For example, the years 1700, 1800, and 1900 are not leap years, but the year 2000 is."""@en.

calendar:ProlepticJulianCalendar
	rdfs:isDefinedBy <http://www.nie.org/ontology/calendar#>;
	a rdfs:Class, calendar:Calendar;
	rdfs:label "proleptic Julian calendar"@en, "proleptischer julianischer Kalender"@de, "calendrier julien proleptique"@fr, "calendario juliano proleptico"@it;
	rdfs:comment """Produced by extending the Julian calendar backward to dates preceding its use in stable form from 4 AD on."""@en;
	skos:note """There is no proleptic Julian year 0. Year 1 BC is followed by year 1 AD."""@en.

calendar:GregorianCalendar
	rdfs:isDefinedBy <http://www.nie.org/ontology/calendar#>;
	a rdfs:Class, calendar:Calendar;
	rdfs:label "Gregorian calendar"@en, "gregorianischer Kalender"@de, "calendrier grégorien"@fr, "calendario gregoriano"@it;
	rdfs:comment """Calendar introduced on 15 October 1582 AD by Pope Gregory XIII, and a correction of the Julian calendar. It is based on a solar year of 365 days. Every fourth year is a leap year of 366 days except for centenary years not evenly divisible by 400."""@en;
	skos:note """Has 365.2425 days/year or or 365 days, 5 hours, 49 minutes and 12 seconds."""@en.

calendar:ProlepticGregorianCalendar
	rdfs:isDefinedBy <http://www.nie.org/ontology/calendar#>;
	a rdfs:Class, calendar:Calendar;
	rdfs:label "proleptic Gregorian calendar"@en, "proleptischer gregorianischer Kalender"@de, "calendrier grégorien proleptique"@fr, "calendario gregoriano proleptico"@it;
	rdfs:comment """Produced by extending the Gregorian calendar backward to dates preceding its introduction on 15 October 1582."""@en;
	skos:note """There is no proleptic Gregorian year 0. Year 1 BC is followed by year 1 AD."""@en.

#
# PROPERTIES
#

calendar:hasCalendar
	rdfs:isDefinedBy <http://www.nie.org/ontology/calendar#>;
	a owl:ObjectProperty;
	rdfs:label "has calendar"@en;
	rdfs:comment """Relating an event to a calendar."""@en;
	rdfs:domain event:Event; # [owl:disjointUnionOf (event:Event event:Output)];
	rdfs:range calendar:Calendar.

calendar:hasGregorianDateList
	rdfs:isDefinedBy <http://www.nie.org/ontology/calendar#>;
	a owl:ObjectProperty;
	rdfs:label "has Gregorian date list"@en;
	rdfs:comment """Relating something to its Gregorian date as a list of integers."""@en;
	skos:note """Used in an N3-rule to convert a Gregorian date list to a typed date literal and to a Julian Day Number."""@en;
	rdfs:domain rdfs:Resource;
	rdfs:range rdf:List.

calendar:hasGregorianDate
	rdfs:isDefinedBy <http://www.nie.org/ontology/calendar#>;
	a owl:DatatypeProperty;
	rdfs:label "has Gregorian date"@en;
	rdfs:comment """Relating something to its Gregorian date."""@en;
	rdfs:domain rdfs:Resource;
	rdfs:range xsd:date.

# [rdfs:subClassOf event:Output, [a owl:Restriction; owl:onProperty calendar:hasCalendar; owl:someValuesFrom calendar:GregorianCalendar]];
#	owl:propertyChainAxiom (event:isOutputOf time:hasOutputDateTime). #°

calendar:hasGregorianStartDateList
	rdfs:isDefinedBy <http://www.nie.org/ontology/calendar#>;
	a owl:ObjectProperty;
	rdfs:label "has Gregorian start date list"@en;
	rdfs:comment """Relating an event to its Gregorian start date as a list of integers."""@en;
	skos:note """Used in an N3-rule to convert an event with a Gregorian start date list to an event with a start Julian Day Number."""@en;
	rdfs:domain event:Event;
	rdfs:range rdf:List.

calendar:hasGregorianStartDate
	rdfs:isDefinedBy <http://www.nie.org/ontology/calendar#>;
	a owl:DatatypeProperty;
	rdfs:label "has Gregorian start date"@en;
	rdfs:comment """Relating an event to its Gregorian start date."""@en;
	rdfs:domain event:Event;
	rdfs:range xsd:date.

calendar:hasGregorianEndDateList
	rdfs:isDefinedBy <http://www.nie.org/ontology/calendar#>;
	a owl:ObjectProperty;
	rdfs:label "has Gregorian end date list"@en;
	rdfs:comment """Relating an event to its Gregorian end date as a list of integers."""@en;
	skos:note """Used in an N3-rule to convert an event with a Gregorian end date list to an event with an end Julian Day Number."""@en;
	rdfs:domain event:Event;
	rdfs:range rdf:List.

calendar:hasGregorianEndDate
	rdfs:isDefinedBy <http://www.nie.org/ontology/calendar#>;
	a owl:DatatypeProperty;
	rdfs:label "has Gregorian end date"@en;
	rdfs:comment """Relating an event to its Gregorian end date."""@en;
	rdfs:domain event:Event;
	rdfs:range xsd:date.

calendar:hasGregorianYear
	rdfs:isDefinedBy <http://www.nie.org/ontology/calendar#>;
	a owl:DatatypeProperty;
	rdfs:label "has Gregorian year"@en;
	rdfs:comment """Relating a Gregorian date list to its year."""@en;
	skos:note """Used in an N3-rule to derive the year from a Gregorian date or start date list."""@en;
	rdfs:domain rdf:List;
	rdfs:range xsd:positiveInteger.

calendar:hasJulianDateList
	rdfs:isDefinedBy <http://www.nie.org/ontology/calendar#>;
	a owl:ObjectProperty;
	rdfs:label "has Julian date list"@en;
	rdfs:comment """Relating something to its Julian date as a list of integers."""@en;
	skos:note """Used in an N3-rule to convert a Julian date list to a typed date literal and to a Julian Day Number."""@en;
	rdfs:domain rdfs:Resource;
	rdfs:range rdf:List.

calendar:hasJulianDate
	rdfs:isDefinedBy <http://www.nie.org/ontology/calendar#>;
	a owl:DatatypeProperty;
	rdfs:label "has Julian date"@en;
	rdfs:comment """Relating something to its Julian date."""@en;
	rdfs:domain rdfs:Resource;
	rdfs:range xsd:date.

calendar:hasJulianStartDateList
	rdfs:isDefinedBy <http://www.nie.org/ontology/calendar#>;
	a owl:ObjectProperty;
	rdfs:label "has Julian start date list"@en;
	rdfs:comment """Relating an event to its Julian start date as a list of integers."""@en;
	skos:note """Used in an N3-rule to convert an event with a Julian start date list to an event with a start Julian Day Number."""@en;
	rdfs:domain event:Event;
	rdfs:range rdf:List.

calendar:hasJulianStartDate
	rdfs:isDefinedBy <http://www.nie.org/ontology/calendar#>;
	a owl:DatatypeProperty;
	rdfs:label "has Julian start date"@en;
	rdfs:comment """Relating something to its Julian start date."""@en;
	rdfs:domain rdfs:Resource;
	rdfs:range xsd:date.

calendar:hasJulianEndDateList
	rdfs:isDefinedBy <http://www.nie.org/ontology/calendar#>;
	a owl:ObjectProperty;
	rdfs:label "has Julian end date list"@en;
	rdfs:comment """Relating an event to its Julian end date as a list of integers."""@en;
	skos:note """Used in an N3-rule to convert an event with a Julian end date list to an event with an end Julian Day Number."""@en;
	rdfs:domain event:Event;
	rdfs:range rdf:List.

calendar:hasJulianEndDate
	rdfs:isDefinedBy <http://www.nie.org/ontology/calendar#>;
	a owl:DatatypeProperty;
	rdfs:label "has Julian end date"@en;
	rdfs:comment """Relating something to its Julian end date."""@en;
	rdfs:domain rdfs:Resource;
	rdfs:range xsd:date.

calendar:hasJulianYear
	rdfs:isDefinedBy <http://www.nie.org/ontology/calendar#>;
	a owl:DatatypeProperty;
	rdfs:label "has Julian year"@en;
	rdfs:comment """Relating a Julian date list to its year."""@en;
	skos:note """Used in an N3-rule to derive the year from a Julian date or start date list."""@en;
	rdfs:domain rdf:List;
	rdfs:range xsd:positiveInteger.

calendar:hasProlepticJulianDateList
	rdfs:isDefinedBy <http://www.nie.org/ontology/calendar#>;
	a owl:ObjectProperty;
	rdfs:label "has proleptic Julian date list"@en;
	rdfs:comment """Relating something to its proleptic Julian date as a list of integers."""@en;
	skos:note """Used in an N3-rule to convert a proleptic Julian date list to a typed date literal and to a Julian Day Number."""@en;
	rdfs:domain rdfs:Resource;
	rdfs:range rdf:List.

calendar:hasProlepticJulianDate
	rdfs:isDefinedBy <http://www.nie.org/ontology/calendar#>;
	a owl:DatatypeProperty;
	rdfs:label "has proleptic Julian date"@en;
	rdfs:comment """Relating something to its proleptic Julian date."""@en;
	rdfs:domain rdfs:Resource;
	rdfs:range xsd:date.

calendar:hasProlepticJulianStartDateList
	rdfs:isDefinedBy <http://www.nie.org/ontology/calendar#>;
	a owl:ObjectProperty;
	rdfs:label "has proleptic Julian start date list"@en;
	rdfs:comment """Relating an event to its proleptic Julian start date as a list of integers."""@en;
	skos:note """Used in an N3-rule to convert an event with a proleptic Julian start date list to an event with a start Julian Day Number."""@en;
	rdfs:domain event:Event;
	rdfs:range rdf:List.

calendar:hasProlepticJulianStartDate
	rdfs:isDefinedBy <http://www.nie.org/ontology/calendar#>;
	a owl:DatatypeProperty;
	rdfs:label "has proleptic Julian start date"@en;
	rdfs:comment """Relating something to its proleptic Julian start date."""@en;
	rdfs:domain rdfs:Resource;
	rdfs:range xsd:date.

calendar:hasProlepticJulianEndDateList
	rdfs:isDefinedBy <http://www.nie.org/ontology/calendar#>;
	a owl:ObjectProperty;
	rdfs:label "has proleptic Julian end date list"@en;
	rdfs:comment """Relating an event to its proleptic Julian end date as a list of integers."""@en;
	skos:note """Used in an N3-rule to convert an event with a proleptic Julian end date list to an event with a start Julian Day Number."""@en;
	rdfs:domain event:Event;
	rdfs:range rdf:List.

calendar:hasProlepticJulianEndDate
	rdfs:isDefinedBy <http://www.nie.org/ontology/calendar#>;
	a owl:DatatypeProperty;
	rdfs:label "has proleptic Julian end date"@en;
	rdfs:comment """Relating something to its proleptic Julian end date."""@en;
	rdfs:domain rdfs:Resource;
	rdfs:range xsd:date.

calendar:hasProlepticJulianYear
	rdfs:isDefinedBy <http://www.nie.org/ontology/calendar#>;
	a owl:DatatypeProperty;
	rdfs:label "has proleptic Julian year"@en;
	rdfs:comment """Relating a proleptic Julian date list to its year."""@en;
	skos:note """Used in an N3-rule to derive the year from a proleptic Julian date or start date list."""@en;
	rdfs:domain rdf:List;
	rdfs:range xsd:positiveInteger.

calendar:hasJulianDayNumber
	rdfs:isDefinedBy <http://www.nie.org/ontology/calendar#>;
	a owl:DatatypeProperty;
	rdfs:label "has Julian Day Number"@en;
	rdfs:comment """Relating something to its Julian Day Number."""@en;
	rdfs:comment """The Julian Day Number (JDN) is the integer assigned to a whole solar day in the Julian day count starting from noon Universal time, with Julian Day Number 0 assigned to the day starting at noon on Monday, January 1, 4713 BC, proleptic Julian calendar (November 24, 4714 BC, in the proleptic Gregorian calendar), a date at which three multi-year cycles started (Indiction, Solar, and Lunar cycles) and which precedes any date in recorded human history."""@en;
	rdfs:domain rdfs:Resource;
	rdfs:range xsd:integer.

calendar:hasStartJulianDayNumber
	rdfs:isDefinedBy <http://www.nie.org/ontology/calendar#>;
	a owl:DatatypeProperty;
	rdfs:label "has start Julian Day Number"@en;
	rdfs:comment """Relating something to its start Julian Day Number."""@en;
	rdfs:domain event:Event;
	rdfs:range xsd:integer. # ; rdfs:subPropertyOf calendar:hasJulianDayNumber.

calendar:hasEndJulianDayNumber
	rdfs:isDefinedBy <http://www.nie.org/ontology/calendar#>;
	a owl:DatatypeProperty;
	rdfs:label "has end Julian Day Number"@en;
	rdfs:comment """Relating an event to its end Julian Day Number."""@en;
	rdfs:domain event:Event;
	rdfs:range xsd:integer. # ; rdfs:subPropertyOf calendar:hasJulianDayNumber.