@prefix rdfs: <http://www.w3.org/2000/01/rdf-schema#>.
@prefix owl: <http://www.w3.org/2002/07/owl#>.
@prefix xsd: <http://www.w3.org/2001/XMLSchema#>.
@prefix skos: <http://www.w3.org/2004/02/skos/core#>.
@prefix dct: <http://purl.org/dc/terms/>.
@prefix foaf: <http://xmlns.com/foaf/0.1/>.
@prefix unicore: <http://purl.uniprot.org/core/>.
@prefix cidoc: <http://www.cidoc-crm.org/cidoc-crm/>.
@prefix frbroo: <http://iflastandards.info/ns/fr/frbr/frbroo/>.
@prefix event: <http://www.nie.org/ontology/shared/event#>.
@prefix physical: <http://www.nie.org/ontology/shared/physical-entity#>.
@prefix agent: <http://www.nie.org/ontology/shared/agent#>.
@prefix human: <http://www.nie.org/ontology/shared/human#>.
@prefix creating: <http://www.nie.org/ontology/shared/creating#>.
@prefix infocar: <http://www.nie.org/ontology/shared/information-carrier#>.

# @base <http://www.nie.org/ontology/shared/device>.
@prefix device: <http://www.nie.org/ontology/shared/device#>.

<http://www.nie.org/ontology/shared/device>
	a owl:Ontology;
	dct:license <http://creativecommons.org/licenses/by/3.0/>;
	dct:title "An ontology about device"@en;
	dct:description """Formal description of a device, general subclasses, related classes and properties."""@en;
	dct:creator "Hans Cools, MD, knowledge engineer, ontologist, software developer, NIE-INE, Basel University, Switzerland"@en;
	dct:publisher "Basel University, Switzerland"@en.

#
# CLASSES
#

device:Device
	a rdfs:Class;
	rdfs:label "device"@en, "Ger채t"@de;
	rdfs:comment """Physical creation serving a particular purpose."""@en;
	rdfs:subClassOf creating:PhysicalCreation.

device:Machine
	a rdfs:Class;
	rdfs:label "machine"@en, "Maschine"@de;
	rdfs:comment """Device having more than one part, each with a function, and transmitting a force or directing its application to perform a task."""@en;
	rdfs:subClassOf device:Device, agent:Agent.

device:MechanicalMachine
	a rdfs:Class;
	rdfs:label "mechanical machine"@en, "mechanische Maschine"@de;
	rdfs:comment """Machine using kinetic energy to perform a task."""@en;
	rdfs:subClassOf device:Machine.

device:ElectricMachine
	a rdfs:Class;
	rdfs:label "electric machine"@en, "elektrische Maschine"@de;
	rdfs:comment """Machine using electric potential energy to convert it via electrical current to kinetic energy to perform a task."""@en;
	rdfs:subClassOf device:Machine.

# device:ElectronicDevice
#	a rdfs:Class;
#	rdfs:label "electronic device"@en, "elektronisches Ger채t"@de;
#	rdfs:comment """Device using electrical current in serving a particular purpose."""@en;
#	rdfs:subClassOf device:Device.

device:ElectronicMachine
	a rdfs:Class;
	rdfs:label "electronic machine"@en, "elektronische Maschine"@de;
	rdfs:comment """Electric machine manipulating the motion of electrons in an electrical current in ways that add meaningful information to the current, to perform a task."""@en;
	rdfs:subClassOf device:ElectricMachine.

device:Computer
	a rdfs:Class;
	rdfs:label "computer"@en, "Rechner"@de;
	rdfs:comment """Machine using programmed instructions to perform arithmetic and logic operations automatically, to perform a task."""@en;
	rdfs:subClassOf device:Machine.

device:ElectronicComputer
	a rdfs:Class;
	rdfs:label "electronic computer"@en, "elektronische Rechner"@de;
	rdfs:comment """Computer also being an electronic machine."""@en;
	rdfs:subClassOf device:Computer, device:ElectronicMachine.

device:DigitalComputer #째
	a rdfs:Class;
	rdfs:label "digital computer"@en, "digitale Rechner"@de;
	rdfs:comment """Computer ...."""@en; #째
	rdfs:subClassOf device:Computer.

device:DigitalElectronicComputer
	a rdfs:Class;
	rdfs:label "digital electronic computer"@en, "digitale elektronische Rechner"@de;
	rdfs:comment """Electronic computer using digital software and data to perform a task."""@en;
	rdfs:subClassOf device:DigitalComputer, device:ElectronicComputer, infocar:ElectronicCarrier.